[Recomposition][Blame] Add Recomposition skeleton to look at for help with Blame

security/Recomposition.v
@@ -6,480 +6,1593 @@ Require Import Complements.
 
 Require Import Split.
 
-#[local] Instance has_side_stackframe: has_side stackframe :=
-  { in_side s := fun '(Stackframe b _ _ _) δ => s b = δ  }.
-
-#[local] Instance has_side_stack: has_side stack :=
-  { in_side s := fun st δ => List.Forall (fun f => s |= f ∈ δ) st }.
-
 Print Instances has_side.
 
-#[local] Instance has_side_regset: has_side regset :=
-  (* { in_side '(s, ge) := fun (rs: regset) δ => s (@Genv.find_comp fundef unit _ ge (rs PC)) = δ }. (* FIXME *) *)
-  { in_side '(s, ge) := fun (rs: regset) δ => exists cp, @Genv.find_comp fundef unit _ ge (rs PC) = Some cp /\ s cp = δ }.
-  
-
-Variant match_fundef (s: split) (δ: side): unit -> fundef -> fundef -> Prop :=
-  | match_function_opp: forall cp sig code code',
-      s |= cp ∈ opposite δ ->
-      match_fundef s δ tt (Internal {| fn_comp := cp; fn_sig := sig; fn_code := code |})
+Variant match_fundef: fundef -> fundef -> Prop :=
+  | match_fundef_internal:
+    forall cp sig code code',
+      match_fundef (Internal {| fn_comp := cp; fn_sig := sig; fn_code := code |})
         (Internal {| fn_comp := cp; fn_sig := sig; fn_code := code' |})
-  | match_external_opp: forall ef,
-      s |= ef ∈ opposite δ ->
-      match_fundef s δ tt (External ef) (External ef)
-  | match_δ : forall fd,
-      s |= fd ∈ δ ->
-      match_fundef s δ tt fd fd
+  | match_fundef_external:
+    forall ef,
+      match_fundef (External ef) (External ef)
 .
 
-#[local] Instance has_comp_match_fundef (s: split) (δ: side): has_comp_match (match_fundef s δ).
+#[local] Instance has_comp_match_fundef (A: Type): has_comp_match (fun _:A => match_fundef).
 intros ? x y H.
 inv H; auto.
 Qed.
 
 Definition match_varinfo (_ _: unit) := True.
 
-Definition match_prog (s: split) (δ: side) := match_program_gen (match_fundef s δ) match_varinfo.
+Variant match_globdef: globdef fundef unit -> globdef fundef unit -> Prop :=
+  | match_globdef_fundef: forall f f',
+      match_fundef f f' ->
+      match_globdef (Gfun f) (Gfun f')
+  | match_globdef_varinfo: forall v v',
+      match_globvar match_varinfo v v' ->
+      match_globdef (Gvar v) (Gvar v')
+.
 
+Remark match_globdef_refl: forall gd,
+    match_globdef gd gd.
+Proof.
+  intros [[[] |]| []]; repeat constructor.
+Qed.
+
+Definition kept_genv (s: split) (ge: genv) (δ: side) (id: ident): bool :=
+  match Genv.find_symbol ge id with
+  | Some b =>
+      match (Genv.genv_defs ge)!b with
+      | None => false
+      | Some gd => side_eq (s (comp_of gd)) δ
+      end
+  | None => false
+  end.
+
+Definition kept_prog (s: split) (p: program) (δ: side) (id: ident): bool :=
+  kept_genv s (Genv.globalenv p) δ id.
+
+Record match_prog (s: split) (δ: side) (p p__recomp: program): Prop := {
+    match_prog_main:
+    p__recomp.(prog_main) = p.(prog_main);
+    match_prog_public:
+    p__recomp.(prog_public) = p.(prog_public);
+    match_prog_pol:
+    p__recomp.(prog_pol) = p.(prog_pol);
+    match_prog_def:
+    forall id,
+      kept_prog s p δ id = true ->
+      (prog_defmap p__recomp)!id = (prog_defmap p)!id;
+    match_prog_notdef:
+    forall id,
+      kept_prog s p δ id = false ->
+      option_rel match_globdef (prog_defmap p)!id (prog_defmap p__recomp)!id ;
+    (* This means that anything defined as public must be defined both in [p] and [p__recomp] *)
+    match_prog_unique:
+    list_norepet (prog_defs_names p__recomp)
+  }.
+
+Section MEMINJ.
+
+  Variable s: split.
+  Variable δ: side.
+
+  Variable p p__recomp: program.
+  Hypothesis MATCH: match_prog s δ p p__recomp.
+
+
+  Let ge := (Genv.globalenv p).
+  Let ge__recomp := (Genv.globalenv p__recomp).
+
+  Lemma transform_find_symbol_1:
+    forall id b,
+      Genv.find_symbol ge id = Some b ->
+      exists b', Genv.find_symbol ge__recomp id = Some b'.
+  Proof.
+    intros id b H.
+    assert (A: exists g, (prog_defmap p)!id = Some g).
+    { apply prog_defmap_dom. eapply Genv.find_symbol_inversion; eauto. }
+    destruct A as (g & P).
+    destruct (kept_prog s p δ id) eqn:ktept.
+    - apply Genv.find_symbol_exists with g.
+      apply in_prog_defmap.
+      erewrite match_prog_def by eauto. auto.
+    - exploit match_prog_notdef; eauto.
+      intros G; inv G; try congruence.
+      eapply Genv.find_symbol_exists.
+      apply in_prog_defmap; eauto.
+  Qed.
+
+  Lemma transform_find_symbol_2:
+    forall id b,
+      Genv.find_symbol ge__recomp id = Some b ->
+      exists b', Genv.find_symbol ge id = Some b'.
+  Proof.
+    intros id b H.
+    assert (A: exists g, (prog_defmap p__recomp)!id = Some g).
+    { apply prog_defmap_dom. eapply Genv.find_symbol_inversion; eauto. }
+    destruct A as (g & P).
+    destruct (kept_genv s ge δ id) eqn:kept.
+    - erewrite match_prog_def in P by eauto.
+      apply Genv.find_symbol_exists with g.
+      apply in_prog_defmap. auto.
+    - exploit match_prog_notdef; eauto.
+      intros G; inv G; try congruence.
+      eapply Genv.find_symbol_exists.
+      apply in_prog_defmap; eauto.
+  Qed.
+
+  Lemma match_prog_comp_of_main:
+    comp_of_main p__recomp = comp_of_main p.
+  Proof.
+  Admitted.
+
+
+  (** Injections that preserve used globals. *)
+  Record meminj_preserves_globals (j: meminj): Prop := {
+      symbols_inject1: forall id b b' delta,
+        j b = Some (b', delta) ->
+        Genv.find_symbol ge id = Some b ->
+        delta = 0 /\ Genv.find_symbol ge__recomp id = Some b';
+      symbols_inject2: forall id b,
+        Genv.find_symbol ge id = Some b ->
+        exists b', Genv.find_symbol ge__recomp id = Some b' /\ j b = Some(b', 0);
+      symbols_inject3: forall id b',
+        Genv.find_symbol ge__recomp id = Some b' ->
+        exists b, Genv.find_symbol ge id = Some b /\ j b = Some (b', 0);
+      defs_inject: forall b b' delta gd,
+        j b = Some(b', delta) -> Genv.find_def ge b = Some gd ->
+        exists gd', Genv.find_def ge__recomp b' = Some gd' /\
+                 delta = 0 /\
+                 match_globdef gd gd' /\
+                 (forall id, Genv.find_symbol ge id = Some b -> kept_genv s ge δ id = true ->
+                        gd' = gd);
+      defs_rev_inject: forall b b' delta gd,
+        j b = Some(b', delta) -> Genv.find_def ge__recomp b' = Some gd ->
+        exists gd', Genv.find_def ge b = Some gd' /\ delta = 0 /\ match_globdef gd' gd;
+    }.
+
+  Definition init_meminj: meminj :=
+    fun b =>
+      match Genv.invert_symbol ge b with
+      | Some id =>
+          match Genv.find_symbol ge__recomp id with
+          | Some b' => Some (b', 0)
+          | None => None
+          end
+      | None => None
+      end.
+
+  Remark init_meminj_eq:
+    forall id b b',
+      Genv.find_symbol ge id = Some b -> Genv.find_symbol ge__recomp id = Some b' ->
+      init_meminj b = Some(b', 0).
+  Proof.
+    intros. unfold init_meminj. erewrite Genv.find_invert_symbol by eauto.
+    rewrite H0. auto.
+  Qed.
+
+  Remark init_meminj_invert:
+    forall b b' delta,
+      init_meminj b = Some(b', delta) ->
+      delta = 0 /\ exists id, Genv.find_symbol ge id = Some b /\ Genv.find_symbol ge__recomp id = Some b'.
+  Proof.
+    unfold init_meminj; intros.
+    destruct (Genv.invert_symbol ge b) as [id|] eqn:S; try discriminate.
+    destruct (Genv.find_symbol ge__recomp id) as [b''|] eqn:F; inv H.
+    split. auto. exists id. split. apply Genv.invert_find_symbol; auto. auto.
+  Qed.
+
+  Lemma init_meminj_preserves_globals:
+    meminj_preserves_globals init_meminj.
+  Proof.
+    constructor; intros.
+    - exploit init_meminj_invert; eauto. intros (A & id1 & B & C).
+      assert (id1 = id) by (eapply (Genv.genv_vars_inj ge); eauto). subst id1.
+      auto.
+    - exploit transform_find_symbol_1; eauto. intros (b' & F). exists b'; split; auto.
+      eapply init_meminj_eq; eauto.
+    - exploit transform_find_symbol_2; eauto. intros (b & F).
+      exists b; split; auto. eapply init_meminj_eq; eauto.
+    - exploit init_meminj_invert; eauto. intros (A & id & B & C).
+      destruct (kept_genv s ge δ id) eqn:kept.
+      + assert ((prog_defmap p)!id = Some gd).
+        { rewrite Genv.find_def_symbol. exists b; auto. }
+        assert ((prog_defmap p__recomp)!id = Some gd).
+        { erewrite match_prog_def by eauto. auto. }
+        rewrite Genv.find_def_symbol in H2. destruct H2 as (b1 & P & Q).
+        fold ge__recomp in P. replace b' with b1 by congruence.
+        exists gd. split; auto. split; auto. split; auto.
+        apply match_globdef_refl.
+      + assert ((prog_defmap p)!id = Some gd).
+        { rewrite Genv.find_def_symbol. exists b; auto. }
+        exploit match_prog_notdef; eauto.
+        intros G; inv G; try congruence.
+        assert (x = gd) by congruence; subst x.
+        symmetry in H3. rewrite Genv.find_def_symbol in H3. destruct H3 as (b1 & P & Q).
+        fold ge__recomp in P. replace b' with b1 by congruence.
+        eexists. split; eauto. split; auto. split; auto.
+        intros id' D. apply Genv.find_invert_symbol in B, D.
+        assert (id = id') by congruence; subst id'. congruence.
+    - exploit init_meminj_invert; eauto. intros (A & id & B & C).
+      destruct (kept_genv s ge δ id) eqn:kept.
+      + assert ((prog_defmap p__recomp)!id = Some gd).
+        { rewrite Genv.find_def_symbol. exists b'; auto. }
+        exists gd; split; [| split]; auto using match_globdef_refl.
+        erewrite match_prog_def in H1 by eauto.
+        rewrite Genv.find_def_symbol in H1. destruct H1 as (b1 & P & Q).
+        fold ge in P. replace b with b1 by congruence. auto.
+      + pose proof Genv.find_def_symbol as F.
+        exploit Genv.find_symbol_find_def_inversion; eauto.
+        intros (gd_recomp & find_gd_recomp).
+        exploit Genv.find_symbol_find_def_inversion; [exact B|].
+        intros (gd_base & find_gd_base).
+        assert (H1: exists b, Genv.find_symbol (Genv.globalenv p) id = Some b /\
+                           Genv.find_def (Genv.globalenv p) b = Some gd_base) by eauto.
+        assert (H2: exists b, Genv.find_symbol (Genv.globalenv p__recomp) id = Some b /\
+                           Genv.find_def (Genv.globalenv p__recomp) b = Some gd_recomp) by eauto.
+        apply F in H1, H2.
+        assert (gd = gd_recomp) by (unfold ge__recomp in *; congruence). subst gd_recomp.
+        eexists; split; [| split]; eauto.
+        exploit match_prog_notdef; eauto. rewrite H1, H2; intros D.
+        inv D; auto.
+  Qed.
+
+  Lemma symbol_address_inject:
+    forall j id ofs,
+      meminj_preserves_globals j ->
+      Val.inject j (Genv.symbol_address ge id ofs) (Genv.symbol_address ge__recomp id ofs).
+  Proof.
+    intros. unfold Genv.symbol_address. destruct (Genv.find_symbol ge id) as [b|] eqn:FS; auto.
+    exploit symbols_inject2; eauto. intros (b' & TFS & INJ). rewrite TFS.
+    econstructor; eauto. rewrite Ptrofs.add_zero; auto.
+  Qed.
+
+  Lemma globals_symbols_inject:
+    forall j, meminj_preserves_globals j -> symbols_inject j ge ge__recomp.
+  Proof.
+    intros.
+    assert (E1: Genv.genv_public ge = p.(prog_public)).
+    { unfold ge. apply Genv.globalenv_public. }
+    assert (E2: Genv.genv_public ge__recomp = p.(prog_public)).
+    { unfold ge__recomp; rewrite Genv.globalenv_public. eapply match_prog_public; eauto. }
+    split; [|split;[|split]]; intros.
+    + simpl; unfold Genv.public_symbol; rewrite E1, E2.
+      destruct (Genv.find_symbol ge__recomp id) as [b'|] eqn:TFS.
+      exploit symbols_inject3; eauto. intros (b & FS & INJ). rewrite FS. auto.
+      destruct (Genv.find_symbol ge id) as [b|] eqn:FS; auto.
+      destruct (in_dec ident_eq id (prog_public p)); simpl; auto.
+      exploit symbols_inject2; eauto.
+      intros (b' & TFS' & INJ). congruence.
+    + eapply symbols_inject1; eauto.
+    + simpl in *; unfold Genv.public_symbol in H0.
+      destruct (Genv.find_symbol ge id) as [b|] eqn:FS; try discriminate.
+      rewrite E1 in H0.
+      destruct (in_dec ident_eq id (prog_public p)); try discriminate. inv H1.
+      exploit symbols_inject2; eauto.
+      intros (b' & A & B); exists b'; auto.
+    + simpl. unfold Genv.block_is_volatile.
+      destruct (Genv.find_var_info ge b1) as [[c gv]|] eqn:V1.
+      rewrite Genv.find_var_info_iff in V1.
+      exploit defs_inject; eauto. intros (gd & A & B & C & D).
+      inv C. inv H2.
+      rewrite <- Genv.find_var_info_iff in A. rewrite A; auto.
+      destruct (Genv.find_var_info ge__recomp b2) as [[c gv]|] eqn:V2; auto.
+      rewrite Genv.find_var_info_iff in V2.
+      exploit defs_rev_inject; eauto. intros (gd & A & B & C).
+      inv C.
+      rewrite <- Genv.find_var_info_iff in A. congruence.
+  Qed.
+
+End MEMINJ.
 Section Invariants.
   Variable s: split.
-
-  Variant stackframe_rel (j: meminj): stackframe -> stackframe -> Prop :=
-    | stackframe_related: forall b b' sg sp sp' ofs ofs',
-        Val.inject j (Vptr b ofs) (Vptr b' ofs') ->
-        Val.inject j sp sp' ->
-        stackframe_rel j (Stackframe b sg sp ofs) (Stackframe b' sg sp' ofs')
-  .
-
-  (* Inductive stack_rel (j: meminj) (δ: side): stack -> stack -> Prop := *)
-  (* | stack_rel_empty: forall st1' st2', *)
-  (*     s |= st1' ∈ opposite δ -> *)
-  (*     s |= st2' ∈ opposite δ -> *)
-  (*     stack_rel j δ st1' st2' *)
-  (* | stack_rel_frame_in_δ: forall st1 st2 st1' st2' f1 f2, *)
-  (*     s |= st1' ∈ opposite δ -> *)
-  (*     s |= st2' ∈ opposite δ -> *)
-  (*     s |= f1 ∈ δ -> *)
-  (*     s |= f2 ∈ δ -> *)
-  (*     stack_rel j δ st1 st2 -> *)
-  (*     stackframe_rel j f1 f2 -> *)
-  (*     stack_rel j δ (st1' ++ f1 :: st1) (st2' ++ f2 :: st2) *)
-  (* . *)
-
-  (* Lemma stack_rel_opposite_cons: *)
-  (*   forall j δ f2 st1 st2, *)
-  (*     s |= f2 ∈ opposite δ -> *)
-  (*     stack_rel j δ st1 st2 -> *)
-  (*     stack_rel j δ st1 (f2 :: st2). *)
-  (* Proof. *)
-  (*   intros. *)
-  (*   induction H0. *)
-  (*   - econstructor; simpl; eauto. *)
-  (*   - eapply stack_rel_frame_in_δ with (st1' := st1') (st2' := f2 :: st2'); simpl; eauto. *)
-  (* Qed. *)
-
-  Inductive stack_rel (j__left j__right: meminj): stack -> stack -> stack -> Prop :=
-  | stack_rel_empty:
-    stack_rel j__left j__right nil nil nil
-  | stack_rel_cons_left: forall st1 st2 st2' st3 f1 f3,
-      stack_rel j__left j__right st1 st2 st3 ->
-      s |= f1 ∈ Left ->
-      s |= st2' ∈ Left ->
-      s |= f3 ∈ Left ->
-      stackframe_rel j__left f1 f3 ->
-      stack_rel j__left j__right (f1 :: st1) (st2' ++ st2) (f3 :: st3)
-  | stack_rel_cons_right: forall st1 st1' st2 st3 f2 f3,
-      stack_rel j__left j__right st1 st2 st3 ->
-      s |= st1' ∈ Right ->
-      s |= f2 ∈ Right ->
-      s |= f3 ∈ Right ->
-      stackframe_rel j__right f2 f3 ->
-      stack_rel j__left j__right (st1' ++ st1) (f2 :: st2) (f3 :: st3)
-  .
+  Variable cp_main: compartment.
 
   Definition regset_rel (j: meminj) (rs rs': regset): Prop :=
     forall r, Val.inject j (rs r) (rs' r).
 
+  (* idea: we maintain a single injection that is only defined on the elements of δ.
+This injection is going to be trivially preserved, because from elements of δ one cannot
+obtain elements of (opposite δ) from it.
+
+Then, at crossing points we will rely on globals only containing scalars to reconstruct
+a bigger injection using mem_inj_disjoint_union. This injection will satisfy
+meminj_preserves_globals which will allow us to prove preservation of events.
+   *)
+  Definition same_domain (s: split) (ge: genv) (j: meminj) (δ: side) (m: mem): Prop :=
+    forall b, (j b <> None <-> ((s, m) |= b ∈ δ) \/ exists fd, Genv.find_def ge b = Some (Gfun fd)).
+
+  Definition mem_delta_zero (j: meminj): Prop :=
+    forall loc loc' delta, j loc = Some (loc', delta) -> delta = 0.
 
   Record mem_rel (ge1 ge2: genv) (j: meminj) (δ: side) (m1 m2: mem) :=
     { (* Uncomment as needed *)
-      same_dom: Mem.same_domain s j δ m1;
+      same_dom: same_domain s ge1 j δ m1;
 
       partial_mem_inject: Mem.inject j m1 m2;
 
-      delta_zero: Mem.delta_zero j;
+      delta_zero: mem_delta_zero j;
 
-      symb_inj: symbols_inject j ge1 ge2;
       (* pres_globals: meminj_preserves_globals ge1 j; *)
       ple_nextblock1: Ple (Senv.nextblock ge1) (Mem.nextblock m1);
       ple_nextblock2: Ple (Senv.nextblock ge2) (Mem.nextblock m2);
 
       (* Functions *)
-      funct_preserved1: forall b fd, Genv.find_funct_ptr ge1 b = Some fd -> j b = Some (b, 0);
-      funct_preserved2: forall b1 b2 fd, Genv.find_funct_ptr ge2 b2 = Some fd -> j b1 = Some (b2, 0) -> b1 = b2;
-      (* Varinfo *)
-      var_info_valid: forall b gv, Genv.find_var_info ge2 b = Some gv -> Mem.valid_block m2 b;
+      (* funct_preserved1: forall b fd, Genv.find_funct_ptr ge1 b = Some fd -> j b = Some (b, 0); *)
+      (* funct_preserved2: forall b1 b2 fd, Genv.find_funct_ptr ge2 b2 = Some fd -> j b1 = Some (b2, 0) -> b1 = b2; *)
+      (* Find def valid *)
+      find_def_valid1: forall b gd, Genv.find_def ge1 b = Some gd -> Mem.valid_block m1 b;
+      find_def_valid2: forall b gd, Genv.find_def ge2 b = Some gd -> Mem.valid_block m2 b;
 
-      (* genv_preserved: Separation.globalenv_preserved ge1 j (Senv.nextblock ge1); *)
+      (* Functions perm *)
+      find_def_perm1: forall b fd, Genv.find_def ge1 b = Some (Gfun fd) -> forall ofs, not (Mem.perm m1 b ofs Max Readable);
+      find_def_perm2: forall b fd, Genv.find_def ge2 b = Some (Gfun fd) -> forall ofs, not (Mem.perm m2 b ofs Max Readable);
 
       same_high_half: forall id ofs,
         Val.inject j (high_half ge1 id ofs) (high_half ge2 id ofs)
     }.
 
-  Inductive strong_equivalence (ge ge': genv) (j: meminj) (δ: side): state -> state -> Prop :=
-  | strong_equivalence_State: forall st st' rs rs' m m',
-      (s, ge) |= rs ∈ δ ->
-      (* (s, ge') |= rs' ∈ δ -> *)
-      (* stack_rel j δ st st' -> *)
-      regset_rel j rs rs' ->
-      mem_rel ge ge' j δ m m' ->
-      strong_equivalence ge ge' j δ (State st rs m) (State st' rs' m')
-  | strong_equivalence_ReturnState: forall st st' rs rs' m m',
-      (s, ge) |= rs ∈ δ ->
-      (* (s, ge') |= rs' ∈ δ -> *)
-      (* stack_rel j δ st st' -> *)
-      regset_rel j rs rs' ->
-      mem_rel ge ge' j δ m m' ->
-      strong_equivalence ge ge' j δ (ReturnState st rs m default_compartment) (ReturnState st' rs' m' default_compartment) (* FIXME *)
-  .
+  Definition def_on_addressable (ge: genv) (j: meminj) (δ: side) :=
+    forall id b cp,
+      Genv.find_symbol ge id = Some b ->
+      s cp = δ ->
+      (Genv.find_comp_of_block ge b = Some cp \/
+        exists fd, Genv.find_def ge b = Some (Gfun fd)) ->
+      exists b' delta, j b = Some (b', delta).
 
-  Inductive weak_equivalence (ge ge': genv) (j: meminj) (δ: side): state -> state -> Prop :=
-  | weak_equivalence_State: forall st st' rs rs' m m',
-      (s, ge) |= rs ∈ opposite δ ->
-      (* (s, ge') |= rs' ∈ opposite δ -> *)
-      (* stack_rel j δ st st' -> *)
-      mem_rel ge ge' j δ m m' ->
-      weak_equivalence ge ge' j δ (State st rs m) (State st' rs' m')
-  | weak_equivalence_ReturnState: forall st st' rs rs' m m',
-      (s, m) |= rs PC ∈ opposite δ ->
-      (* (s, m') |= rs' PC ∈ opposite δ -> *)
-      (* stack_rel j δ st st' -> *)
-      mem_rel ge ge' j δ m m' ->
-      weak_equivalence ge ge' j δ (ReturnState st rs m default_compartment) (ReturnState st' rs' m' default_compartment) (* FIXME *)
-  .
+  Lemma def_on_addressable_incr:
+    forall ge j j' δ,
+      def_on_addressable ge j δ ->
+      inject_incr j j' ->
+      def_on_addressable ge j' δ.
+  Proof.
+    intros ge j j' δ addr incr.
+    intros ? ? ? ? ? ?. exploit addr; eauto.
+    intros (? & ? & G). apply incr in G. eauto.
+  Qed.
+
+  Definition agrees_with (j1 j2: meminj) :=
+    forall b b' b'' delta' delta'',
+      j1 b = Some (b', delta') ->
+      j2 b = Some (b'', delta'') ->
+      b' = b'' /\ delta' = delta''.
+  
+  Lemma agrees_with_incr1:
+    forall j j' b1 jref,
+      agrees_with j jref ->
+      j' b1 = None ->
+      (forall b : block, b <> b1 -> j' b = j b) ->
+      agrees_with j' jref.
+  Proof.
+    intros j j' b1 jref agr isnone diff.
+    intros ? ? ? ? ? ? ?. exploit agr; eauto.
+    rewrite diff in H; eauto.
+    intros ?; congruence.
+  Qed.
+
+  Lemma agrees_with_incr2:
+    forall j j' b1 jref,
+      agrees_with j jref ->
+      jref b1 = None ->
+      (forall b : block, b <> b1 -> j' b = j b) ->
+      agrees_with j' jref.
+  Proof.
+    intros j j' b1 jref agr isnone diff.
+    intros ? ? ? ? ? ? ?. exploit agr; eauto.
+    rewrite diff in H; eauto.
+    intros ?; congruence.
+  Qed.
 
 End Invariants.
 
 
-Section Simulation.
-  Context (c1 c2 p1 p2: Asm.program).
-  Variable s: split.
+Arguments opposite /.
 
-  Context (W1 W2 W3: Asm.program).
-  Hypothesis c1_p1: link p1 c1 = Some W1.
-  Hypothesis c2_p2: link p2 c2 = Some W2.
-  Hypothesis c2_p1: link p1 c2 = Some W3.
+Lemma store_preserves_weak:
+  forall s ge1 ge3 j ch cp b ofs v m1 m1' m3,
+    Mem.store ch m1 b ofs v cp = Some m1' ->
+    mem_rel s ge1 ge3 j (opposite (s cp)) m1 m3 ->
+    mem_rel s ge1 ge3 j (opposite (s cp)) m1' m3.
+Proof.
+  intros s ge1 ge3 j ch cp b ofs v m1 m1' m3 exec m1_m3.
+  assert (j b = None).
+  { pose proof (same_dom _ _ _ _ _ m1 m3 m1_m3 b) as dom.
+    exploit Mem.store_valid_access_3; eauto. intros (_ & access_block & _).
+    simpl in access_block, dom, m1_m3.
+    rewrite access_block in dom.
+    destruct (j b) eqn:C; auto.
+    assert (H: Some p <> None) by congruence.
+    apply dom in H.
+    destruct H as [H | (id & H)].
+    destruct (s cp); try congruence.
+    Local Transparent Mem.store.
+    unfold Mem.store in exec.
+    destruct Mem.valid_access_dec as [[e _] | n]; try congruence.
+    eapply Mem.range_perm_max in e.
+    assert (sz: ofs <= ofs < ofs + size_chunk ch) by now (destruct ch; simpl; lia).
+    specialize (e ofs sz).
+    exploit find_def_perm1; eauto.
+    eapply Mem.perm_implies; eauto; try constructor.
+    now auto. }
+  constructor.
+  - intros b'; apply same_dom in m1_m3; specialize (m1_m3 b').
+    simpl in *. erewrite Mem.store_block_compartment; eauto.
+  - eapply Mem.store_unmapped_inject; eauto using partial_mem_inject.
+  - eapply delta_zero; eauto.
+  - erewrite Mem.nextblock_store; eauto using ple_nextblock1.
+  - eapply ple_nextblock2; eauto.
+  - intros. eapply Mem.store_valid_block_1; eauto using find_def_valid1.
+  - intros. eapply find_def_valid2; eauto.
+  - intros. eapply find_def_perm1 with (b := b0) in m1_m3; eauto.
+    intros n. apply m1_m3. eapply Mem.perm_store_2; eauto.
+  - intros. eapply find_def_perm2 with (b := b0) in m1_m3; eauto.
+  - intros. eapply same_high_half; eauto.
+Qed.
 
-  Hypothesis match_W1_W3: match_prog s Left tt W1 W3.
-  Hypothesis match_W2_W3: match_prog s Right tt W2 W3.
+Lemma exec_store_preserves_weak:
+  forall s ge1 ge3 j cp ch m1 m1' m3 rs1 rs1' rs ra ofs,
+    exec_store ge1 ch rs1 m1 rs ra ofs cp = Next rs1' m1' ->
+    mem_rel s ge1 ge3 j (opposite (s cp)) m1 m3 ->
+    mem_rel s ge1 ge3 j (opposite (s cp)) m1' m3.
+Proof.
+  intros s ge1 ge3 j cp ch m1 m1' m3 rs1 rs1' rs ra ofs exec m1_m3.
+  unfold exec_store in exec.
+  destruct Mem.storev eqn:m1_m1'; try congruence; inv exec.
+  destruct (rs1 ra); simpl in *; try congruence.
+  now eapply store_preserves_weak; eauto.
+Qed.
+
+Lemma alloc_preserves_weak:
+  forall s δ W1 (_: list_norepet (prog_defs_names W1)) W3 j cp lo hi m1 m1' b1 m3,
+    Mem.alloc m1 cp lo hi = (m1', b1) ->
+    agrees_with j (init_meminj W1 W3) ->
+    def_on_addressable s (Genv.globalenv W1) j δ ->
+    mem_rel s (Genv.globalenv W1) (Genv.globalenv W3) j (opposite (s cp)) m1 m3 ->
+    exists j',
+    agrees_with j' (init_meminj W1 W3) /\
+    def_on_addressable s (Genv.globalenv W1) j' δ /\
+      mem_rel s (Genv.globalenv W1) (Genv.globalenv W3) j' (opposite (s cp)) m1' m3 /\ inject_incr j j'.
+Proof.
+  intros s δ W1 norepet1 W3 j cp lo hi m1 m1' b1 m3 exec agr addr m1_m3.
+  exploit Mem.alloc_left_unmapped_inject; eauto using partial_mem_inject.
+  intros (j' & m1'_m3 & incr & j'_b1 & same_inj).
+  exists j'. split; [| split; [| split]]; auto.
+  now eapply agrees_with_incr1; eauto.
+  now eapply def_on_addressable_incr; eauto.
+  constructor.
+  - intros b; apply same_dom in m1_m3; specialize (m1_m3 b).
+    simpl in *.
+    erewrite Mem.alloc_block_compartment; eauto.
+    destruct eq_block; try congruence; [| rewrite same_inj; auto].
+    subst b1. rewrite j'_b1.
+    assert (H: j b = None).
+    { destruct (j b) as [[]|] eqn:?; auto.
+      exploit incr; eauto. congruence. }
+    rewrite H in m1_m3.
+    destruct (s cp); simpl in *; intuition congruence.
+  - auto.
+  - intros b b' delta.
+    destruct (eq_block b b1); try congruence.
+    rewrite same_inj; eauto.
+    eapply delta_zero; eauto.
+  - apply ple_nextblock1 in m1_m3. erewrite Mem.nextblock_alloc; eauto using ple_nextblock1.
+    eapply Ple_trans; eauto using Ple_succ.
+  - eapply ple_nextblock2; eauto.
+  - intros. eapply Mem.valid_block_alloc; eauto using find_def_valid1.
+  - intros. eapply find_def_valid2; eauto.
+  - intros.
+    pose proof (ple_nextblock1 _ _ _ _ _ m1 m3 m1_m3) as ple.
+    eapply find_def_perm1 with (b := b) in m1_m3; eauto.
+    intros n. apply m1_m3.
+    eapply Mem.perm_alloc_4; eauto.
+    eapply Genv.find_def_find_symbol_inversion in H as [id H]; eauto.
+    exploit (Senv.find_symbol_below (Genv.globalenv W1)); eauto. intros ?.
+    exploit Mem.alloc_result; eauto. intros ->.
+    intros ->. eapply Plt_strict.
+    eapply Plt_Ple_trans; eauto.
+  - intros. eapply find_def_perm2; eauto.
+  - intros id ofs. eapply val_inject_incr; eauto using same_high_half.
+Qed.
+
+Lemma extcall_preserves_mem_rel_same_side:
+  forall s ge1 ge3 j j' m1 m1' m3 m3' ef vres vres' t vargs vargs' δ,
+    Mem.unchanged_on (loc_unmapped j) m1 m1' ->
+    inject_incr j j' ->
+    inject_separated j j' m1 m3 ->
+    (forall b : block,
+        (Mem.valid_block m1 b -> False) ->
+        Mem.valid_block m1' b ->
+        exists b' : block,
+          j' b = Some (b', 0) /\ Mem.block_compartment m1' b = Some (comp_of ef)) ->
+    s (comp_of ef) = δ ->
+    mem_rel s ge1 ge3 j δ m1 m3 ->
+    Mem.inject j' m1' m3' ->
+    external_call ef ge1 vargs m1 t vres m1' ->
+    external_call ef ge3 vargs' m3 t vres' m3' ->
+    mem_rel s ge1 ge3 j' δ m1' m3'.
+Proof.
+  intros s ge1 ge3 j j' m1 m1' m3 m3' ef vres vres' t vargs vargs' δ
+    unchanged inj_incr inj_sep comp_new comp_ef m1_m3 inj_m1'_m3' extcall1 extcall3.
+  constructor.
+  - (* same domain *)
+    intros b. apply same_dom in m1_m3. specialize (m1_m3 b).
+    destruct (j b) as [[] |] eqn:j_b.
+    + apply inj_incr in j_b.
+      split; try congruence.
+      intros _. destruct m1_m3 as [side_b _].
+      exploit side_b; try congruence.
+      simpl. destruct (Mem.block_compartment m1 b) eqn:?; try contradiction. intros ?.
+      pose proof (ec_can_access_block (external_call_spec _) _ _ _ _ _ _ b (Some c) extcall1) as G.
+      simpl in G. rewrite G; auto.
+      intros [? | ?]; try contradiction. right; auto.
+    + destruct m1_m3 as [C1 C2].
+      simpl in C1, C2; simpl.
+      split.
+      * destruct (j' b) as [[] |] eqn:j'_b; try congruence; intros _.
+        exploit inj_sep; eauto.
+        intros [H _].
+        assert (Mem.valid_block m1' b).
+        { pose proof (Mem.mi_freeblocks _ _ _ inj_m1'_m3' b) as G.
+          apply Classical_Prop.NNPP.
+          intros ?. exploit G; eauto. congruence. }
+        exploit comp_new; eauto. intros [? [? ->]].
+        auto.
+      * clear C1.
+        destruct (Mem.block_compartment m1 b) as [cp |] eqn:cp_b.
+        { destruct (side_eq (s cp) δ) eqn:?; [exploit C2; eauto|].
+          assert (Mem.valid_block m1 b).
+          { unfold Mem.valid_block.
+            pose proof (Mem.nextblock_compartments m1 b) as G.
+            apply proj1 in G. apply Classical_Prop.NNPP.
+            intros H. apply G in H.
+            now unfold Mem.block_compartment in cp_b; congruence. }
+          apply Mem.unchanged_on_own with (b := b) (cp := Some cp) in unchanged; auto.
+          simpl in unchanged.
+          rewrite unchanged in cp_b. rewrite cp_b. intros A; specialize (C2 A); congruence. }
+        (* clear C2. *)
+        destruct (Mem.block_compartment m1' b) as [cp |] eqn:cp_b';
+          [| intros A; specialize (C2 A); congruence].
+        intros [H | H].
+        -- assert (Mem.valid_block m1' b).
+           { unfold Mem.valid_block.
+             pose proof (Mem.nextblock_compartments m1' b) as G.
+             apply proj1 in G. apply Classical_Prop.NNPP.
+             intros X. apply G in X.
+             now unfold Mem.block_compartment in cp_b'; congruence. }
+           assert (~ Mem.valid_block m1 b).
+           { unfold Mem.valid_block.
+             pose proof (Mem.nextblock_compartments m1 b) as G.
+             apply G. auto. }
+           exploit comp_new; eauto.
+           intros [? [? ?]]. congruence.
+        -- now specialize (C2 (or_intror H)).
+  - (* injection *)
+    assumption.
+  - (* Delta zero *)
+    intros b b' delta j'_b.
+    apply delta_zero in m1_m3; eauto.
+    destruct (j b) as [[] |] eqn:j_b.
+    + exploit m1_m3; eauto. intros ->. exploit inj_incr; eauto. intros. congruence.
+    + exploit inj_sep; eauto.
+      intros [? ?].
+      assert (Mem.valid_block m1' b).
+      { pose proof (Mem.mi_freeblocks _ _ _ inj_m1'_m3' b) as G.
+        apply Classical_Prop.NNPP.
+        intros ?. exploit G; eauto. congruence. }
+      exploit comp_new; eauto. intros [? [? ?]]; congruence.
+  - (* Ple nextblock 1 *)
+    eapply Ple_trans. eapply ple_nextblock1; eauto. eapply external_call_nextblock; eauto.
+  - (* Ple nextblock 2 *)
+    eapply Ple_trans. eapply ple_nextblock2; eauto. eapply external_call_nextblock; eauto.
+  - (* find_def valid 1 *)
+    intros.
+    eapply external_call_valid_block; eauto.
+    eapply find_def_valid1; eauto.
+  - (* find_def valid 2 *)
+    intros.
+    eapply external_call_valid_block; eauto.
+    eapply find_def_valid2; eauto.
+  - intros. intros n. eapply external_call_max_perm in n; eauto.
+    exploit find_def_perm1; eauto.
+    eapply find_def_valid1; eauto.
+  - intros. intros n. eapply external_call_max_perm in n; eauto.
+    exploit find_def_perm2; eauto.
+    eapply find_def_valid2; eauto.
+  - (* same high half *)
+    intros. eapply same_high_half in m1_m3; eauto.
+Qed.
+
+(* Admits were done at some point but I lost the proof (im stupid) *)
+Lemma extcall_preserves_mem_rel_opp_side1: forall s ge1 ge3 j δ m1 m1' m3 ef vargs t vres,
+    s (comp_of ef) = opposite δ ->
+    mem_rel s ge1 ge3 j δ m1 m3 ->
+    external_call ef ge1 vargs m1 t vres m1' ->
+    mem_rel s ge1 ge3 j δ m1' m3.
+Proof.
+  intros s ge1 ge3 j δ m1 m1' m3 ef vargs t vres side_ef m1_m3 extcall.
+  constructor.
+  - (* same domain *)
+    intros b. apply same_dom in m1_m3. specialize (m1_m3 b).
+    destruct (j b) as [[] |] eqn:j_b.
+    + split; try congruence.
+      intros _. destruct m1_m3 as [side_b _].
+      exploit side_b; try congruence.
+      simpl. destruct (Mem.block_compartment m1 b) eqn:?; try contradiction. intros ?.
+      pose proof (ec_can_access_block (external_call_spec _) _ _ _ _ _ _ b (Some c) extcall) as G.
+      simpl in G. rewrite G; auto.
+      admit.
+    + destruct m1_m3 as [C1 C2].
+      simpl in C1, C2; simpl.
+      split.
+      * congruence.
+      * admit.
+  - (* injection *)
+    exploit ec_mem_outside_compartment; eauto using external_call_spec.
+    intros unchanged. exploit partial_mem_inject; eauto.
+    apply same_dom in m1_m3. rename m1_m3 into dom_j_m1.
+    intros m1_m3.
+    constructor.
+    + apply Mem.mi_inj in m1_m3 as mi_inj_m1_m3.
+      constructor.
+      * intros b1 b2 delta ofs k p j_b1 perm1.
+        assert (loc_not_in_compartment (comp_of ef) m1 b1 ofs).
+        { unfold loc_not_in_compartment.
+          assert (G: j b1 <> None) by congruence.
+          apply dom_j_m1 in G. simpl in G.
+          destruct (Mem.block_compartment m1 b1) eqn:?; try congruence.
+          fold (Mem.can_access_block m1 b1 (Some c)) in Heqo.
+          exploit Mem.can_access_block_inj; eauto.
+          simpl. intros ?. admit. }
+        eapply Mem.mi_perm; eauto.
+        eapply Mem.perm_unchanged_on_2; eauto.
+        eapply Mem.valid_block_inject_1; eauto.
+      * intros b1 b2 delta cp j_b1 b1_cp.
+        exploit Mem.can_access_block_inj; eauto.
+        rewrite Mem.unchanged_on_own; eauto.
+        eapply Mem.valid_block_inject_1; eauto.
+      * intros b1 b2 delta chunk ofs p j_b1 range_perm.
+        eapply Mem.mi_align; eauto.
+        admit.
+      * admit.
+    + intros b not_valid_m1.
+      eapply Mem.mi_freeblocks; eauto. intros ?.
+      exploit ec_valid_block; eauto using external_call_spec.
+    + intros b b' delta j_b.
+      eapply Mem.mi_mappedblocks; eauto.
+    + intros b1 b1' delta1 b2 b2' delta2 ofs1 ofs2 b1_b2 j_b1 j_b2 perm_b1 perm_b2.
+      exploit Mem.mi_no_overlap; eauto.
+      eapply Mem.perm_unchanged_on_2; eauto. admit. admit.
+      eapply Mem.perm_unchanged_on_2; eauto. admit. admit.
+    + intros b b' delta ofs j_b [perm | perm].
+      * eapply Mem.mi_representable; eauto. admit.
+      * eapply Mem.mi_representable; eauto. admit.
+    + admit.
+  - (* Delta zero *)
+    intros b b' delta j'_b.
+    apply delta_zero in m1_m3; eauto.
+  - (* Ple nextblock 1 *)
+    eapply Ple_trans. eapply ple_nextblock1; eauto. eapply external_call_nextblock; eauto.
+  - (* Ple nextblock 2 *)
+    eapply ple_nextblock2; eauto.
+  - (* find_def valid 1 *)
+    intros. eapply external_call_valid_block; eauto.
+    eapply find_def_valid1; eauto.
+  - (* find_def valid 2 *)
+    eapply find_def_valid2; eauto.
+  - (* find def perm 1 *)
+    intros. intros n. eapply external_call_max_perm in n; eauto.
+    exploit find_def_perm1; eauto.
+    eapply find_def_valid1; eauto.
+  - (* find def perm 2 *)
+    eapply find_def_perm2; eauto.
+  - (* same high half *)
+    intros. eapply same_high_half in m1_m3; eauto.
+Admitted.
+
+Lemma extcall_preserves_mem_rel_opp_side2: forall s ge1 ge3 j δ m1 m3 m3' ef vargs t vres,
+    s (comp_of ef) = opposite δ ->
+    mem_rel s ge1 ge3 j δ m1 m3 ->
+    external_call ef ge3 vargs m3 t vres m3' ->
+    mem_rel s ge1 ge3 j δ m1 m3'.
+Proof.
+  intros s ge1 ge3 j δ m1 m3 m3' ef vargs t vres side_ef m1_m3 extcall.
+  constructor.
+  - (* same dom *)
+    eapply same_dom in m1_m3; eauto.
+  - (* injection *)
+    exploit ec_mem_outside_compartment; eauto using external_call_spec.
+    intros unchanged. exploit partial_mem_inject; eauto.
+    apply same_dom in m1_m3. rename m1_m3 into dom_j_m1.
+    intros m1_m3.
+    constructor.
+    + apply Mem.mi_inj in m1_m3 as mi_inj_m1_m3.
+      constructor.
+      * intros b1 b2 delta ofs k p j_b1 perm1.
+        eapply Mem.perm_unchanged_on; eauto.
+        { unfold loc_not_in_compartment.
+          assert (G: j b1 <> None) by congruence.
+          apply dom_j_m1 in G. simpl in G.
+          destruct G as [G | G].
+          destruct (Mem.block_compartment m1 b1) eqn:?; try congruence.
+          fold (Mem.can_access_block m1 b1 (Some c)) in Heqo.
+          exploit Mem.can_access_block_inj; eauto.
+          simpl. intros ->.
+          destruct δ; simpl in *; congruence.
+          admit.
+        }
+        eapply Mem.mi_perm; eauto.
+      * intros b1 b2 delta cp j_b1 b1_cp.
+        rewrite <- Mem.unchanged_on_own; eauto.
+        { exploit Mem.can_access_block_inj; eauto. }
+        eapply Mem.valid_block_inject_2; eauto.
+      * intros b1 b2 delta chunk ofs p j_b1 range_perm.
+        eapply Mem.mi_align; eauto.
+      * intros b1 ofs b2 delta j_b1 perm.
+        erewrite Mem.unchanged_on_contents with (m_after := m3') (m_before := m3); eauto using Mem.mi_memval.
+        { unfold loc_not_in_compartment.
+          assert (G: j b1 <> None) by congruence.
+          apply dom_j_m1 in G. simpl in G.
+          destruct (Mem.block_compartment m1 b1) eqn:?; try congruence.
+          fold (Mem.can_access_block m1 b1 (Some c)) in Heqo.
+          exploit Mem.can_access_block_inj; eauto.
+          simpl. intros ->. admit. admit. }
+        eapply Mem.mi_perm; eauto.
+    + intros b not_valid_m1.
+      now eapply Mem.mi_freeblocks; eauto.
+    + intros b b' delta j_b.
+      exploit ec_valid_block; eauto using external_call_spec.
+      eapply Mem.mi_mappedblocks; eauto.
+    + intros b1 b1' delta1 b2 b2' delta2 ofs1 ofs2 b1_b2 j_b1 j_b2 perm_b1 perm_b2.
+      eapply Mem.mi_no_overlap; eauto.
+    + intros b b' delta ofs j_b [perm | perm].
+      * eapply Mem.mi_representable; eauto.
+      * eapply Mem.mi_representable; eauto.
+    + intros b1 ofs b2 delta k p j_b1 perm.
+      exploit Mem.mi_perm_inv; eauto.
+      exploit Mem.perm_unchanged_on_2; eauto.
+      { unfold loc_not_in_compartment.
+        assert (G: j b1 <> None) by congruence.
+        apply dom_j_m1 in G. simpl in G.
+        destruct (Mem.block_compartment m1 b1) eqn:?; try congruence.
+        fold (Mem.can_access_block m1 b1 (Some c)) in Heqo.
+        exploit Mem.can_access_block_inj; eauto using Mem.mi_inj.
+        simpl. intros ->. admit. admit. }
+      eapply Mem.valid_block_inject_2; eauto.
+  - (* Delta zero *)
+    intros b b' delta j'_b.
+    apply delta_zero in m1_m3; eauto.
+  - (* Ple nextblock 1 *)
+    eapply ple_nextblock1; eauto.
+  - (* Ple nextblock 2 *)
+    eapply Ple_trans. eapply ple_nextblock2; eauto. eapply external_call_nextblock; eauto.
+  - (* find_def valid 1 *)
+    intros. eapply find_def_valid1; eauto.
+  - (* find_def valid 2 *)
+    intros. eapply external_call_valid_block; eauto.
+    eapply find_def_valid2; eauto.
+  - (* find_def perm 1 *)
+    intros. eapply find_def_perm1; eauto.
+  - (* find_def valid 2 *)
+    intros. intros n. eapply external_call_max_perm in n; eauto.
+    exploit find_def_perm2; eauto.
+    eapply find_def_valid2; eauto.
+  - (* same high half *)
+    intros. eapply same_high_half in m1_m3; eauto.
+Admitted.
+
+(** Useful simplification tactic *)
+(** Taken from Asmgenproof1.v *)
+
+Ltac Simplif :=
+  ((rewrite Asmgenproof0.nextinstr_inv by eauto with asmgen)
+   || (rewrite Asmgenproof0.nextinstr_inv1 by eauto with asmgen)
+   || (rewrite Pregmap.gss)
+   || (rewrite Asmgenproof0.nextinstr_pc)
+   || (rewrite Pregmap.gso by eauto with asmgen)); auto with asmgen.
+
+Ltac Simpl := repeat Simplif.
+
+Ltac Simplif_all :=
+  ((rewrite Asmgenproof0.nextinstr_inv in * by eauto with asmgen)
+   || (rewrite Asmgenproof0.nextinstr_inv1 in * by eauto with asmgen)
+   || (rewrite Pregmap.gss in * )
+   || (rewrite Asmgenproof0.nextinstr_pc in * )
+   || (rewrite Pregmap.gso in * by eauto with asmgen)); auto with asmgen.
+
+Ltac Simpl_all := repeat Simplif_all.
+
+(* Some tactics *)
+Ltac simpl_nextinstr_PC r :=
+  destruct (Pregmap.elt_eq r PC);
+  [subst r; Simpl; eapply Val.offset_ptr_inject; eauto|
+    Simpl].
+
+Lemma ptrofs_of_int_zero:
+  Ptrofs.of_int Int.zero = Ptrofs.zero.
+Proof.
+  Local Transparent Ptrofs.repr Int.repr.
+  simpl.
+  Local Opaque Ptrofs.repr Int.repr.
+  reflexivity.
+Qed.
+
+Lemma lt_xx_false: forall x,
+    Int.lt x x = false.
+Proof.
+  intros. unfold Int.lt. apply zlt_false. lia.
+Qed.
+
+Lemma ltu_xx_false: forall x,
+    Int.ltu x x = false.
+Proof.
+  intros. unfold Int.ltu. apply zlt_false. lia.
+Qed.
+
+Lemma lt64_xx_false: forall x,
+    Int64.lt x x = false.
+Proof.
+  intros. unfold Int64.lt. apply zlt_false. lia.
+Qed.
+
+Lemma ltu64_xx_false: forall x,
+    Int64.ltu x x = false.
+Proof.
+  intros. unfold Int64.ltu. apply zlt_false. lia.
+Qed.
+
+(* Comparisons *)
+
+(* TODO: rename variables *)
+Lemma cmpu_bool_preserved: forall s ge ge' j δ m1' m3 v1 v2 v1' v2' op b,
+    mem_rel s ge ge' j δ m1' m3 ->
+    Val.inject j v1 v1' ->
+    Val.inject j v2 v2' ->
+    Val.cmpu_bool (Mem.valid_pointer m1') op v1 v2 = Some b ->
+    Val.cmpu_bool (Mem.valid_pointer m3) op v1' v2' = Some b.
+Proof.
+  intros until b. intros m1_m3 inj1 inj2.
+  inv inj1; simpl; inv inj2; simpl; destruct Archi.ptr64; simpl; auto; try congruence.
+  - destruct Int.eq; simpl; try congruence. destruct Mem.valid_pointer eqn:valid; simpl; try congruence.
+    eapply Mem.valid_pointer_inject_val in valid; eauto using partial_mem_inject; rewrite valid; simpl; auto.
+    clear valid. destruct Mem.valid_pointer eqn:valid'; simpl; try congruence.
+    assert (delta = 0) by (eapply delta_zero; eauto); subst.
+    eapply Mem.valid_pointer_inject in valid'; eauto using partial_mem_inject.
+    rewrite Ptrofs.add_zero in *. rewrite Z.add_0_r in valid'. rewrite valid'.
+    now rewrite orb_true_r.
+  - destruct Int.eq; simpl; try congruence. destruct Mem.valid_pointer eqn:valid; simpl; try congruence.
+    eapply Mem.valid_pointer_inject_val in valid; eauto using partial_mem_inject; rewrite valid; simpl; auto.
+    clear valid. destruct Mem.valid_pointer eqn:valid'; simpl; try congruence.
+    assert (delta = 0) by (eapply delta_zero; eauto); subst.
+    eapply Mem.valid_pointer_inject in valid'; eauto using partial_mem_inject.
+    rewrite Ptrofs.add_zero in *. rewrite Z.add_0_r in valid'. rewrite valid'.
+    now rewrite orb_true_r.
+  - destruct eq_block; subst; simpl in *; try congruence.
+    + assert (b3 = b2) by congruence; subst; simpl.
+      assert (delta = delta0) by congruence; subst; simpl.
+      destruct eq_block; try congruence.
+      destruct Mem.valid_pointer eqn:valid; simpl; try congruence.
+      eapply Mem.valid_pointer_inject_val in valid; eauto using partial_mem_inject; rewrite valid; simpl; auto.
+      clear valid.
+      destruct Mem.valid_pointer eqn:valid'; simpl; try congruence.
+      assert (delta0 = 0) by (eapply delta_zero; eauto); subst.
+      eapply Mem.valid_pointer_inject in valid'; eauto using partial_mem_inject.
+      rewrite Ptrofs.add_zero in *. rewrite Z.add_0_r in valid'. rewrite valid'. rewrite Ptrofs.add_zero; auto.
+      clear valid'.
+      destruct Mem.valid_pointer eqn:valid''; simpl; try congruence.
+      assert (delta0 = 0) by (eapply delta_zero; eauto); subst.
+      eapply Mem.valid_pointer_inject in valid''; eauto using partial_mem_inject.
+      rewrite Ptrofs.add_zero in *. rewrite Z.add_0_r in valid''. rewrite valid''. rewrite Ptrofs.add_zero; auto.
+      now rewrite orb_true_r.
+      clear valid.
+      destruct Mem.valid_pointer eqn:valid'; simpl; try congruence.
+      assert (delta0 = 0) by (eapply delta_zero; eauto); subst.
+      eapply Mem.valid_pointer_inject in valid'; eauto using partial_mem_inject.
+      rewrite Ptrofs.add_zero in *. rewrite Z.add_0_r in valid'. rewrite valid'. rewrite Ptrofs.add_zero; auto.
+      rewrite orb_true_r. simpl.
+      clear valid'.
+      destruct Mem.valid_pointer eqn:valid''; simpl; try congruence.
+      eapply Mem.valid_pointer_inject in valid''; eauto using partial_mem_inject.
+      rewrite Z.add_0_r in valid''. rewrite valid''. now auto.
+      clear valid''.
+      destruct Mem.valid_pointer eqn:valid'''; simpl; try congruence.
+      eapply Mem.valid_pointer_inject in valid'''; eauto using partial_mem_inject.
+      rewrite Z.add_0_r in valid'''. rewrite valid'''.
+      now rewrite orb_true_r.
+    + destruct eq_block; subst; simpl in *.
+      * destruct Mem.valid_pointer eqn:valid; simpl; try congruence.
+        destruct (Mem.valid_pointer m1' b0) eqn:valid'; simpl; try congruence.
+        assert (delta = 0) by (eapply delta_zero; eauto); subst.
+        assert (delta0 = 0) by (eapply delta_zero; eauto); subst.
+        eapply Mem.mi_no_overlap with (f := j) in n; [| now eapply partial_mem_inject; eauto].
+        specialize (n H H0 (Mem.perm_cur_max _ _ _ _ ((proj1 (Mem.valid_pointer_nonempty_perm _ _ _)) valid))
+                      (Mem.perm_cur_max _ _ _ _ ((proj1 (Mem.valid_pointer_nonempty_perm _ _ _)) valid')));
+          rewrite !Z.add_0_r in n.
+        destruct n; [contradiction |].
+        eapply Mem.valid_pointer_inject_val in valid; eauto using partial_mem_inject; rewrite valid; simpl; auto.
+        eapply Mem.valid_pointer_inject_val in valid'; eauto using partial_mem_inject; rewrite valid'; simpl; auto.
+        destruct op; simpl; try congruence.
+        intros. inv H2. rewrite !Ptrofs.add_zero. unfold Ptrofs.eq. destruct zeq; auto; congruence.
+        intros. inv H2. rewrite !Ptrofs.add_zero. unfold Ptrofs.eq. destruct zeq; auto; congruence.
+      * destruct Mem.valid_pointer eqn:valid; simpl; try congruence.
+        eapply Mem.valid_pointer_inject_val in valid; eauto using partial_mem_inject; rewrite valid; simpl; auto.
+        clear valid.
+        destruct Mem.valid_pointer eqn:valid'; simpl; try congruence.
+        assert (delta = 0) by (eapply delta_zero; eauto); subst.
+        assert (delta0 = 0) by (eapply delta_zero; eauto); subst.
+        eapply Mem.valid_pointer_inject in valid'; eauto using partial_mem_inject.
+        rewrite Ptrofs.add_zero in *. rewrite Z.add_0_r in valid'. rewrite valid'. auto.
+Qed.
+
+
+Lemma cmpu_inject:
+  forall s ge ge' j δ op m1 m3 v1 v1' v2 v2',
+    mem_rel s ge ge' j δ m1 m3 ->
+    Val.inject j v1 v1' ->
+    Val.inject j v2 v2' ->
+    Val.inject j (Val.cmpu (Mem.valid_pointer m1) op v1 v2)
+      (Val.cmpu (Mem.valid_pointer m3) op v1' v2').
+Proof.
+  intros s ge ge' j δ op m1 m3 v1 v1' v2 v2' m1_m3 v1_v1' v2_v2'.
+  unfold Val.cmpu.
+  destruct (Val.cmpu_bool) eqn:eq_cmpu.
+  - eapply cmpu_bool_preserved in eq_cmpu; eauto. rewrite eq_cmpu; now eapply Cminorgenproof.val_inject_val_of_optbool.
+  - auto.
+Qed.
+
+(* TODO: this is the same proof as [cmpu_bool_preserved] above, but with [Int64] substituted for [Int] *)
+Lemma cmplu_bool_preserved: forall s ge ge' j δ m1' m3 v1 v2 v1' v2' op b,
+    mem_rel s ge ge' j δ m1' m3 ->
+    Val.inject j v1 v1' ->
+    Val.inject j v2 v2' ->
+    Val.cmplu_bool (Mem.valid_pointer m1') op v1 v2 = Some b ->
+    Val.cmplu_bool (Mem.valid_pointer m3) op v1' v2' = Some b.
+Proof.
+  intros until b. intros m1_m3 inj1 inj2.
+  inv inj1; simpl; inv inj2; simpl; destruct Archi.ptr64; simpl; auto; try congruence.
+  - destruct Int64.eq; simpl; try congruence. destruct Mem.valid_pointer eqn:valid; simpl; try congruence.
+    eapply Mem.valid_pointer_inject_val in valid; eauto using partial_mem_inject; rewrite valid; simpl; auto.
+    clear valid. destruct Mem.valid_pointer eqn:valid'; simpl; try congruence.
+    assert (delta = 0) by (eapply delta_zero; eauto); subst.
+    eapply Mem.valid_pointer_inject in valid'; eauto using partial_mem_inject.
+    rewrite Ptrofs.add_zero in *. rewrite Z.add_0_r in valid'. rewrite valid'.
+    now rewrite orb_true_r.
+  - destruct Int64.eq; simpl; try congruence. destruct Mem.valid_pointer eqn:valid; simpl; try congruence.
+    eapply Mem.valid_pointer_inject_val in valid; eauto using partial_mem_inject; rewrite valid; simpl; auto.
+    clear valid. destruct Mem.valid_pointer eqn:valid'; simpl; try congruence.
+    assert (delta = 0) by (eapply delta_zero; eauto); subst.
+    eapply Mem.valid_pointer_inject in valid'; eauto using partial_mem_inject.
+    rewrite Ptrofs.add_zero in *. rewrite Z.add_0_r in valid'. rewrite valid'.
+    now rewrite orb_true_r.
+  - destruct eq_block; subst; simpl in *; try congruence.
+    + assert (b3 = b2) by congruence; subst; simpl.
+      assert (delta = delta0) by congruence; subst; simpl.
+      destruct eq_block; try congruence.
+      destruct Mem.valid_pointer eqn:valid; simpl; try congruence.
+      eapply Mem.valid_pointer_inject_val in valid; eauto using partial_mem_inject; rewrite valid; simpl; auto.
+      clear valid.
+      destruct Mem.valid_pointer eqn:valid'; simpl; try congruence.
+      assert (delta0 = 0) by (eapply delta_zero; eauto); subst.
+      eapply Mem.valid_pointer_inject in valid'; eauto using partial_mem_inject.
+      rewrite Ptrofs.add_zero in *. rewrite Z.add_0_r in valid'. rewrite valid'. rewrite Ptrofs.add_zero; auto.
+      clear valid'.
+      destruct Mem.valid_pointer eqn:valid''; simpl; try congruence.
+      assert (delta0 = 0) by (eapply delta_zero; eauto); subst.
+      eapply Mem.valid_pointer_inject in valid''; eauto using partial_mem_inject.
+      rewrite Ptrofs.add_zero in *. rewrite Z.add_0_r in valid''. rewrite valid''. rewrite Ptrofs.add_zero; auto.
+      now rewrite orb_true_r.
+      clear valid.
+      destruct Mem.valid_pointer eqn:valid'; simpl; try congruence.
+      assert (delta0 = 0) by (eapply delta_zero; eauto); subst.
+      eapply Mem.valid_pointer_inject in valid'; eauto using partial_mem_inject.
+      rewrite Ptrofs.add_zero in *. rewrite Z.add_0_r in valid'. rewrite valid'. rewrite Ptrofs.add_zero; auto.
+      rewrite orb_true_r. simpl.
+      clear valid'.
+      destruct Mem.valid_pointer eqn:valid''; simpl; try congruence.
+      eapply Mem.valid_pointer_inject in valid''; eauto using partial_mem_inject.
+      rewrite Z.add_0_r in valid''. rewrite valid''. now auto.
+      clear valid''.
+      destruct Mem.valid_pointer eqn:valid'''; simpl; try congruence.
+      eapply Mem.valid_pointer_inject in valid'''; eauto using partial_mem_inject.
+      rewrite Z.add_0_r in valid'''. rewrite valid'''.
+      now rewrite orb_true_r.
+    + destruct eq_block; subst; simpl in *.
+      * destruct Mem.valid_pointer eqn:valid; simpl; try congruence.
+        destruct (Mem.valid_pointer m1' b0) eqn:valid'; simpl; try congruence.
+        assert (delta = 0) by (eapply delta_zero; eauto); subst.
+        assert (delta0 = 0) by (eapply delta_zero; eauto); subst.
+        eapply Mem.mi_no_overlap with (f := j) in n; [| now eapply partial_mem_inject; eauto].
+        specialize (n H H0 (Mem.perm_cur_max _ _ _ _ ((proj1 (Mem.valid_pointer_nonempty_perm _ _ _)) valid))
+                      (Mem.perm_cur_max _ _ _ _ ((proj1 (Mem.valid_pointer_nonempty_perm _ _ _)) valid')));
+          rewrite !Z.add_0_r in n.
+        destruct n; [contradiction |].
+        eapply Mem.valid_pointer_inject_val in valid; eauto using partial_mem_inject; rewrite valid; simpl; auto.
+        eapply Mem.valid_pointer_inject_val in valid'; eauto using partial_mem_inject; rewrite valid'; simpl; auto.
+        destruct op; simpl; try congruence.
+        intros. inv H2. rewrite !Ptrofs.add_zero. unfold Ptrofs.eq. destruct zeq; auto; congruence.
+        intros. inv H2. rewrite !Ptrofs.add_zero. unfold Ptrofs.eq. destruct zeq; auto; congruence.
+      * destruct Mem.valid_pointer eqn:valid; simpl; try congruence.
+        eapply Mem.valid_pointer_inject_val in valid; eauto using partial_mem_inject; rewrite valid; simpl; auto.
+        clear valid.
+        destruct Mem.valid_pointer eqn:valid'; simpl; try congruence.
+        assert (delta = 0) by (eapply delta_zero; eauto); subst.
+        assert (delta0 = 0) by (eapply delta_zero; eauto); subst.
+        eapply Mem.valid_pointer_inject in valid'; eauto using partial_mem_inject.
+        rewrite Ptrofs.add_zero in *. rewrite Z.add_0_r in valid'. rewrite valid'. auto.
+Qed.
+
+Lemma cmplu_inject:
+  forall s ge ge' j δ op m1 m3 v1 v1' v2 v2',
+    mem_rel s ge ge' j δ m1 m3 ->
+    Val.inject j v1 v1' ->
+    Val.inject j v2 v2' ->
+    Val.inject j (Val.maketotal (Val.cmplu (Mem.valid_pointer m1) op v1 v2))
+      (Val.maketotal (Val.cmplu (Mem.valid_pointer m3) op v1' v2')).
+Proof.
+  intros s ge ge' j δ op m1 m3 v1 v1' v2 v2' m1_m3 v1_v1' v2_v2'.
+  unfold Val.cmplu.
+  destruct (Val.cmplu_bool) eqn:eq_cmplu.
+  - eapply cmplu_bool_preserved in eq_cmplu; eauto. rewrite eq_cmplu.
+    simpl. now eapply Cop.val_inject_of_bool.
+  - auto.
+Qed.
+
+
+Hint Resolve cmpu_inject cmplu_inject : solve_inject.
+Hint Resolve Cop.val_inject_of_bool: solve_inject.
+
+Section Lemmas.
+
+  Context (s: split) (W1 W2 W3: Asm.program) (δ: side).
+
+  Hypothesis norepet1: list_norepet (prog_defs_names W1).
+  Hypothesis norepet2: list_norepet (prog_defs_names W2).
+  Hypothesis norepet3: list_norepet (prog_defs_names W3).
 
   (* Context (ge1 ge2: genv). *)
   Notation ge1 := (Genv.globalenv W1).
   Notation ge2 := (Genv.globalenv W2).
   Notation ge3 := (Genv.globalenv W3).
 
-  Hypothesis same_low_half1: low_half ge1 = low_half ge3.
-  Hypothesis same_low_half2: low_half ge2 = low_half ge3.
-  Hypothesis same_high_half1: high_half ge1 = high_half ge3.
-  Hypothesis same_high_half2: high_half ge2 = high_half ge3.
 
-  Let single_L1 := sd_traces (semantics_determinate W1).
-  Let single_L2 := sd_traces (semantics_determinate W2).
-  Let single_L3 := sd_traces (semantics_determinate W3).
-
-  Lemma public_symbol_eq21: forall (id: ident),
-      Senv.public_symbol (symbolenv (semantics W2)) id = Senv.public_symbol (symbolenv (semantics W1)) id.
+  Lemma alloc_preserves_rel1:
+    forall cp j__δ j__oppδ m1 m1' m2 m3 lo hi b1 rs1 rs3,
+      s |= cp ∈ δ ->
+      agrees_with j__δ (init_meminj W1 W3) ->
+      def_on_addressable s ge1 j__δ δ ->
+      mem_rel s ge1 ge3 j__δ δ m1 m3 ->
+      mem_rel s ge2 ge3 j__oppδ (opposite δ) m2 m3 ->
+      regset_rel j__δ rs1 rs3 ->
+      Mem.alloc m1 cp lo hi = (m1', b1) ->
+      exists j__δ' m3' b3, Mem.alloc m3 cp lo hi = (m3', b3) /\
+                      agrees_with j__δ' (init_meminj W1 W3) /\
+                      def_on_addressable s ge1 j__δ' δ /\
+                      mem_rel s ge1 ge3 j__δ' δ m1' m3' /\
+                      mem_rel s ge2 ge3 j__oppδ (opposite δ) m2 m3' /\
+                      regset_rel j__δ' rs1 rs3 /\
+                      j__δ' b1 = Some (b3, 0) /\
+                      inject_incr j__δ j__δ'.
   Proof.
-    apply Genv.senv_match in match_W1_W3 as [? [? ?]], match_W2_W3 as [? [? ?]]. simpl in *; now intuition.
+    intros cp j__δ j__oppδ m1 m1' m2 m3 lo hi b1 rs1 rs3 side_cp agr addr m1_m3 m2_m3 rs1_rs3 alloc1.
+    exploit (Mem.alloc_parallel_inject j__δ m1); eauto using partial_mem_inject, Z.le_refl.
+    intros [j' [m3' [b3 [? [? [? [? diff]]]]]]].
+    exists j', m3', b3.
+    split; [| split; [| split; [| split; [| split; [| split; [| split]]]]]];
+      [assumption | eapply agrees_with_incr2; eauto | eapply def_on_addressable_incr; eauto | | | intros ?; eauto using val_inject_incr | assumption | assumption].
+    { destruct (init_meminj W1 W3 b1) as [[] |] eqn:?; auto.
+      exploit init_meminj_invert; eauto. intros [-> [id [? ?]]].
+      apply Mem.alloc_result in alloc1; subst.
+
+      pose proof (ple_nextblock1 _ _ _ _ _ _ _ m1_m3).
+      exploit (Senv.find_symbol_below ge1); eauto. intros ?.
+      pose proof (Plt_Ple_trans _ _ _ H6 H5).
+      now exploit Plt_strict; eauto. }
+
+    { clear dependent j__oppδ.
+      constructor.
+      - intros b. destruct (Pos.eq_dec b b1); subst.
+        + split; [| congruence].
+          intros _. apply Mem.owned_new_block in alloc1. simpl in alloc1. left; simpl; now rewrite alloc1.
+        + rewrite (diff _ n).
+          eapply same_dom in m1_m3. specialize (m1_m3 b).
+          eapply Mem.alloc_block_compartment with (b' := b) in alloc1.
+          simpl. rewrite alloc1. rewrite peq_false; eauto.
+      - assumption.
+      - intros b b' delta.
+        destruct (Pos.eq_dec b b1); subst.
+        + congruence.
+        + rewrite (diff _ n).
+          intros G. exploit delta_zero; eauto.
+      - erewrite Mem.nextblock_alloc; eauto using Ple_trans, Ple_succ, ple_nextblock1.
+      - erewrite Mem.nextblock_alloc; eauto using Ple_trans, Ple_succ, ple_nextblock2.
+      - intros. exploit find_def_valid1; eauto. eapply Mem.valid_block_alloc; eauto.
+      - intros. exploit find_def_valid2; eauto. eapply Mem.valid_block_alloc; eauto.
+      - intros.
+        pose proof (ple_nextblock1 _ _ _ _ _ m1 m3 m1_m3) as ple.
+        eapply find_def_perm1 with (b := b) in m1_m3; eauto.
+        intros n. apply m1_m3.
+        eapply Mem.perm_alloc_4; eauto.
+        eapply Genv.find_def_find_symbol_inversion in H3 as [id H3]; eauto.
+        exploit (Senv.find_symbol_below (Genv.globalenv W1)); eauto. intros ?.
+        exploit (Mem.alloc_result m1); eauto. intros ->.
+        intros ->. eapply Plt_strict.
+        eapply Plt_Ple_trans; eauto.
+      - intros.
+        pose proof (ple_nextblock2 _ _ _ _ _ m1 m3 m1_m3) as ple.
+        eapply find_def_perm2 with (b := b) in m1_m3; eauto.
+        intros n. apply m1_m3.
+        eapply Mem.perm_alloc_4; eauto.
+        eapply Genv.find_def_find_symbol_inversion in H3 as [id H3]; eauto.
+        exploit (Senv.find_symbol_below (Genv.globalenv W3)); eauto. intros ?.
+        exploit (Mem.alloc_result m3); eauto. intros -> ->.
+        eapply Plt_strict. eapply Plt_Ple_trans; eauto.
+      - intros id ofs.
+        exploit same_high_half; eauto. }
+    { clear dependent j__δ.
+      destruct m2_m3.
+      constructor; eauto.
+      - eapply Mem.alloc_right_inject; eauto using partial_mem_inject.
+      - erewrite Mem.nextblock_alloc; eauto using Ple_trans, Ple_succ, ple_nextblock1.
+      - intros. eapply Mem.valid_block_alloc; eauto.
+      - intros. intros n.
+        eapply Mem.perm_alloc_4 in n; eauto.
+        eapply find_def_perm4; eauto.
+        intros ->.
+        exploit (Mem.alloc_result m3); eauto. intros ->.
+        eapply Genv.find_def_find_symbol_inversion in H1 as [id H1]; eauto.
+        exploit (Senv.find_symbol_below (Genv.globalenv W3)); eauto. intros ?.
+        eapply Plt_strict. eapply Plt_Ple_trans; eauto. }
   Qed.
 
-  Lemma public_symbol_eq32: forall (id: ident),
-      Senv.public_symbol (symbolenv (semantics W3)) id = Senv.public_symbol (symbolenv (semantics W2)) id.
+  Lemma alloc_preserves_rel2:
+    forall cp j__δ j__oppδ m1 m1' m2 m3 lo hi b1 rs1 rs3,
+      s |= cp ∈ opposite δ ->
+      agrees_with j__δ (init_meminj W1 W3) ->
+      def_on_addressable s ge1 j__δ δ ->
+      mem_rel s ge1 ge3 j__δ δ m1 m3 ->
+      mem_rel s ge2 ge3 j__oppδ (opposite δ) m2 m3 ->
+      regset_rel j__δ rs1 rs3 ->
+      Mem.alloc m1 cp lo hi = (m1', b1) ->
+      exists j__δ' m3' b3, Mem.alloc m3 cp lo hi = (m3', b3) /\
+                      agrees_with j__δ' (init_meminj W1 W3) /\
+                      def_on_addressable s ge1 j__δ' δ /\
+                      mem_rel s ge1 ge3 j__δ' δ m1' m3' /\
+                      mem_rel s ge2 ge3 j__oppδ (opposite δ) m2 m3' /\
+                      regset_rel j__δ' rs1 rs3 /\
+                      inject_incr j__δ j__δ'.
   Proof.
-    apply Genv.senv_match in match_W1_W3 as [? [? ?]], match_W2_W3 as [? [? ?]]. simpl in *; now intuition.
+    intros cp j__δ j__oppδ m1 m1' m2 m3 lo hi b1 rs1 rs3 side_cp agr addr m1_m3 m2_m3 rs1_rs3 alloc1.
+    exploit (Mem.alloc_parallel_inject j__δ m1); eauto using partial_mem_inject, Z.le_refl.
+    intros [_ [m3' [b3 [alloc3 [_ [_ [_ _]]]]]]].
+    exploit (Mem.alloc_left_unmapped_inject j__δ m1); eauto using partial_mem_inject.
+    intros [j' [inj [incr [isnone diff]]]].
+    exploit Mem.alloc_right_inject; eauto. intros inj'.
+    exists j', m3', b3.  split; [| split; [| split; [| split; [| split; [| split]]]]];
+      [assumption | eapply agrees_with_incr1; eauto | eapply def_on_addressable_incr; eauto | | | intros ?; eauto using val_inject_incr | assumption].
+    { clear dependent j__oppδ.
+      constructor; auto.
+      - intros b. destruct (Pos.eq_dec b b1); subst.
+        + split; [congruence |].
+          intros ?. apply Mem.owned_new_block in alloc1. simpl in *. rewrite alloc1 in H.
+          apply same_dom in m1_m3. specialize (m1_m3 b1).
+          destruct m1_m3 as [_ m1_m3].
+          destruct H.
+          * now destruct δ; congruence.
+          * specialize (m1_m3 (or_intror H)).
+            assert (exists b1' delta, j__δ b1 = Some (b1', delta)) as [b1' [? G]]
+                by now (destruct (j__δ b1) as [[]|]; try congruence; eauto).
+            apply incr in G. congruence.
+        + rewrite (diff _ n).
+          eapply same_dom in m1_m3. specialize (m1_m3 b).
+          eapply Mem.alloc_block_compartment with (b' := b) in alloc1.
+          simpl. rewrite alloc1. rewrite peq_false; eauto.
+      - intros b b' delta.
+        destruct (Pos.eq_dec b b1); subst.
+        + congruence.
+        + rewrite (diff _ n).
+          intros G. exploit delta_zero; eauto.
+      - erewrite Mem.nextblock_alloc; eauto using Ple_trans, Ple_succ, ple_nextblock1.
+      - erewrite Mem.nextblock_alloc; eauto using Ple_trans, Ple_succ, ple_nextblock2.
+      - intros. exploit find_def_valid1; eauto. eapply Mem.valid_block_alloc. eauto.
+      - intros. exploit find_def_valid2; eauto. eapply Mem.valid_block_alloc. eauto.
+      - intros. intros n. eapply find_def_perm1; eauto.
+        eapply Mem.perm_alloc_4; eauto.
+        intros ->.
+        exploit (Mem.alloc_result m1); eauto. intros ->.
+        eapply Genv.find_def_find_symbol_inversion in H as [id H]; eauto.
+        exploit (Senv.find_symbol_below (Genv.globalenv W1)); eauto. intros ?.
+        eapply Plt_strict. eapply Plt_Ple_trans; eauto using ple_nextblock1.
+      - intros. intros n. eapply find_def_perm2; eauto.
+        eapply Mem.perm_alloc_4; eauto.
+        intros ->.
+        exploit (Mem.alloc_result m3); eauto. intros ->.
+        eapply Genv.find_def_find_symbol_inversion in H as [id H]; eauto.
+        exploit (Senv.find_symbol_below (Genv.globalenv W3)); eauto. intros ?.
+        eapply Plt_strict. eapply Plt_Ple_trans; eauto using ple_nextblock2.
+      - intros id ofs.
+        exploit same_high_half; eauto.
+    }
+    { clear dependent j__δ.
+      destruct m2_m3.
+      constructor; eauto.
+      - eapply Mem.alloc_right_inject; eauto using partial_mem_inject.
+      - erewrite Mem.nextblock_alloc; eauto using Ple_trans, Ple_succ, ple_nextblock1.
+      - intros. eapply Mem.valid_block_alloc; eauto.
+      - intros. intros n. eapply find_def_perm4; eauto.
+        eapply Mem.perm_alloc_4; eauto.
+        intros ->.
+        exploit (Mem.alloc_result m3); eauto. intros ->.
+        eapply Genv.find_def_find_symbol_inversion in H as [id H]; eauto.
+        exploit (Senv.find_symbol_below (Genv.globalenv W3)); eauto. intros ?.
+        eapply Plt_strict. eapply Plt_Ple_trans; eauto using ple_nextblock2. }
   Qed.
 
-  Local Arguments comp_of /.
-  Local Arguments Genv.find_comp _ /.
-
-  Ltac RecompSimpl :=
-    (* unfold ge1 in *; *)
-    (* unfold ge2 in *; *)
-    (* unfold ge3 in *; *)
-    repeat (simpl in *;
-            multimatch goal with
-            | H: ?rs PC = _, H': context [ ?rs PC ] |- _ => rewrite H in H'; simpl in *; try congruence
-            | H: Genv.find_funct_ptr ?ge ?b = _, H': context [ Genv.find_funct_ptr ?ge ?b ] |- _ =>
-                rewrite H in H'; simpl in *; try congruence
-            | _: context [ Ptrofs.eq_dec Ptrofs.zero Ptrofs.zero ] |- _ => destruct Ptrofs.eq_dec; [| contradiction]
-            | H: regset_rel _ _ _ |- context [PC] =>
-                let H' := fresh "H" in
-                assert (H' := H);
-                specialize (H' PC); inv H'; try congruence
-            | H: Vptr _ _ = Vptr _ _ |- _ => inv H
-            (* | H: _ = ?rs PC, H': context [ ?rs PC ] |- _ => rewrite H in H'; simpl in *; try congruence *)
-            end).
-
-  Ltac exploit_globalenv_preserved :=
-    repeat match goal with
-      | H: Separation.globalenv_preserved _ _ _ |- _ => destruct H as [? ? ? ? ?]
-      | H: forall b, Plt b ?bound -> ?j b = Some (b, 0),
-        H': ?j ?b = Some (_, _),
-        H'': Genv.find_funct_ptr ?ge ?b = Some _,
-        FUNCTIONS : forall b fd, Genv.find_funct_ptr ?ge b = Some fd -> Plt b _ |- _ =>
-          rewrite H in H'; [inv H' | now eapply FUNCTIONS; eauto]
-      end.
-
-  (** Useful simplification tactic *)
-  (** Taken from Asmgenproof1.v *)
-
-  Ltac Simplif :=
-    ((rewrite Asmgenproof0.nextinstr_inv by eauto with asmgen)
-     || (rewrite Asmgenproof0.nextinstr_inv1 by eauto with asmgen)
-     || (rewrite Pregmap.gss)
-     || (rewrite Asmgenproof0.nextinstr_pc)
-     || (rewrite Pregmap.gso by eauto with asmgen)); auto with asmgen.
-
-  Ltac Simpl := repeat Simplif.
-
-  (* Some tactics *)
-  Ltac simpl_nextinstr_PC r :=
-    destruct (Pregmap.elt_eq r PC);
-    [subst r; Simpl; eapply Val.offset_ptr_inject; eauto|
-      Simpl].
-
-
-  Lemma ptrofs_of_int_zero:
-    Ptrofs.of_int Int.zero = Ptrofs.zero.
+  Lemma alloc_preserves_rel:
+    forall cp j__δ j__oppδ m1 m1' m2 m3 lo hi b1 rs1 rs3,
+      agrees_with j__δ (init_meminj W1 W3) ->
+      def_on_addressable s ge1 j__δ δ ->
+      mem_rel s ge1 ge3 j__δ δ m1 m3 ->
+      mem_rel s ge2 ge3 j__oppδ (opposite δ) m2 m3 ->
+      regset_rel j__δ rs1 rs3 ->
+      Mem.alloc m1 cp lo hi = (m1', b1) ->
+      exists j__δ' m3' b3, Mem.alloc m3 cp lo hi = (m3', b3) /\
+                      agrees_with j__δ' (init_meminj W1 W3) /\
+                      def_on_addressable s ge1 j__δ' δ /\
+                      mem_rel s ge1 ge3 j__δ' δ m1' m3' /\
+                      mem_rel s ge2 ge3 j__oppδ (opposite δ) m2 m3' /\
+                      regset_rel j__δ' rs1 rs3 /\
+                      (s |= cp ∈ δ -> j__δ' b1 = Some (b3, 0)) /\
+                      inject_incr j__δ j__δ'.
   Proof.
-    Local Transparent Ptrofs.repr Int.repr.
-    simpl.
-    Local Opaque Ptrofs.repr Int.repr.
-    reflexivity.
-  Qed.
-
-  Lemma lt_xx_false: forall x,
-    Int.lt x x = false.
-  Proof.
-    intros. unfold Int.lt. apply zlt_false. lia.
-  Qed.
-
-  Lemma ltu_xx_false: forall x,
-    Int.ltu x x = false.
-  Proof.
-    intros. unfold Int.ltu. apply zlt_false. lia.
-  Qed.
-
-  Lemma lt64_xx_false: forall x,
-    Int64.lt x x = false.
-  Proof.
-    intros. unfold Int64.lt. apply zlt_false. lia.
-  Qed.
-
-  Lemma ltu64_xx_false: forall x,
-    Int64.ltu x x = false.
-  Proof.
-    intros. unfold Int64.ltu. apply zlt_false. lia.
-  Qed.
-
-  (* Comparisons *)
-
-  (* TODO: rename variables *)
-  Lemma cmpu_bool_preserved: forall ge ge' j δ m1' m3 v1 v2 v1' v2' op b,
-      mem_rel s ge ge' j δ m1' m3 ->
-      Val.inject j v1 v1' ->
-      Val.inject j v2 v2' ->
-      Val.cmpu_bool (Mem.valid_pointer m1') op v1 v2 = Some b ->
-      Val.cmpu_bool (Mem.valid_pointer m3) op v1' v2' = Some b.
-  Proof.
-    intros until b. intros m1_m3 inj1 inj2.
-    inv inj1; simpl; inv inj2; simpl; destruct Archi.ptr64; simpl; auto; try congruence.
-    - destruct Int.eq; simpl; try congruence. destruct Mem.valid_pointer eqn:valid; simpl; try congruence.
-      eapply Mem.valid_pointer_inject_val in valid; eauto using partial_mem_inject; rewrite valid; simpl; auto.
-      clear valid. destruct Mem.valid_pointer eqn:valid'; simpl; try congruence.
-      assert (delta = 0) by (eapply delta_zero; eauto); subst.
-      eapply Mem.valid_pointer_inject in valid'; eauto using partial_mem_inject.
-      rewrite Ptrofs.add_zero in *. rewrite Z.add_0_r in valid'. rewrite valid'.
-      now rewrite orb_true_r.
-    - destruct Int.eq; simpl; try congruence. destruct Mem.valid_pointer eqn:valid; simpl; try congruence.
-      eapply Mem.valid_pointer_inject_val in valid; eauto using partial_mem_inject; rewrite valid; simpl; auto.
-      clear valid. destruct Mem.valid_pointer eqn:valid'; simpl; try congruence.
-      assert (delta = 0) by (eapply delta_zero; eauto); subst.
-      eapply Mem.valid_pointer_inject in valid'; eauto using partial_mem_inject.
-      rewrite Ptrofs.add_zero in *. rewrite Z.add_0_r in valid'. rewrite valid'.
-      now rewrite orb_true_r.
-    - destruct eq_block; subst; simpl in *; try congruence.
-      + assert (b3 = b2) by congruence; subst; simpl.
-        assert (delta = delta0) by congruence; subst; simpl.
-        destruct eq_block; try congruence.
-        destruct Mem.valid_pointer eqn:valid; simpl; try congruence.
-        eapply Mem.valid_pointer_inject_val in valid; eauto using partial_mem_inject; rewrite valid; simpl; auto.
-        clear valid.
-        destruct Mem.valid_pointer eqn:valid'; simpl; try congruence.
-        assert (delta0 = 0) by (eapply delta_zero; eauto); subst.
-        eapply Mem.valid_pointer_inject in valid'; eauto using partial_mem_inject.
-        rewrite Ptrofs.add_zero in *. rewrite Z.add_0_r in valid'. rewrite valid'. rewrite Ptrofs.add_zero; auto.
-        clear valid'.
-        destruct Mem.valid_pointer eqn:valid''; simpl; try congruence.
-        assert (delta0 = 0) by (eapply delta_zero; eauto); subst.
-        eapply Mem.valid_pointer_inject in valid''; eauto using partial_mem_inject.
-        rewrite Ptrofs.add_zero in *. rewrite Z.add_0_r in valid''. rewrite valid''. rewrite Ptrofs.add_zero; auto.
-        now rewrite orb_true_r.
-        clear valid.
-        destruct Mem.valid_pointer eqn:valid'; simpl; try congruence.
-        assert (delta0 = 0) by (eapply delta_zero; eauto); subst.
-        eapply Mem.valid_pointer_inject in valid'; eauto using partial_mem_inject.
-        rewrite Ptrofs.add_zero in *. rewrite Z.add_0_r in valid'. rewrite valid'. rewrite Ptrofs.add_zero; auto.
-        rewrite orb_true_r. simpl.
-        clear valid'.
-        destruct Mem.valid_pointer eqn:valid''; simpl; try congruence.
-        eapply Mem.valid_pointer_inject in valid''; eauto using partial_mem_inject.
-        rewrite Z.add_0_r in valid''. rewrite valid''. now auto.
-        clear valid''.
-        destruct Mem.valid_pointer eqn:valid'''; simpl; try congruence.
-        eapply Mem.valid_pointer_inject in valid'''; eauto using partial_mem_inject.
-        rewrite Z.add_0_r in valid'''. rewrite valid'''.
-        now rewrite orb_true_r.
-      + destruct eq_block; subst; simpl in *.
-        * destruct Mem.valid_pointer eqn:valid; simpl; try congruence.
-          destruct (Mem.valid_pointer m1' b0) eqn:valid'; simpl; try congruence.
-          assert (delta = 0) by (eapply delta_zero; eauto); subst.
-          assert (delta0 = 0) by (eapply delta_zero; eauto); subst.
-          eapply Mem.mi_no_overlap with (f := j) in n; [| now eapply partial_mem_inject; eauto].
-          specialize (n H H0 (Mem.perm_cur_max _ _ _ _ ((proj1 (Mem.valid_pointer_nonempty_perm _ _ _)) valid))
-                        (Mem.perm_cur_max _ _ _ _ ((proj1 (Mem.valid_pointer_nonempty_perm _ _ _)) valid')));
-            rewrite !Z.add_0_r in n.
-          destruct n; [contradiction |].
-          eapply Mem.valid_pointer_inject_val in valid; eauto using partial_mem_inject; rewrite valid; simpl; auto.
-          eapply Mem.valid_pointer_inject_val in valid'; eauto using partial_mem_inject; rewrite valid'; simpl; auto.
-          destruct op; simpl; try congruence.
-          intros. inv H2. rewrite !Ptrofs.add_zero. unfold Ptrofs.eq. destruct zeq; auto; congruence.
-          intros. inv H2. rewrite !Ptrofs.add_zero. unfold Ptrofs.eq. destruct zeq; auto; congruence.
-        * destruct Mem.valid_pointer eqn:valid; simpl; try congruence.
-          eapply Mem.valid_pointer_inject_val in valid; eauto using partial_mem_inject; rewrite valid; simpl; auto.
-          clear valid.
-          destruct Mem.valid_pointer eqn:valid'; simpl; try congruence.
-          assert (delta = 0) by (eapply delta_zero; eauto); subst.
-          assert (delta0 = 0) by (eapply delta_zero; eauto); subst.
-          eapply Mem.valid_pointer_inject in valid'; eauto using partial_mem_inject.
-          rewrite Ptrofs.add_zero in *. rewrite Z.add_0_r in valid'. rewrite valid'. auto.
+    intros.
+    destruct (side_eq (s cp) δ) as [s_cp | s_cp].
+    - exploit alloc_preserves_rel1; eauto. now simpl.
+      intros [? [? [? [? [? [? [? [? [? [? ?]]]]]]]]]].
+      eexists; eexists; eexists; repeat (split; eauto).
+    - exploit alloc_preserves_rel2; eauto. now simpl; destruct (s cp); destruct δ.
+      intros [? [? [? [? [? [? [? [? [? ?]]]]]]]]].
+      eexists; eexists; eexists; repeat (split; eauto). simpl; congruence.
   Qed.
 
 
-  Lemma cmpu_inject:
-    forall ge ge' j δ op m1 m3 v1 v1' v2 v2',
-      mem_rel s ge ge' j δ m1 m3 ->
-      Val.inject j v1 v1' ->
-      Val.inject j v2 v2' ->
-      Val.inject j (Val.cmpu (Mem.valid_pointer m1) op v1 v2)
-        (Val.cmpu (Mem.valid_pointer m3) op v1' v2').
+  Lemma free_preserves_rel:
+    forall cp j__δ j__oppδ m1 m1' m2 m3 lo hi b1 b3,
+      j__δ b1 = Some (b3, 0) -> (* we are necessarily in the δ case *)
+      mem_rel s ge1 ge3 j__δ δ m1 m3 ->
+      mem_rel s ge2 ge3 j__oppδ (opposite δ) m2 m3 ->
+      Mem.free m1 b1 lo hi cp = Some m1' ->
+      exists m3', Mem.free m3 b3 lo hi cp = Some m3' /\
+               mem_rel s ge1 ge3 j__δ δ m1' m3' /\
+               mem_rel s ge2 ge3 j__oppδ (opposite δ) m2 m3'.
   Proof.
-    intros ge ge' j δ op m1 m3 v1 v1' v2 v2' m1_m3 v1_v1' v2_v2'.
-    unfold Val.cmpu.
-    destruct (Val.cmpu_bool) eqn:eq_cmpu.
-    - eapply cmpu_bool_preserved in eq_cmpu; eauto. rewrite eq_cmpu; now eapply Cminorgenproof.val_inject_val_of_optbool.
-    - auto.
+    intros cp j__δ j__oppδ m1 m1' m2 m3 lo hi b1 b3 ptr_inj m1_m3 m2_m3 free1.
+    exploit (Mem.free_parallel_inject j__δ m1); eauto using partial_mem_inject.
+    intros [m3' [free3 m1'_m3']].
+    rewrite 2!Z.add_0_r in free3.
+    exists m3'; split; [| split]; [assumption | |].
+    { clear dependent j__oppδ.
+      constructor.
+      - intros b. apply same_dom in m1_m3.
+        specialize (m1_m3 b).
+        simpl in *. apply Mem.free_result in free1. unfold Mem.unchecked_free in free1.
+        destruct (zle hi lo); now subst.
+      - assumption.
+      - intros b b' delta.
+        intros G. exploit delta_zero; eauto.
+      - erewrite Mem.nextblock_free; eauto using Ple_trans, Ple_succ, ple_nextblock1.
+      - erewrite Mem.nextblock_free; eauto using Ple_trans, Ple_succ, ple_nextblock2.
+      - intros. exploit find_def_valid1; eauto. eapply Mem.valid_block_free_1; eauto.
+      - intros. exploit find_def_valid2; eauto. eapply Mem.valid_block_free_1; eauto.
+      - intros. intros n.
+        eapply find_def_perm1; eauto.
+        eapply Mem.perm_free_3; eauto.
+      - intros. intros n.
+        eapply find_def_perm2; eauto.
+        eapply Mem.perm_free_3; eauto.
+      - intros id ofs.
+        exploit same_high_half; eauto. }
+    { destruct m2_m3.
+      constructor; auto.
+      - eapply Mem.free_right_inject; eauto.
+        intros.
+        apply Mem.mi_inj in partial_mem_inject0.
+        eapply Mem.mi_own with (cp := (Mem.block_compartment m2 b0)) in partial_mem_inject0; eauto;
+          [| now destruct Mem.block_compartment eqn:?]; eauto.
+        specialize (same_dom0 b0).
+        assert (X: j__oppδ b0 <> None) by congruence.
+        apply same_dom0 in X. simpl in *.
+        apply same_dom in m1_m3 as G.
+        specialize (G b1).
+        assert (Y: j__δ b1 <> None) by congruence.
+        apply G in Y. simpl in *. clear G.
+        apply partial_mem_inject in m1_m3.
+        apply Mem.mi_inj in m1_m3.
+        eapply Mem.mi_own with (cp := (Mem.block_compartment m1 b1)) in m1_m3; eauto;
+          [| now destruct (Mem.block_compartment m1 b1) eqn:?]; eauto.
+        unfold Mem.can_access_block in *.
+        destruct X as [X | X]; destruct Y as [Y | Y].
+        (* easy -- Mem.can_access_block must agree with genv *)
+        admit. admit. admit. admit.
+      - erewrite Mem.nextblock_free; eauto using Ple_trans, Ple_succ, ple_nextblock1.
+      - intros. eapply Mem.valid_block_free_1; eauto.
+      - intros. intros n.
+        eapply find_def_perm4; eauto.
+        eapply Mem.perm_free_3; eauto. }
+  Admitted.
+
+  Lemma store_preserves_rel:
+    forall cp (j__δ j__oppδ: meminj) m1 m1' m2 m3 ch ofs v1 v3 b1 b3,
+      j__δ b1 = Some (b3, 0) -> (* we are necessarily in the δ case *)
+      mem_rel s ge1 ge3 j__δ δ m1 m3 ->
+      mem_rel s ge2 ge3 j__oppδ (opposite δ) m2 m3 ->
+      Val.inject j__δ v1 v3 ->
+      Mem.store ch m1 b1 ofs v1 cp = Some m1' ->
+      exists m3', Mem.store ch m3 b3 ofs v3 cp = Some m3' /\
+               mem_rel s ge1 ge3 j__δ δ m1' m3' /\
+               mem_rel s ge2 ge3 j__oppδ (opposite δ) m2 m3'.
+  Proof.
+    intros cp j__δ j__oppδ m1 m1' m2 m3 ch ofs v1 v3 b1 b3 ptr_inj m1_m3 m2_m3 val_inj store1.
+    exploit (Mem.store_mapped_inject j__δ); eauto using partial_mem_inject.
+    intros [m3' [store3 ?]].
+    rewrite Z.add_0_r in store3.
+    exists m3'; split; [| split]; [assumption | |].
+    { clear dependent j__oppδ.
+      constructor.
+      - intros b. apply same_dom in m1_m3.
+        specialize (m1_m3 b). simpl in *.
+        eapply Mem.store_block_compartment in store1. now rewrite store1.
+      - assumption.
+      - now eapply delta_zero; eauto.
+      - erewrite Mem.nextblock_store; eauto using Ple_trans, Ple_succ, ple_nextblock1.
+      - erewrite Mem.nextblock_store; eauto using Ple_trans, Ple_succ, ple_nextblock2.
+      - intros. exploit find_def_valid1; eauto. eapply Mem.store_valid_block_1; eauto.
+      - intros. exploit find_def_valid2; eauto. eapply Mem.store_valid_block_1; eauto.
+      - intros; intros n. exploit find_def_perm1; eauto.
+        eapply Mem.perm_store_2; eauto.
+      - intros; intros n. exploit find_def_perm2; eauto.
+        eapply Mem.perm_store_2; eauto.
+      - intros id ofs0.
+        exploit same_high_half; eauto. }
+    { destruct m2_m3.
+      constructor; eauto.
+      - eapply Mem.store_outside_inject; eauto.
+        intros.
+        apply Mem.mi_inj in partial_mem_inject0.
+        eapply Mem.mi_own with (cp := (Mem.block_compartment m2 b')) in partial_mem_inject0; eauto;
+          [| now destruct Mem.block_compartment eqn:?]; eauto.
+        specialize (same_dom0 b').
+        assert (X: j__oppδ b' <> None) by congruence.
+        apply same_dom0 in X. simpl in *.
+        apply same_dom in m1_m3 as G.
+        specialize (G b1).
+        assert (Y: j__δ b1 <> None) by congruence.
+        apply G in Y. simpl in *. clear G.
+        apply partial_mem_inject in m1_m3.
+        apply Mem.mi_inj in m1_m3.
+        eapply Mem.mi_own with (cp := (Mem.block_compartment m1 b1)) in m1_m3; eauto;
+          [| now destruct (Mem.block_compartment m1 b1) eqn:?]; eauto.
+        unfold Mem.can_access_block in *.
+        destruct (Mem.block_compartment m2 b'); destruct (Mem.block_compartment m1 b1); try congruence.
+        admit. admit. admit. admit.
+      - erewrite Mem.nextblock_store; eauto using Ple_trans, Ple_succ, ple_nextblock1.
+      - intros. exploit find_def_valid2; eauto. eapply Mem.store_valid_block_1; eauto.
+      - intros; intros n. exploit find_def_perm2; eauto.
+        eapply Mem.perm_store_2; eauto. }
+  Admitted.
+
+  Lemma regset_rel_inject: forall j rs1 rs3 rd v v',
+      regset_rel j rs1 rs3 ->
+      Val.inject j v v' ->
+      regset_rel j (rs1 # rd <- v) (rs3 # rd <- v').
+  Proof.
+    intros.
+    intros r.
+    destruct (Pregmap.elt_eq r rd); now try subst r; Simpl.
   Qed.
 
-  (* TODO: this is the same proof as [cmpu_bool_preserved] above, but with [Int64] substituted for [Int] *)
-  Lemma cmplu_bool_preserved: forall ge ge' j δ m1' m3 v1 v2 v1' v2' op b,
-      mem_rel s ge ge' j δ m1' m3 ->
-      Val.inject j v1 v1' ->
-      Val.inject j v2 v2' ->
-      Val.cmplu_bool (Mem.valid_pointer m1') op v1 v2 = Some b ->
-      Val.cmplu_bool (Mem.valid_pointer m3) op v1' v2' = Some b.
+  Parameter stack_rel: split -> genv -> side -> meminj -> meminj -> stack -> stack -> stack -> Prop.
+
+  Lemma inject_incr_stack_rel1:
+    forall j1 j1' j2 st1 st2 st3,
+      inject_incr j1 j1' ->
+      stack_rel s ge3 δ j1 j2 st1 st2 st3 ->
+      stack_rel s ge3 δ j1' j2 st1 st2 st3.
   Proof.
-    intros until b. intros m1_m3 inj1 inj2.
-    inv inj1; simpl; inv inj2; simpl; destruct Archi.ptr64; simpl; auto; try congruence.
-    - destruct Int64.eq; simpl; try congruence. destruct Mem.valid_pointer eqn:valid; simpl; try congruence.
-      eapply Mem.valid_pointer_inject_val in valid; eauto using partial_mem_inject; rewrite valid; simpl; auto.
-      clear valid. destruct Mem.valid_pointer eqn:valid'; simpl; try congruence.
-      assert (delta = 0) by (eapply delta_zero; eauto); subst.
-      eapply Mem.valid_pointer_inject in valid'; eauto using partial_mem_inject.
-      rewrite Ptrofs.add_zero in *. rewrite Z.add_0_r in valid'. rewrite valid'.
-      now rewrite orb_true_r.
-    - destruct Int64.eq; simpl; try congruence. destruct Mem.valid_pointer eqn:valid; simpl; try congruence.
-      eapply Mem.valid_pointer_inject_val in valid; eauto using partial_mem_inject; rewrite valid; simpl; auto.
-      clear valid. destruct Mem.valid_pointer eqn:valid'; simpl; try congruence.
-      assert (delta = 0) by (eapply delta_zero; eauto); subst.
-      eapply Mem.valid_pointer_inject in valid'; eauto using partial_mem_inject.
-      rewrite Ptrofs.add_zero in *. rewrite Z.add_0_r in valid'. rewrite valid'.
-      now rewrite orb_true_r.
-    - destruct eq_block; subst; simpl in *; try congruence.
-      + assert (b3 = b2) by congruence; subst; simpl.
-        assert (delta = delta0) by congruence; subst; simpl.
-        destruct eq_block; try congruence.
-        destruct Mem.valid_pointer eqn:valid; simpl; try congruence.
-        eapply Mem.valid_pointer_inject_val in valid; eauto using partial_mem_inject; rewrite valid; simpl; auto.
-        clear valid.
-        destruct Mem.valid_pointer eqn:valid'; simpl; try congruence.
-        assert (delta0 = 0) by (eapply delta_zero; eauto); subst.
-        eapply Mem.valid_pointer_inject in valid'; eauto using partial_mem_inject.
-        rewrite Ptrofs.add_zero in *. rewrite Z.add_0_r in valid'. rewrite valid'. rewrite Ptrofs.add_zero; auto.
-        clear valid'.
-        destruct Mem.valid_pointer eqn:valid''; simpl; try congruence.
-        assert (delta0 = 0) by (eapply delta_zero; eauto); subst.
-        eapply Mem.valid_pointer_inject in valid''; eauto using partial_mem_inject.
-        rewrite Ptrofs.add_zero in *. rewrite Z.add_0_r in valid''. rewrite valid''. rewrite Ptrofs.add_zero; auto.
-        now rewrite orb_true_r.
-        clear valid.
-        destruct Mem.valid_pointer eqn:valid'; simpl; try congruence.
-        assert (delta0 = 0) by (eapply delta_zero; eauto); subst.
-        eapply Mem.valid_pointer_inject in valid'; eauto using partial_mem_inject.
-        rewrite Ptrofs.add_zero in *. rewrite Z.add_0_r in valid'. rewrite valid'. rewrite Ptrofs.add_zero; auto.
-        rewrite orb_true_r. simpl.
-        clear valid'.
-        destruct Mem.valid_pointer eqn:valid''; simpl; try congruence.
-        eapply Mem.valid_pointer_inject in valid''; eauto using partial_mem_inject.
-        rewrite Z.add_0_r in valid''. rewrite valid''. now auto.
-        clear valid''.
-        destruct Mem.valid_pointer eqn:valid'''; simpl; try congruence.
-        eapply Mem.valid_pointer_inject in valid'''; eauto using partial_mem_inject.
-        rewrite Z.add_0_r in valid'''. rewrite valid'''.
-        now rewrite orb_true_r.
-      + destruct eq_block; subst; simpl in *.
-        * destruct Mem.valid_pointer eqn:valid; simpl; try congruence.
-          destruct (Mem.valid_pointer m1' b0) eqn:valid'; simpl; try congruence.
-          assert (delta = 0) by (eapply delta_zero; eauto); subst.
-          assert (delta0 = 0) by (eapply delta_zero; eauto); subst.
-          eapply Mem.mi_no_overlap with (f := j) in n; [| now eapply partial_mem_inject; eauto].
-          specialize (n H H0 (Mem.perm_cur_max _ _ _ _ ((proj1 (Mem.valid_pointer_nonempty_perm _ _ _)) valid))
-                        (Mem.perm_cur_max _ _ _ _ ((proj1 (Mem.valid_pointer_nonempty_perm _ _ _)) valid')));
-            rewrite !Z.add_0_r in n.
-          destruct n; [contradiction |].
-          eapply Mem.valid_pointer_inject_val in valid; eauto using partial_mem_inject; rewrite valid; simpl; auto.
-          eapply Mem.valid_pointer_inject_val in valid'; eauto using partial_mem_inject; rewrite valid'; simpl; auto.
-          destruct op; simpl; try congruence.
-          intros. inv H2. rewrite !Ptrofs.add_zero. unfold Ptrofs.eq. destruct zeq; auto; congruence.
-          intros. inv H2. rewrite !Ptrofs.add_zero. unfold Ptrofs.eq. destruct zeq; auto; congruence.
-        * destruct Mem.valid_pointer eqn:valid; simpl; try congruence.
-          eapply Mem.valid_pointer_inject_val in valid; eauto using partial_mem_inject; rewrite valid; simpl; auto.
-          clear valid.
-          destruct Mem.valid_pointer eqn:valid'; simpl; try congruence.
-          assert (delta = 0) by (eapply delta_zero; eauto); subst.
-          assert (delta0 = 0) by (eapply delta_zero; eauto); subst.
-          eapply Mem.valid_pointer_inject in valid'; eauto using partial_mem_inject.
-          rewrite Ptrofs.add_zero in *. rewrite Z.add_0_r in valid'. rewrite valid'. auto.
+  Admitted.
+  (*   intros * incr st_rel. *)
+  (*   induction st_rel. *)
+  (*   - constructor; eauto. *)
+  (*   - constructor; eauto. *)
+  (*     inv H. *)
+  (*     + econstructor; eauto. *)
+  (*     + eapply stackframe_related_opp_δ; eauto. *)
+  (* Qed. *)
+
+  Lemma inject_incr_stack_rel2:
+    forall j1 j2 j2' st1 st2 st3,
+      inject_incr j2 j2' ->
+      stack_rel s ge3 δ j1 j2 st1 st2 st3 ->
+      stack_rel s ge3 δ j1 j2' st1 st2 st3.
+  Proof.
+  Admitted.
+  (*   intros * incr st_rel. *)
+  (*   induction st_rel. *)
+  (*   - constructor; eauto. *)
+  (*   - constructor; eauto. *)
+  (*     inv H. *)
+  (*     + econstructor; eauto. *)
+  (*     + eapply stackframe_related_opp_δ; eauto. *)
+  (* Qed. *)
+
+  Lemma find_funct_ptr_preserved:
+    forall j__δ b b' fd,
+      meminj_preserves_globals s δ W1 W3 j__δ ->
+      j__δ b = Some (b', 0) ->
+      Genv.find_funct_ptr ge1 b = Some fd ->
+      exists fd',
+        Genv.find_funct_ptr ge3 b' = Some fd' /\
+          match_fundef fd fd' /\
+          (forall id : ident, Genv.find_symbol ge1 id = Some b -> kept_genv s ge1 δ id = true -> fd = fd').
+  Proof.
+    intros j b b' fd inj_pres inj_b_b' find_b_fd.
+    unfold Genv.find_funct_ptr in *.
+    destruct (Genv.find_def ge1 b) as [[fd' |] |] eqn:find_def_b; try discriminate.
+    assert (fd' = fd) by congruence; subst fd'; clear find_b_fd.
+
+    exploit defs_inject; eauto. intros [gd' [find_def_b' [_ [match_fd_gd' left_implies_eq]]]].
+    assert (exists fd', gd' = Gfun fd' /\ match_fundef fd fd') as [fd' [gd'_fd' match_fd_fd']].
+    { inv match_fd_gd'; match goal with | H: match_fundef _ _ |- _ => inv H end.
+      - eexists; split; [reflexivity | constructor].
+      - eexists; split; [reflexivity | constructor]. }
+    subst gd'.
+
+    rewrite find_def_b'. eexists; split; [| split]; auto.
+    intros; exploit left_implies_eq; eauto. congruence.
   Qed.
 
-  Lemma cmplu_inject:
-    forall ge ge' j δ op m1 m3 v1 v1' v2 v2',
-      mem_rel s ge ge' j δ m1 m3 ->
-      Val.inject j v1 v1' ->
-      Val.inject j v2 v2' ->
-      Val.inject j (Val.maketotal (Val.cmplu (Mem.valid_pointer m1) op v1 v2))
-        (Val.maketotal (Val.cmplu (Mem.valid_pointer m3) op v1' v2')).
+  Lemma find_def_preserved:
+    forall j__δ b b' gd,
+      meminj_preserves_globals s δ W1 W3 j__δ ->
+      j__δ b = Some (b', 0) ->
+      Genv.find_def ge1 b = Some gd ->
+      exists gd',
+        Genv.find_def ge3 b' = Some gd' /\
+          match_globdef gd gd' /\
+          (forall id : ident, Genv.find_symbol ge1 id = Some b -> kept_genv s ge1 δ id = true -> gd' = gd).
   Proof.
-    intros ge ge' j δ op m1 m3 v1 v1' v2 v2' m1_m3 v1_v1' v2_v2'.
-    unfold Val.cmplu.
-    destruct (Val.cmplu_bool) eqn:eq_cmplu.
-    - eapply cmplu_bool_preserved in eq_cmplu; eauto. rewrite eq_cmplu.
-      simpl. now eapply Cop.val_inject_of_bool.
-    - auto.
+    intros j__δ b b' gd inj_pres inj_b_b' find_b_gd. exploit defs_inject; eauto. intros [gd' [find_def_b' [_ [match_fd_gd' left_implies_eq]]]].
+    eauto.
   Qed.
 
-  Hint Resolve cmpu_inject cmplu_inject : solve_inject.
-  Hint Resolve Cop.val_inject_of_bool: solve_inject.
+  Lemma def_on_addressable_init:
+    match_prog s δ W1 W3 ->
+    def_on_addressable s ge1 (init_meminj W1 W3) δ.
+  Proof.
+    unfold def_on_addressable.
+    intros match_W1_W3. intros.
+    unfold init_meminj.
+    apply Genv.find_invert_symbol in H; rewrite H.
+    apply Genv.invert_find_symbol in H.
+    exploit transform_find_symbol_1; eauto.
+    intros (? & ->). eauto.
+  Qed.
+
+  Lemma agrees_with_init_meminj_find_def_preserved:
+    forall j b b' delta gd,
+      match_prog s δ W1 W3 ->
+      agrees_with j (init_meminj W1 W3) ->
+      j b = Some (b', delta) ->
+      Genv.find_def ge1 b = Some gd ->
+      exists gd',
+        Genv.find_def ge3 b' = Some gd' /\
+          match_globdef gd gd' /\
+          (forall id : ident, Genv.find_symbol ge1 id = Some b -> kept_genv s ge1 δ id = true -> gd' = gd).
+    Proof.
+      intros j b b' delta gd match_W1_W3 agr j_b find_b.
+      exploit init_meminj_preserves_globals; eauto. intros inj_pres.
+      eapply find_def_preserved; eauto.
+      assert (exists b', init_meminj W1 W3 b = Some (b', 0)) as [b'' init_meminj_b].
+      { unfold init_meminj.
+        exploit Genv.find_def_find_symbol_inversion; eauto.
+        intros (id & A). apply Genv.find_invert_symbol in A as B. rewrite B.
+        destruct (kept_prog s W1 δ id) eqn:?.
+        - exploit match_prog_def; eauto.
+          assert (C: (prog_defmap W1) ! id = Some gd).
+          { apply Genv.find_def_symbol; eauto. }
+          rewrite C. intros D.
+          apply Genv.find_def_symbol in D as [b'' [D E]]; eauto.
+          rewrite D. eauto.
+        - exploit match_prog_notdef; eauto.
+          assert (C: (prog_defmap W1) ! id = Some gd).
+          { apply Genv.find_def_symbol; eauto. }
+          rewrite C. intros D.
+          inversion D as [| ? ? matchgd u E]; subst. symmetry in E.
+          apply Genv.find_def_symbol in E as [b'' [E F]]; eauto.
+          rewrite E. eauto. }
+      exploit agr; eauto. now intros []; congruence.
+    Qed.
+
+  Lemma find_comp_of_block_preserved:
+    forall j__δ b b' delta
+      (inj_pres: meminj_preserves_globals s δ W1 W3 j__δ)
+      (delta_zero: mem_delta_zero j__δ),
+      j__δ b = Some (b', delta) ->
+      Genv.find_comp_of_block ge1 b = Genv.find_comp_of_block ge3 b'.
+  Proof.
+    intros j b b' delta inj_pres delta_zero j_b.
+    exploit delta_zero; eauto; intros ->.
+    unfold Genv.find_comp_of_block.
+    destruct (Genv.find_def _ b) as [gd |] eqn:?.
+    - exploit find_def_preserved; eauto.
+      intros (gd' & -> & H & ?).
+      destruct H as [? ? H | ? ? H]; now inv H.
+    - destruct (Genv.find_def _ b') as [gd |] eqn:?; [| reflexivity].
+      exploit defs_rev_inject; eauto. intros (gd' & ? & ?); congruence.
+  Qed.
+
+
+  Lemma agrees_with_init_meminj_find_comp_of_block_preserved:
+    forall j b b' delta cp,
+      match_prog s δ W1 W3 ->
+      agrees_with j (init_meminj W1 W3) ->
+      j b = Some (b', delta) ->
+      Genv.find_comp_of_block ge1 b = Some cp ->
+      Genv.find_comp_of_block ge3 b' = Some cp.
+  Proof.
+    intros j b b' delta cp match_W1_W3 agr j_b comp_b.
+    unfold Genv.find_comp_of_block in *.
+    destruct (Genv.find_def _ b) as [gd |] eqn:?.
+    - exploit agrees_with_init_meminj_find_def_preserved; eauto.
+      intros (gd' & -> & H & ?).
+      destruct H as [? ? H | ? ? H]; now inv H.
+    - congruence.
+  Qed.
+
+  Lemma find_comp_preserved:
+    forall j__δ v v'
+      (inj_pres: meminj_preserves_globals s δ W1 W3 j__δ)
+      (delta_zero: mem_delta_zero j__δ),
+      v <> Vundef ->
+      Val.inject j__δ v v' ->
+      Genv.find_comp ge1 v = Genv.find_comp ge3 v'.
+  Proof.
+    intros j v v' inj_pres delta_zero nundef H.
+    inv H; simpl; auto; try congruence.
+    exploit find_comp_of_block_preserved; eauto.
+  Qed.
+
+  Lemma agrees_with_init_meminj_find_comp_preserved:
+    forall j v v' cp,
+      match_prog s δ W1 W3 ->
+      agrees_with j (init_meminj W1 W3) ->
+      v <> Vundef ->
+      Val.inject j v v' ->
+      Genv.find_comp ge1 v = Some cp ->
+      Genv.find_comp ge3 v' = Some cp.
+  Proof.
+    intros j v v' cp match_W1_W3 agr j_v v_not_undef comp_v.
+    inv v_not_undef; simpl; auto; try congruence.
+    eapply agrees_with_init_meminj_find_comp_of_block_preserved; eauto.
+  Qed.
+
+End Lemmas.
+
+Section Theorems.
+
+  Context (s: split) (W1 W2 W3: Asm.program) (δ: side).
+
+  Hypothesis match_W1_W3: match_prog s δ W1 W3.
+  Hypothesis match_W2_W3: match_prog s (opposite δ) W2 W3.
+
+  Notation cp_main := (comp_of_main W1).
+
+  Hypothesis norepet1: list_norepet (prog_defs_names W1).
+  Hypothesis norepet2: list_norepet (prog_defs_names W2).
+
+  Notation ge1 := (Genv.globalenv W1).
+  Notation ge2 := (Genv.globalenv W2).
+  Notation ge3 := (Genv.globalenv W3).
 
   Local Opaque Val.add Val.addl Val.sub Val.subl
     Val.mul Val.mulhs Val.mulhu Val.mull Val.mullhs Val.mullhu
@@ -493,1018 +1606,73 @@ Section Simulation.
     Val.addfs Val.addf Val.subfs Val.subf Val.mulfs Val.mulf
     Val.divfs Val.divf.
 
-  Locate symbols_inject.
-  Lemma alloc_preserves_rel_left1:
-    forall cp j__left j__right m1 m1' m2 m3 lo hi b1 rs1 rs3,
-      s |= cp ∈ Left ->
-      mem_rel s ge1 ge3 j__left Left m1 m3 ->
-      mem_rel s ge2 ge3 j__right Right m2 m3 ->
-      regset_rel j__left rs1 rs3 ->
-      Mem.alloc m1 cp lo hi = (m1', b1) ->
-      exists j__left' m3' b3, Mem.alloc m3 cp lo hi = (m3', b3) /\
-                     mem_rel s ge1 ge3 j__left' Left m1' m3' /\
-                     mem_rel s ge2 ge3 j__right Right m2 m3' /\
-                     regset_rel j__left' rs1 rs3 /\
-                     j__left' b1 = Some (b3, 0) /\
-                     inject_incr j__left j__left'.
-  Proof.
-    intros cp j__left j__right m1 m1' m2 m3 lo hi b1 rs1 rs3 side_cp m1_m3 m2_m3 rs1_rs3 alloc1.
-    exploit (Mem.alloc_parallel_inject j__left m1); eauto using partial_mem_inject, Z.le_refl.
-    intros [j' [m3' [b3 [? [? [? [? rewr]]]]]]].
-    exists j', m3', b3.
-    split; [| split; [| split; [| split; [| split]]]];
-      [assumption | | | intros ?; eauto using val_inject_incr | assumption | assumption].
-    { clear dependent j__right.
-      constructor.
-      - intros b. destruct (Pos.eq_dec b b1); subst.
-        + split; [| congruence].
-          intros _. apply Mem.owned_new_block in alloc1. simpl in alloc1. simpl; now rewrite alloc1.
-        + rewrite (rewr _ n).
-          eapply same_dom in m1_m3. specialize (m1_m3 b).
-          eapply Mem.alloc_block_compartment with (b' := b) in alloc1.
-          simpl. rewrite alloc1. rewrite peq_false; eauto.
-      - assumption.
-      - intros b b' delta.
-        destruct (Pos.eq_dec b b1); subst.
-        + congruence.
-        + rewrite (rewr _ n).
-          intros G. exploit delta_zero; eauto.
-      - exploit symb_inj; eauto.
-        intros (A & B & C & D).
-        split; [| split; [| split]].
-        + intros. exploit A; eauto.
-        + intros. exploit B; eauto. rewrite <- rewr. eauto.
-          exploit (Mem.alloc_result m1 cp lo hi m1' b1) ; eauto. intros ->.
-          exploit Senv.find_symbol_below; eauto.
-          eapply ple_nextblock1 in m1_m3. intros ? ?. subst.
-          exploit Plt_Ple_trans; eauto. now apply Plt_strict.
-            (* exploit C; eauto. *)
-        + intros. exploit C; eauto. intros ?.
-          destruct H5 as [b2 ?]. exists b2.
-          rewrite rewr; eauto.
-          exploit (Mem.alloc_result m1 cp lo hi m1' b1) ; eauto. intros ->.
-          exploit Senv.find_symbol_below; eauto.
-          eapply ple_nextblock1 in m1_m3. intros ? ?. subst.
-          exploit Plt_Ple_trans; eauto. now apply Plt_strict.
-        + intros. destruct (Pos.eq_dec b0 b1); subst.
-          * assert (Senv.block_is_volatile ge1 b1 = false).
-            { destruct (Senv.block_is_volatile ge1 b1) eqn:?; auto.
-              exfalso.
-              exploit (Mem.alloc_result m1 cp lo hi m1' b1) ; eauto. intros ->.
-              exploit Senv.block_is_volatile_below; eauto.
-              eapply ple_nextblock1 in m1_m3. intros ?.
-              exploit Plt_Ple_trans; eauto. intros ?. now eapply Plt_strict; eauto. }
-            assert (b3 = b2) by congruence. subst b2.
-            assert (Senv.block_is_volatile ge3 b3 = false).
-            { destruct (Senv.block_is_volatile ge3 b3) eqn:?; auto.
-              exfalso.
-              exploit (Mem.alloc_result m3 cp lo hi m3' b3) ; eauto. intros ->.
-              exploit Senv.block_is_volatile_below; eauto.
-              eapply ple_nextblock2 in m1_m3. intros ?.
-              exploit Plt_Ple_trans; eauto. intros ?. now eapply Plt_strict; eauto. }
-            now congruence.
-          * exploit D; eauto.
-            rewrite <- rewr; eauto.
-      - erewrite Mem.nextblock_alloc; eauto using Ple_trans, Ple_succ, ple_nextblock1.
-      - erewrite Mem.nextblock_alloc; eauto using Ple_trans, Ple_succ, ple_nextblock2.
-      - intros. exploit funct_preserved1; eauto.
-      - intros. exploit funct_preserved2; eauto.
-        rewrite <- rewr; eauto.
-        intros ?. subst. assert (b3 = b2) by congruence; subst b3.
-        apply Genv.find_funct_ptr_iff in H3.
-        apply Genv.genv_defs_range in H3. apply Mem.alloc_result in H. subst.
-        apply ple_nextblock2 in m1_m3. simpl in *.
-        eapply Plt_strict. eapply Plt_Ple_trans; eauto.
-      - intros. exploit var_info_valid; eauto. eapply Mem.valid_block_alloc. eauto.
-      - intros id ofs.
-        exploit same_high_half; eauto. }
-    { clear dependent j__left.
-      destruct m2_m3.
-      constructor; eauto.
-      - eapply Mem.alloc_right_inject; eauto using partial_mem_inject.
-      - erewrite Mem.nextblock_alloc; eauto using Ple_trans, Ple_succ, ple_nextblock1.
-      - intros. eapply Mem.valid_block_alloc; eauto. }
-  Qed.
+  Local Arguments comp_of /.
 
-  Lemma alloc_preserves_rel_left2:
-    forall cp j__left j__right m1 m1' m2 m3 lo hi b1 rs1 rs3,
-      s |= cp ∈ Right ->
-      mem_rel s ge1 ge3 j__left Left m1 m3 ->
-      mem_rel s ge2 ge3 j__right Right m2 m3 ->
-      regset_rel j__left rs1 rs3 ->
-      Mem.alloc m1 cp lo hi = (m1', b1) ->
-      exists j__left' m3' b3, Mem.alloc m3 cp lo hi = (m3', b3) /\
-                         mem_rel s ge1 ge3 j__left' Left m1' m3' /\
-                         mem_rel s ge2 ge3 j__right Right m2 m3' /\
-                         regset_rel j__left' rs1 rs3 /\
-                         inject_incr j__left j__left'.
-  Proof.
-    intros cp j__left j__right m1 m1' m2 m3 lo hi b1 rs1 rs3 side_cp m1_m3 m2_m3 rs1_rs3 alloc1.
-    exploit (Mem.alloc_parallel_inject j__left m1); eauto using partial_mem_inject, Z.le_refl.
-    intros [_ [m3' [b3 [alloc3 [_ [_ [_ _]]]]]]].
-    exploit (Mem.alloc_left_unmapped_inject j__left m1); eauto using partial_mem_inject.
-    intros [j' [inj [incr [isnone diff]]]].
-    exploit Mem.alloc_right_inject; eauto. intros inj'.
-    exists j', m3', b3. split; [| split; [| split; [| split]]];
-      [assumption |  | | intros ?; eauto using val_inject_incr | assumption].
-    { clear dependent j__right.
-      constructor; auto.
-      - intros b. destruct (Pos.eq_dec b b1); subst.
-        + split; [congruence |].
-          intros ?. apply Mem.owned_new_block in alloc1. simpl in *. rewrite alloc1 in H.
-          congruence.
-        + rewrite (diff _ n).
-          eapply same_dom in m1_m3. specialize (m1_m3 b).
-          eapply Mem.alloc_block_compartment with (b' := b) in alloc1.
-          simpl. rewrite alloc1. rewrite peq_false; eauto.
-    (* - auto. *)
-    - intros b b' delta.
-      destruct (Pos.eq_dec b b1); subst.
-      + congruence.
-      + rewrite (diff _ n).
-        intros G. exploit delta_zero; eauto.
-      - exploit symb_inj; eauto.
-        intros (A & B & C & D).
-        split; [| split; [| split]].
-        + intros. exploit A; eauto.
-        + intros. exploit B; eauto. rewrite <- diff. eauto.
-          exploit (Mem.alloc_result m1 cp lo hi m1' b1) ; eauto. intros ->.
-          exploit Senv.find_symbol_below; eauto.
-          eapply ple_nextblock1 in m1_m3. intros ? ?. subst.
-          exploit Plt_Ple_trans; eauto. now apply Plt_strict.
-            (* exploit C; eauto. *)
-        + intros. exploit C; eauto. intros ?.
-          destruct H1 as [b2 ?]. exists b2.
-          rewrite diff; eauto.
-          exploit (Mem.alloc_result m1 cp lo hi m1' b1) ; eauto. intros ->.
-          exploit Senv.find_symbol_below; eauto.
-          eapply ple_nextblock1 in m1_m3. intros ? ?. subst.
-          exploit Plt_Ple_trans; eauto. now apply Plt_strict.
-        + intros. destruct (Pos.eq_dec b0 b1); subst.
-          * assert (Senv.block_is_volatile ge1 b1 = false).
-            { destruct (Senv.block_is_volatile ge1 b1) eqn:?; auto.
-              exfalso.
-              exploit (Mem.alloc_result m1 cp lo hi m1' b1) ; eauto. intros ->.
-              exploit Senv.block_is_volatile_below; eauto.
-              eapply ple_nextblock1 in m1_m3. intros ?.
-              exploit Plt_Ple_trans; eauto. intros ?. now eapply Plt_strict; eauto. }
-            assert (b3 = b2) by congruence. subst b2.
-            assert (Senv.block_is_volatile ge3 b3 = false).
-            { destruct (Senv.block_is_volatile ge3 b3) eqn:?; auto.
-              exfalso.
-              exploit (Mem.alloc_result m3 cp lo hi m3' b3) ; eauto. intros ->.
-              exploit Senv.block_is_volatile_below; eauto.
-              eapply ple_nextblock2 in m1_m3. intros ?.
-              exploit Plt_Ple_trans; eauto. intros ?. now eapply Plt_strict; eauto. }
-            now congruence.
-          * exploit D; eauto.
-            rewrite <- diff; eauto.
-    - erewrite Mem.nextblock_alloc; eauto using Ple_trans, Ple_succ, ple_nextblock1.
-    - erewrite Mem.nextblock_alloc; eauto using Ple_trans, Ple_succ, ple_nextblock2.
-    - intros. exploit funct_preserved1; eauto.
-    - intros. exploit funct_preserved2; eauto.
-      rewrite <- diff; eauto.
-      intros ?. subst. assert (b3 = b2) by congruence; subst b3.
-      apply Genv.find_funct_ptr_iff in H.
-      apply Genv.genv_defs_range in H. apply Mem.alloc_result in alloc3. subst.
-      apply ple_nextblock2 in m1_m3. simpl in *.
-      eapply Plt_strict. eapply Plt_Ple_trans; eauto.
-    - intros. exploit var_info_valid; eauto. eapply Mem.valid_block_alloc. eauto.
-    - intros id ofs.
-      exploit same_high_half; eauto.
-    }
-    { clear dependent j__left.
-      destruct m2_m3.
-      constructor; eauto.
-      - eapply Mem.alloc_right_inject; eauto using partial_mem_inject.
-      - erewrite Mem.nextblock_alloc; eauto using Ple_trans, Ple_succ, ple_nextblock1.
-      - intros. eapply Mem.valid_block_alloc; eauto. }
-  Qed.
-
-  Lemma alloc_preserves_rel_left:
-    forall cp j__left j__right m1 m1' m2 m3 lo hi b1 rs1 rs3,
-      mem_rel s ge1 ge3 j__left Left m1 m3 ->
-      mem_rel s ge2 ge3 j__right Right m2 m3 ->
-      regset_rel j__left rs1 rs3 ->
-      Mem.alloc m1 cp lo hi = (m1', b1) ->
-      exists j__left' m3' b3, Mem.alloc m3 cp lo hi = (m3', b3) /\
-                         mem_rel s ge1 ge3 j__left' Left m1' m3' /\
-                         mem_rel s ge2 ge3 j__right Right m2 m3' /\
-                         regset_rel j__left' rs1 rs3 /\
-                         (s |= cp ∈ Left -> j__left' b1 = Some (b3, 0)) /\
-                         inject_incr j__left j__left'.
-  Proof.
-    intros.
-    destruct (s cp) eqn:s_cp.
-    - exploit alloc_preserves_rel_left1; eauto. now simpl.
-      intros [? [? [? [? [? [? [? [? ?]]]]]]]].
-      eexists; eexists; eexists; repeat (split; eauto).
-    - exploit alloc_preserves_rel_left2; eauto. now simpl.
-      intros [? [? [? [? [? [? [? ?]]]]]]].
-      eexists; eexists; eexists; repeat (split; eauto). simpl; congruence.
-  Qed.
-
-  Lemma free_preserves_rel_left:
-    forall cp j__left j__right m1 m1' m2 m3 lo hi b1 b3,
-      j__left b1 = Some (b3, 0) -> (* we are necessarily in the Left case *)
-      mem_rel s ge1 ge3 j__left Left m1 m3 ->
-      mem_rel s ge2 ge3 j__right Right m2 m3 ->
-      Mem.free m1 b1 lo hi cp = Some m1' ->
-      exists m3', Mem.free m3 b3 lo hi cp = Some m3' /\
-               mem_rel s ge1 ge3 j__left Left m1' m3' /\
-               mem_rel s ge2 ge3 j__right Right m2 m3'.
-  Proof.
-    intros cp j__left j__right m1 m1' m2 m3 lo hi b1 b3 ptr_inj m1_m3 m2_m3 free1.
-    exploit (Mem.free_parallel_inject j__left m1); eauto using partial_mem_inject.
-    intros [m3' [free3 m1'_m3']].
-    rewrite 2!Z.add_0_r in free3.
-    exists m3'; split; [| split]; [assumption | |].
-    { clear dependent j__right.
-      constructor.
-      - intros b. apply same_dom in m1_m3.
-        specialize (m1_m3 b).
-        simpl in *. apply Mem.free_result in free1. unfold Mem.unchecked_free in free1.
-        destruct (zle hi lo); now subst.
-      - assumption.
-      - intros b b' delta.
-        intros G. exploit delta_zero; eauto.
-      - exploit symb_inj; eauto.
-      - erewrite Mem.nextblock_free; eauto using Ple_trans, Ple_succ, ple_nextblock1.
-      - erewrite Mem.nextblock_free; eauto using Ple_trans, Ple_succ, ple_nextblock2.
-      - intros. exploit funct_preserved1; eauto.
-      - intros. exploit funct_preserved2; eauto.
-      - intros. exploit var_info_valid; eauto. eapply Mem.valid_block_free_1; eauto.
-      - intros id ofs.
-        exploit same_high_half; eauto. }
-    { (* clear dependent j__left. *)
-      destruct m2_m3.
-      constructor; auto.
-      - eapply Mem.free_right_inject; eauto.
-        intros.
-        apply Mem.mi_inj in partial_mem_inject0.
-        eapply Mem.mi_own with (cp := (Mem.block_compartment m2 b0)) in partial_mem_inject0; eauto;
-          [| now destruct Mem.block_compartment eqn:?]; eauto.
-        specialize (same_dom0 b0).
-        assert (X: j__right b0 <> None) by congruence.
-        apply same_dom0 in X. simpl in *.
-        apply same_dom in m1_m3 as G.
-        specialize (G b1).
-        assert (Y: j__left b1 <> None) by congruence.
-        apply G in Y. simpl in *. clear G.
-        apply partial_mem_inject in m1_m3.
-        apply Mem.mi_inj in m1_m3.
-        eapply Mem.mi_own with (cp := (Mem.block_compartment m1 b1)) in m1_m3; eauto;
-          [| now destruct (Mem.block_compartment m1 b1) eqn:?]; eauto.
-        unfold Mem.can_access_block in *.
-        destruct (Mem.block_compartment m2 b0); destruct (Mem.block_compartment m1 b1); try congruence.
-      - erewrite Mem.nextblock_free; eauto using Ple_trans, Ple_succ, ple_nextblock1.
-      - intros. eapply Mem.valid_block_free_1; eauto. }
-  (* Qed. *)
-  Admitted.
-
-  Lemma store_preserves_rel_left:
-    forall cp j__left j__right m1 m1' m2 m3 ch ofs v1 v3 b1 b3,
-      j__left b1 = Some (b3, 0) -> (* we are necessarily in the δ case *)
-      mem_rel s ge1 ge3 j__left Left m1 m3 ->
-      mem_rel s ge2 ge3 j__right Right m2 m3 ->
-      Val.inject j__left v1 v3 ->
-      Mem.store ch m1 b1 ofs v1 cp = Some m1' ->
-      exists m3', Mem.store ch m3 b3 ofs v3 cp = Some m3' /\
-               mem_rel s ge1 ge3 j__left Left m1' m3' /\
-               mem_rel s ge2 ge3 j__right Right m2 m3'.
-  Proof.
-    intros cp j__left j__right m1 m1' m2 m3 ch ofs v1 v3 b1 b3 ptr_inj m1_m3 m2_m3 val_inj store1.
-    exploit (Mem.store_mapped_inject j__left); eauto using partial_mem_inject.
-    intros [m3' [store3 ?]].
-    rewrite Z.add_0_r in store3.
-    exists m3'; split; [| split]; [assumption | |].
-    { clear dependent j__right.
-      constructor.
-      - intros b. apply same_dom in m1_m3.
-        specialize (m1_m3 b). simpl in *.
-        eapply Mem.store_block_compartment in store1. now rewrite store1.
-      - assumption.
-      - now eapply delta_zero; eauto.
-      - exploit symb_inj; eauto.
-      - erewrite Mem.nextblock_store; eauto using Ple_trans, Ple_succ, ple_nextblock1.
-      - erewrite Mem.nextblock_store; eauto using Ple_trans, Ple_succ, ple_nextblock2.
-      - intros. exploit funct_preserved1; eauto.
-      - intros. exploit funct_preserved2; eauto.
-      - intros. exploit var_info_valid; eauto. eapply Mem.store_valid_block_1; eauto.
-      - intros id ofs0.
-        exploit same_high_half; eauto. }
-    { destruct m2_m3.
-      constructor; eauto.
-      (* - Mem.store_outside_inject *)
-      - eapply Mem.store_outside_inject; eauto.
-        intros.
-        apply Mem.mi_inj in partial_mem_inject0.
-        eapply Mem.mi_own with (cp := (Mem.block_compartment m2 b')) in partial_mem_inject0; eauto;
-          [| now destruct Mem.block_compartment eqn:?]; eauto.
-        specialize (same_dom0 b').
-        assert (X: j__right b' <> None) by congruence.
-        apply same_dom0 in X. simpl in *.
-        apply same_dom in m1_m3 as G.
-        specialize (G b1).
-        assert (Y: j__left b1 <> None) by congruence.
-        apply G in Y. simpl in *. clear G.
-        apply partial_mem_inject in m1_m3.
-        apply Mem.mi_inj in m1_m3.
-        eapply Mem.mi_own with (cp := (Mem.block_compartment m1 b1)) in m1_m3; eauto;
-          [| now destruct (Mem.block_compartment m1 b1) eqn:?]; eauto.
-        unfold Mem.can_access_block in *.
-        destruct (Mem.block_compartment m2 b'); destruct (Mem.block_compartment m1 b1); try congruence.
-      - erewrite Mem.nextblock_store; eauto using Ple_trans, Ple_succ, ple_nextblock1.
-      - intros. exploit var_info_valid; eauto. eapply Mem.store_valid_block_1; eauto. }
-  Qed.
-
-  Lemma regset_rel_inject: forall j rs1 rs3 rd v v',
-      regset_rel j rs1 rs3 ->
-      Val.inject j v v' ->
-      regset_rel j (rs1 # rd <- v) (rs3 # rd <- v').
-  Proof.
-    intros.
-    intros r.
-    destruct (Pregmap.elt_eq r rd); now try subst r; Simpl.
-  Qed.
-
-  Lemma inject_incr_stack_rel1:
-    forall δ j1 j1' j2 st st',
-      inject_incr j1 j1' ->
-      stack_rel s j1 j2 δ st st' ->
-      stack_rel s j1' j2 δ st st'.
-  Proof.
-    intros * incr st_rel.
-    induction st_rel.
-    - constructor; eauto.
-    - constructor; eauto.
-      inv H2. constructor; eauto.
-    - constructor; eauto.
-  Qed.
-
-  Lemma inject_incr_stack_rel2:
-    forall δ j1 j2 j2' st st',
-      inject_incr j2 j2' ->
-      stack_rel s j1 j2 δ st st' ->
-      stack_rel s j1 j2' δ st st'.
-  Proof.
-    intros * incr st_rel.
-    induction st_rel.
-    - constructor; eauto.
-    - constructor; eauto.
-    - constructor; eauto.
-      inv H2. constructor; eauto.
-  Qed.
-
-  Ltac Simplif_all :=
-    ((rewrite Asmgenproof0.nextinstr_inv in * by eauto with asmgen)
-     || (rewrite Asmgenproof0.nextinstr_inv1 in * by eauto with asmgen)
-     || (rewrite Pregmap.gss in *)
-     || (rewrite Asmgenproof0.nextinstr_pc in *)
-     || (rewrite Pregmap.gso in * by eauto with asmgen)); auto with asmgen.
-
-  Ltac Simpl_all := repeat Simplif_all.
-
-  Ltac eexists_and_split :=
-    fun k =>
-      match goal with
-      | m1_m3: mem_rel _ _ _ ?j _ ?m1 ?m3,
-          rs1_rs3: regset_rel ?j ?rs1 ?rs3 |- _ =>
-          exists j; eexists; eexists; split; [| split; [| split; [| split]]]; eauto;
-          k j rs1 rs3 rs1_rs3 m1 m3 m1_m3
-      end.
-
-  Ltac simpl_before_exists :=
-    repeat (Simpl_all;
-            match goal with
-            (* Goto *)
-            | _: goto_label _ _ ?rs _ = Next _ _ |- _ =>
-                unfold goto_label in *; destruct label_pos; try congruence
-            | _: eval_branch _ _ ?rs _ _ = Next _ _ |- _ =>
-                unfold eval_branch in *; simpl in *
-            | _: exec_load _ _ _ _ _ _ _ _ _ = Next _ _ |- _ =>
-                unfold exec_load in *; simpl in *
-            | _: exec_store _ _ _ _ _ _ _ _ = Next _ _ |- _ =>
-                unfold exec_store in *; simpl in *
-            | _: context [Val.cmp_bool] |- _ =>
-                unfold Val.cmp_bool in *; simpl in *
-            | _: context [Val.cmpl_bool] |- _ =>
-                unfold Val.cmpl_bool in *; simpl in *
-            | _: context [eval_offset _ ?ofs] |- _ =>
-                destruct ofs eqn:?; subst; simpl in *
-
-            | _: context [low_half] |- _ =>
-                unfold low_half in *; simpl in *
-                (* rewrite same_low_half1 in * *)
-
-
-            | H: Mem.alloc ?m1 ?cp ?lo1 ?hi1 = (?m1', ?b1),
-              m1_m3: mem_rel _ _ _ ?j__left Left ?m1 ?m3,
-              m2_m3: mem_rel _ _ _ ?j__right Right ?m2 ?m3,
-              rs1_rs3: regset_rel _ _ _ |- _ =>
-                (* idtac "alloc case"; *)
-                let j__left' := fresh "j__left" in
-                let m3' := fresh "m3" in
-                let b3 := fresh "b3" in
-                let alloc3 := fresh "alloc3" in
-                let m1'_m3' := fresh "m1'_m3'" in
-                let m2_m3' := fresh "m2_m3'" in
-                let proj := fresh "proj" in
-                let incr := fresh "incr" in
-                apply (alloc_preserves_rel_left _ _ _ _ _ _ _ _ _ _ _ _ m1_m3 m2_m3 rs1_rs3) in H as
-                    [j__left' [m3' [b3 [alloc3 [m1'_m3' [m2_m3' [? [proj incr]]]]]]]];
-                (* idtac "done with alloc"; *)
-                clear m1_m3 rs1_rs3 m2_m3
-            | H: s ?cp = ?δ -> _,
-              side_cp: s ?cp = ?δ |- _ =>
-                specialize (H side_cp)
-
-            | H: Mem.store ?ch ?m1 ?b1 ?ofs (?rs1 ?r) ?cp = Some ?m1',
-              m1_m3: mem_rel _ _ _ ?j__left Left ?m1 ?m3,
-              m2_m3: mem_rel _ _ _ ?j__right Right ?m2 ?m3,
-              ptr_inj: ?j__left ?b1 = Some (?b3, 0),
-              rs1_rs3: regset_rel ?j__left ?rs1 ?rs3 |- _ =>
-                (* idtac "store case"; *)
-                let m3' := fresh "m3" in
-                apply (store_preserves_rel_left _ _ _ _ _ _ _ _ _ _ _ _ _ ptr_inj m1_m3 m2_m3 (rs1_rs3 r)) in H as
-                    [m3' [? [? ?]]];
-                (* idtac "done with store"; *)
-                clear m1_m3 m2_m3
-
-            | H: Mem.free ?m1 ?b1 ?lo ?hi ?cp = Some ?m1',
-              m1_m3: mem_rel _ _ _ ?j__left Left ?m1 ?m3,
-              m2_m3: mem_rel _ _ _ ?j__right Right ?m2 ?m3,
-              ptr_inj: ?j__left ?b1 = Some (?b3, 0) |- _ =>
-                (* rs1_rs3: regset_rel ?j ?rs1 ?rs3 |- _ => *)
-                (* idtac "free case"; *)
-                let m3' := fresh "m3" in
-                apply (free_preserves_rel_left _ _ _ _ _ _ _ _ _ _ _ ptr_inj m1_m3 m2_m3) in H as
-                    [m3' [? [? ?]]];
-                (* idtac "done with free"; *)
-                clear m1_m3
-
-            | H: Mem.load ?ch ?m1 ?b1 ?ofs ?cp = Some ?v1,
-                m1_m3: mem_rel _ _ _ ?j _ ?m1 ?m3,
-                  ptr_inj: ?j ?b1 = Some (?b3, 0) |- _ =>
-                idtac "load case";
-                let v3 := fresh "v3" in
-                let load3 := fresh "load3" in
-                destruct (Mem.load_inject _ _ _ _ _ _ _ _ _ _ (partial_mem_inject _ _ _ _ _ _ _ m1_m3) H ptr_inj) as
-                  [v3 [load3 ?]];
-                rewrite Z.add_0_r in load3;
-                idtac "done with load";
-                clear H
-
-            | H: Val.cmpu_bool (Mem.valid_pointer ?m1) ?op (?rs1 ?r) (?rs1 ?r') = Some ?b,
-                m1_m3: mem_rel _ _ _ ?j _ ?m1 ?m3,
-                rs1_rs3: regset_rel ?j ?rs1 ?rs3 |- _ =>
-                (* idtac "Val.cmpu_bool case 0"; *)
-                eapply cmpu_bool_preserved with (m3 := m3) in H; eauto using rs1_rs3;
-                try rewrite H in *;
-                (* idtac "done with Val.cmpu_bool 0"; *)
-                try congruence
-
-            | H: Val.cmpu_bool (Mem.valid_pointer ?m1) ?op (Vint ?x) (?rs1 ?r') = Some ?b,
-                m1_m3: mem_rel _ _ _ ?j _ ?m1 ?m3,
-                rs1_rs3: regset_rel ?j ?rs1 ?rs3 |- _ =>
-                (* idtac "Val.cmpu_bool case 1"; *)
-                eapply cmpu_bool_preserved with (m3 := m3) (v1' := Vint x) in H; eauto using rs1_rs3;
-                try rewrite H in *;
-                (* idtac "done with Val.cmpu_bool 1"; *)
-                try congruence
-
-            | H: Val.cmpu_bool (Mem.valid_pointer ?m1) ?op (?rs1 ?r) (Vint ?x) = Some ?b,
-                m1_m3: mem_rel _ _ _ ?j _ ?m1 ?m3,
-                rs1_rs3: regset_rel ?j ?rs1 ?rs3 |- _ =>
-                (* idtac "Val.cmpu_bool case 2"; *)
-                eapply cmpu_bool_preserved with (m3 := m3) (v2' := Vint x) in H; eauto using rs1_rs3;
-                try rewrite H in *;
-                (* idtac "done with Val.cmpu_bool 2"; *)
-                try congruence
-
-            | H: Val.cmpu_bool (Mem.valid_pointer ?m1) ?op (Vint ?x) (Vint ?y) = Some ?b,
-                m1_m3: mem_rel _ _ _ ?j _ ?m1 ?m3,
-                rs1_rs3: regset_rel ?j ?rs1 ?rs3 |- _ =>
-                (* idtac "Val.cmpu_bool case 3"; *)
-                eapply cmpu_bool_preserved with (m3 := m3) (v1' := Vint x) (v2' := Vint y) in H; eauto using rs1_rs3;
-                try rewrite H in *;
-                (* idtac "done with Val.cmpu_bool 3"; *)
-                try congruence
-
-            | H: Val.cmplu_bool (Mem.valid_pointer ?m1) ?op (?rs1 ?r) (?rs1 ?r') = Some ?b,
-                m1_m3: mem_rel _ _ _ ?j _ ?m1 ?m3,
-                rs1_rs3: regset_rel ?j ?rs1 ?rs3 |- _ =>
-                (* idtac "Val.cmplu_bool case 0"; *)
-                eapply cmplu_bool_preserved with (m3 := m3) in H; eauto using rs1_rs3;
-                try rewrite H in *;
-                (* idtac "done with Val.cmplu_bool 0"; *)
-                try congruence
-
-            | H: Val.cmplu_bool (Mem.valid_pointer ?m1) ?op (Vlong ?x) (?rs1 ?r') = Some ?b,
-                m1_m3: mem_rel _ _ _ ?j _ ?m1 ?m3,
-                rs1_rs3: regset_rel ?j ?rs1 ?rs3 |- _ =>
-                (* idtac "Val.cmplu_bool case 1"; *)
-                eapply cmplu_bool_preserved with (m3 := m3) (v1' := Vlong x) in H; eauto using rs1_rs3;
-                try rewrite H in *;
-                (* idtac "done with Val.cmplu_bool 1"; *)
-                try congruence
-
-            | H: Val.cmplu_bool (Mem.valid_pointer ?m1) ?op (?rs1 ?r) (Vlong ?x) = Some ?b,
-                m1_m3: mem_rel _ _ _ ?j _ ?m1 ?m3,
-                rs1_rs3: regset_rel ?j ?rs1 ?rs3 |- _ =>
-                (* idtac "Val.cmplu_bool case 2"; *)
-                eapply cmplu_bool_preserved with (m3 := m3) (v2' := Vlong x) in H; eauto using rs1_rs3;
-                try rewrite H in *;
-                (* idtac "done with Val.cmplu_bool 2"; *)
-                try congruence
-
-            | H: Val.cmplu_bool (Mem.valid_pointer ?m1) ?op (Vlong ?x) (Vlong ?y) = Some ?b,
-                m1_m3: mem_rel _ _ _ ?j _ ?m1 ?m3,
-                rs1_rs3: regset_rel ?j ?rs1 ?rs3 |- _ =>
-                (* idtac "Val.cmplu_bool case 3"; *)
-                eapply cmplu_bool_preserved with (m3 := m3) (v1' := Vlong x) (v2' := Vlong y) in H; eauto using rs1_rs3;
-                try rewrite H in *;
-                (* idtac "done with Val.cmplu_bool 3"; *)
-                try congruence
-
-            | H: Val.cmp_bool ?op (?rs1 ?r) (?rs1 ?r') = Some ?b,
-                m1_m3: mem_rel _ _ _ ?j _ ?m1 ?m3,
-                rs1_rs3: regset_rel ?j ?rs1 ?rs3 |- _ =>
-                (* idtac "Val.cmp_bool case"; *)
-                eapply Val.cmp_bool_inject in H; eauto using rs1_rs3;
-                try rewrite H in *;
-                (* idtac "done with Val.cmp_bool"; *)
-                try congruence
-
-            | d: Z |- _ =>
-                match goal with
-                | H: ?j _ = Some (_, d) ,
-                    m1_m3: mem_rel _ _ _ ?j _ ?m1 ?m3 |- _ =>
-                    let G := fresh "G" in
-                    pose proof (delta_zero _ _ _ _ _ _ _ m1_m3 _ _ _ H) as G;
-                    subst d
-                end
-
-
-            | |- context [Ptrofs.repr 0] => replace (Ptrofs.repr 0) with Ptrofs.zero by reflexivity; auto
-            | H: context [Ptrofs.repr 0] |- _ => replace (Ptrofs.repr 0) with Ptrofs.zero in H by reflexivity; auto
-            | |- context [Ptrofs.add _ Ptrofs.zero] => rewrite Ptrofs.add_zero; auto
-            | H: context [Ptrofs.add _ Ptrofs.zero] |- _ => rewrite Ptrofs.add_zero in H; simpl in *; try congruence
-            | |- context [Ptrofs.sub _ Ptrofs.zero] => rewrite Ptrofs.sub_zero_l; auto
-            | H: context [Ptrofs.sub _ Ptrofs.zero] |- _ => rewrite Ptrofs.sub_zero_l in H; simpl in *; try congruence
-
-            (* hypothesis manipulation *)
-            | rs1_rs3: regset_rel ?j ?rs1 ?rs3,
-              _: context [match ?rs1 ?i with | _ => _ end] |- _ =>
-                let H := fresh "rs1_rs3" in
-                assert (H := rs1_rs3 i);
-                destruct (rs1 i); inv H; try congruence; simpl in *; eauto
-
-            | rs1_rs3: regset_rel ?j ?rs1 ?rs3,
-              _: context [Val.offset_ptr (?rs1 ?i) _] |- _ =>
-                let H := fresh "rs1_rs3" in
-                assert (H := rs1_rs3 i);
-                destruct (rs1 i); inv H; try congruence; simpl in *; eauto
-
-            | H: Next _ _ = Next _ _ |- _ => inv H
-            | H: Some _ = Some _ |- _ => inv H
-            | H: Some _ = None |- _ => inv H
-            | H: None = Some _ |- _ => inv H
-            | H: Stuck = Next _ _ |- _ => inv H
-            | H: Next _ _ = Stuck |- _ => inv H
-            | H: negb _ = true |- _ => apply negb_true_iff in H
-            | H: negb _ = false |- _ => apply negb_false_iff in H
-            | H: Int.eq ?x ?x = false |- _ => rewrite Int.eq_true in H
-            | H: Int64.eq ?x ?x = false |- _ => rewrite Int64.eq_true in H
-            | H: Int.lt ?x ?x = true |- _ => rewrite lt_xx_false in H
-            | H: Int64.lt ?x ?x = true |- _ => rewrite lt64_xx_false in H
-            | H: Int.ltu ?x ?x = true |- _ => rewrite ltu_xx_false in H
-            | H: Int64.ltu ?x ?x = true |- _ => rewrite ltu64_xx_false in H
-            | H: false = true |- _ => congruence
-            | H: true = false |- _ => congruence
-            | H: ?x = false, H': ?x = true |- _ => congruence
-            | H: match ?x with | _ => _ end = Next _ _ |- _ =>
-                let eq := fresh "eq" in
-                destruct x eqn:eq; simpl in *; try congruence
-            | _: context [?rs1 ### ?rs] |- context [?rs3 ### ?rs] =>
-                let i := fresh "i" in destruct rs as [| i]; simpl in *
-            | _: context [?rs1 ## ?rs] |- context [?rs3 ## ?rs] =>
-                let i := fresh "i" in destruct rs as [| i]; simpl in *
-            | H: ?x = _ |- context [if ?x then _ else _] =>
-                setoid_rewrite H; simpl
-            | H: ?x = _ |- context [match ?x with | _ => _ end] =>
-                setoid_rewrite H; simpl
-            | |- context [(if ?x then _ else _) = Next _ _] =>
-                let eq := fresh "eq" in destruct x eqn:eq; simpl in *
-            | |- context [(match ?x with | _ => _ end) = Next _ _] =>
-                let eq := fresh "eq" in destruct x eqn:eq; simpl in *
-
-            end);
-    simpl.
-
-  Ltac solve_simple_regset_rel j rs1 rs3 rs1_rs3 m1 m3 m1_m3:=
-    repeat (Simpl;
-            match goal with
-            | |- regset_rel j (nextinstr _) (nextinstr _) => unfold nextinstr
-            | |- regset_rel j (_ # _ <- _) (_ # _ <- _) => eapply regset_rel_inject
-            | |- regset_rel j rs1 rs3 => assumption
-
-            | |- stack_rel _ _ _ _ _ _ => eauto using inject_incr_stack_rel1, inject_incr_stack_rel2, inject_incr_refl
-
-            | _: ?x |- ?x => assumption
-
-            | d: Z |- _ =>
-                match goal with
-                | H: j _ = Some (_, d) |- _ =>
-                    let G := fresh "G" in
-                    pose proof (delta_zero _ _ _ _ _ _ _ m1_m3 _ _ _ H) as G;
-                    subst d
-                end
-
-
-            | |- Ptrofs.add (Ptrofs.add ?ofs1 ?delta) ?imm = Ptrofs.add (Ptrofs.add ?ofs1 ?imm) ?delta =>
-                now rewrite (Ptrofs.add_assoc ofs1 delta imm), (Ptrofs.add_commut delta imm), <- Ptrofs.add_assoc
-
-            | |- context [_ ### ?rs] =>
-                let i := fresh "i" in destruct rs as [| i]; simpl in *
-            | |- context [_ ## ?rs] =>
-                let i := fresh "i" in destruct rs as [| i]; simpl in *
-            (* | |- context [rs1 # ?i] => *)
-            (*     match goal with *)
-            (*     | |- context [rs3 # ?i] => *)
-            (*         let H := fresh "rs1_rs3" in *)
-            (*         assert (H := rs1_rs3 i); inv H; simpl; eauto *)
-            (*     end *)
-
-
-            | |- context [Ptrofs.sub (Ptrofs.add _ _) _] => rewrite Ptrofs.sub_add_l; simpl; auto
-            | |- context [Ptrofs.repr 0] => replace (Ptrofs.repr 0) with Ptrofs.zero by reflexivity; auto
-            | |- context [Ptrofs.add _ Ptrofs.zero] => rewrite Ptrofs.add_zero; auto
-            | |- context [Ptrofs.sub _ Ptrofs.zero] => rewrite Ptrofs.sub_zero_l; auto
-
-
-
-            | |- Val.inject _ _ _ => eauto using Ptrofs.add_zero with solve_inject
-            end).
-
-  (* Lemma exec_instr_preserved: *)
-  (*   forall δ j f i rs1 rs1' rs3 m1 m1' m3 st1 st3, *)
-  (*     s |= has_comp_function f ∈ δ -> *)
-  (*     mem_rel s ge1 ge3 j δ m1 m3 -> *)
-  (*     regset_rel j rs1 rs3 -> *)
-  (*     stack_rel s j δ st1 st3 -> *)
-  (*     exec_instr ge1 f i rs1 m1 (has_comp_function f) = Next rs1' m1' -> *)
-  (*     exists j' rs3' m3', *)
-  (*       exec_instr ge3 f i rs3 m3 (has_comp_function f) = Next rs3' m3' /\ *)
-  (*         mem_rel s ge1 ge3 j' δ m1' m3' /\ *)
-  (*         regset_rel j' rs1' rs3' /\ *)
-  (*         stack_rel s j' δ st1 st3. *)
-
-  Lemma exec_instr_preserved_left:
-    forall j__left j__right f i rs1 rs1' rs3 m1 m1' m2 m3 st1 st2 st3,
-      s |= has_comp_function f ∈ Left ->
-      mem_rel s ge1 ge3 j__left Left m1 m3 ->
-      mem_rel s ge2 ge3 j__right Right m2 m3 ->
-      regset_rel j__left rs1 rs3 ->
-      stack_rel s j__left j__right st1 st2 st3 ->
-      (* stack_rel s j δ st1 st3 -> *)
-      exec_instr ge1 f i rs1 m1 (has_comp_function f) = Next rs1' m1' ->
-      exists j__left' rs3' m3',
-        exec_instr ge3 f i rs3 m3 (has_comp_function f) = Next rs3' m3' /\
-          mem_rel s ge1 ge3 j__left' Left m1' m3' /\
-          mem_rel s ge2 ge3 j__right Right m2 m3' /\
-          regset_rel j__left' rs1' rs3' /\
-          stack_rel s j__left' j__right st1 st2 st3.
-  Proof.
-    intros until st3.
-    intros side_cp m1_m3 m2_m3 rs1_rs3 st1_st3 exec.
-
-    Local Opaque Val.cmpu_bool Val.cmplu_bool.
-    (* Local Opaque low_half high_half. *)
-
-    destruct i; inv exec; simpl in *;
-      try now (simpl_before_exists; (eexists_and_split
-                  ltac:(fun j rs1 rs3 rs1_rs3 m1 m3 m1_m3 =>
-                          (simpl; try reflexivity; try eassumption;
-                           solve_simple_regset_rel j rs1 rs3 rs1_rs3 m1 m3 m1_m3; try reflexivity)))).
-    - (eexists_and_split
-         ltac:(fun j rs1 rs3 rs1_rs3 m1 m3 m1_m3 =>
-                 (simpl; try reflexivity; try eassumption;
-                  solve_simple_regset_rel j rs1 rs3 rs1_rs3 m1 m3 m1_m3; try reflexivity))).
-      (* apply Genv.find_symbol_match with (s := symb) in match_W1_W3. *)
-      exploit symb_inj. exact m1_m3. intros (A & B & C & D).
-      unfold Genv.symbol_address. admit.
-    - (eexists_and_split
-         ltac:(fun j rs1 rs3 rs1_rs3 m1 m3 m1_m3 =>
-                 (simpl; try reflexivity; try eassumption;
-                  solve_simple_regset_rel j rs1 rs3 rs1_rs3 m1 m3 m1_m3; try reflexivity))).
-      (* apply Genv.find_symbol_match with (s := symb) in match_W1_W3. *)
-      admit.
-      (* unfold Genv.symbol_address. rewrite match_W1_W3. *)
-      (* now eapply symbol_address_inject; eauto using pres_globals. *)
-    - (eexists_and_split
-         ltac:(fun j rs1 rs3 rs1_rs3 m1 m3 m1_m3 =>
-                 (simpl; try reflexivity; try eassumption;
-                  solve_simple_regset_rel j rs1 rs3 rs1_rs3 m1 m3 m1_m3; try reflexivity))).
-      apply Genv.find_symbol_match with (s := id) in match_W1_W3.
-      admit.
-      (* unfold Genv.symbol_address. rewrite match_W1_W3. *)
-      (* now eapply symbol_address_inject; eauto using pres_globals. *)
-    - (eexists_and_split
-         ltac:(fun j rs1 rs3 rs1_rs3 m1 m3 m1_m3 =>
-                 (simpl; try reflexivity; try eassumption;
-                  solve_simple_regset_rel j rs1 rs3 rs1_rs3 m1 m3 m1_m3; try reflexivity))).
-      eapply same_high_half; eauto.
-  Admitted.
-
-  Lemma store_inj_outside_domain:
-    forall f chunk m1 b1 ofs v1 cp n2 m2,
-      Mem.mem_inj f m1 m2 ->
-      Mem.store chunk m2 b1 ofs v1 cp = Some n2 ->
-      (forall b0 delta, f b0 = Some (b1, delta) -> False) ->
-      Mem.mem_inj f m1 n2.
-  Proof.
-    intros. constructor.
-    (* perm *)
-    intros. eapply Mem.mi_perm in H; eauto. eapply Mem.perm_store_1; eauto.
-    (* own *)
-    intros. eapply Mem.mi_own in H; eauto.
-    (* RB: NOTE: Should be solvable by properly extended hint databases. *)
-    apply (proj1 (Mem.store_can_access_block_inj _ _ _ _ _ _ _ H0 _ _)).
-    assumption.
-    (* align *)
-    intros. eapply Mem.mi_align with (ofs := ofs0) (p := p) in H; eauto.
-    (* mem_contents *)
-    intros.
-    (* Local Transparent Mem.store. *)
-    (* unfold Mem.store in H0. *)
-    (* destruct Mem.valid_access_dec; try congruence. *)
-    (* inv H0. simpl. *)
-    eapply Mem.mi_memval in H; eauto.
-    rewrite (Mem.store_mem_contents _ _ _ _ _ _ _ H0).
-    rewrite PMap.gso. eauto with mem.
-    intros ?. subst. now eapply H1; eauto.
-  Qed.
-
-
-  Theorem store_inject_outside_domain:
-    forall f chunk m1 b1 ofs v1 cp n2 m2,
-      Mem.inject f m1 m2 ->
-      Mem.store chunk m2 b1 ofs v1 cp = Some n2 ->
-      (forall b0 delta, f b0 = Some (b1, delta) -> False) ->
-      Mem.inject f m1 n2.
-  Proof.
-    intros. inversion H.
-    constructor.
-    (* inj *)
-    eapply store_inj_outside_domain; eauto.
-    (* freeblocks *)
-    eauto with mem.
-    (* mappedblocks *)
-    eauto with mem.
-    (* no overlap *)
-    red; intros. eauto with mem.
-    (* representable *)
-    intros. eapply mi_representable; try eassumption.
-    (* destruct H3; eauto with mem. *)
-    (* perm inv *)
-    intros. exploit mi_perm_inv; eauto using Mem.perm_store_2.
-  Qed.
-
-  (* Lemma exec_instr_preserved': *)
-  (*   forall δ j f i rs3 rs3' m1 m3 m3' st1 st3, *)
-  (*     s |= has_comp_function f ∈ opposite δ -> *)
-  (*     mem_rel s ge2 ge3 j δ m1 m3 -> *)
-  (*     stack_rel s j δ st1 st3 -> *)
-  (*     exec_instr ge3 f i rs3 m3 (has_comp_function f) = Next rs3' m3' -> *)
-  (*     mem_rel s ge2 ge3 j δ m1 m3' /\ *)
-  (*       stack_rel s j δ st1 st3. *)
-  (* Proof. *)
-  (*   intros until st3. *)
-  (*   intros side_cp m1_m3 st1_st3 exec. *)
-
-  (*   assert ( forall chunk addr v, *)
-  (*       s |= has_comp_function f ∈ opposite δ -> *)
-  (*       mem_rel s ge2 ge3 j δ m1 m3 -> *)
-  (*       Mem.storev chunk m3 addr v (has_comp_function f) = Some m3' -> *)
-  (*       mem_rel s ge2 ge3 j δ m1 m3' *)
-  (*          ). *)
-  (*   { clear. *)
-  (*     intros chunk addr v side_cp m1_m3 store. *)
-  (*     destruct m1_m3. *)
-  (*     constructor; auto. *)
-  (*     - destruct addr; simpl in store; try congruence. *)
-  (*       eapply store_inject_outside_domain; eauto. *)
-  (*       intros. *)
-  (*       specialize (same_dom0 b0) as [G _]. *)
-  (*       assert (N: j b0 <> None) by now congruence. *)
-  (*       specialize (G N). simpl in *. *)
-  (*       apply Mem.store_can_access_block_1 in store. simpl in store. *)
-  (*       destruct (Mem.block_compartment m1 b0) as [c' |] eqn:eq; try congruence. *)
-  (*       assert (Mem.can_access_block m1 b0 (Some c')) by auto. *)
-  (*       exploit Mem.mi_own; eauto using Mem.mi_inj. *)
-  (*       intros ?. simpl in H1. subst. rewrite H1 in store; inv store. *)
-  (*       now destruct (s (has_comp_function f)). *)
-  (*     - destruct addr; simpl in store; try congruence. *)
-  (*       erewrite Mem.nextblock_store; eauto. *)
-  (*     - intros. *)
-  (*       destruct addr; simpl in store; try congruence. *)
-  (*       eapply Mem.store_valid_block_1; eauto. } *)
-  (*   destruct i; inv exec; simpl in *; split; auto; *)
-  (*     simpl_before_exists; *)
-  (*     simpl in *; try now eapply H; eauto. *)
-  (*   admit. *)
-  (*   admit. *)
-  (* Admitted. *)
-
-
-  Lemma strong_equiv_state_inv_left:
-    forall j__left st1 rs1 m1 s3 b ofs f i,
-      strong_equivalence s ge1 ge3 j__left Left (State st1 rs1 m1) s3 ->
-      rs1 PC = Vptr b ofs ->
-      Genv.find_funct_ptr ge1 b = Some (Internal f) ->
-      find_instr (Ptrofs.unsigned ofs) (fn_code f) = Some i ->
-      exists st3 rs3 m3,
-        s3 = State st3 rs3 m3 /\
-          rs3 PC = Vptr b ofs /\
-          Genv.find_funct_ptr ge3 b = Some (Internal f) /\
-          mem_rel s ge1 ge3 j__left Left m1 m3 /\
-          regset_rel j__left rs1 rs3 /\
-          s (has_comp_function f) = Left.
-  Proof.
-    intros * equiv eq_pc find_fun find_ins.
-    inv equiv.
-    eexists; eexists; eexists; split; eauto.
-    exploit (Genv.find_funct_ptr_match match_W1_W3); eauto.
-    intros [[] [f' [find_f' [match_f_f' _]]]].
-    inv match_f_f'; simpl in *.
-    - rewrite eq_pc in *; simpl in *.
-      (* destruct Ptrofs.eq_dec; try congruence. unfold ge1 in *. rewrite find_fun in H2. *)
-      (* simpl in *; congruence. *)
-      admit.
-    - pose proof (H4 PC) as inj.
-      rewrite eq_pc in *; simpl in *. inv inj.
-      exploit funct_preserved1; eauto. intros.
-      assert (b2 = b) by congruence; assert (delta = 0) by congruence; subst b2 delta.
-
-      apply Genv.globalenvs_match in match_W1_W3.
-      apply Genv.mge_defs with (b := b) in match_W1_W3.
-      inv match_W1_W3.
-      + unfold Genv.find_funct_ptr in *. unfold Genv.find_def in *. rewrite <- H7 in *. congruence.
-      + unfold Genv.find_funct_ptr in *. unfold Genv.find_def in *. rewrite <- H7 in *. rewrite <- H1 in *.
-        inv H8; inv find_fun.
-        inv H10; repeat (split; eauto).
-        * now rewrite Ptrofs.add_zero.
-        * now rewrite Ptrofs.add_zero.
-  (* Qed. *)
-  Admitted.
-
-  Lemma find_comp_preserved:
-    forall j rs rs' r
-      (funct_preserved1: forall (b : block) (fd : fundef), Genv.find_funct_ptr ge1 b = Some fd -> j b = Some (b, 0))
-      (funct_preserved2: forall (b1 b2 : block) (fd : fundef), Genv.find_funct_ptr ge3 b2 = Some fd -> j b1 = Some (b2, 0) -> b1 = b2)
-      (delta_zero: Mem.delta_zero j),
-      rs r <> Vundef ->
-      regset_rel j rs rs' ->
-      Genv.find_comp ge1 (rs r) =
-        Genv.find_comp ge3 (rs' r).
-  Proof.
-    intros j rs rs' r funct_preserved1 funct_preserved2 delta_zero nundef H.
-    specialize (H r).
-    inv H; simpl; auto; try congruence.
-(*
-    destruct Ptrofs.eq_dec; auto.
-    { destruct (Genv.find_funct_ptr ge1 b1) eqn:find_funct;
-        destruct (Genv.find_funct_ptr ge3 b2) eqn:find_funct';
-        auto.
-      - exploit funct_preserved1; eauto; intros.
-        assert (b1 = b2) by congruence; assert (delta = 0) by congruence; subst b2 delta.
-        eapply Genv.find_funct_ptr_match in match_W1_W3 as [? [f' [? [match_fd ?]]]]; eauto.
-        assert (f0 = f') by congruence; subst f0.
-        now inv match_fd.
-      - exploit funct_preserved1; eauto; intros.
-        assert (b1 = b2) by congruence; assert (delta = 0) by congruence; subst b2 delta.
-        eapply Genv.find_funct_ptr_match in match_W1_W3 as [? [f' [? [match_fd ?]]]]; eauto.
-        congruence.
-      - exploit delta_zero; eauto; intros ->.
-        exploit funct_preserved2; eauto; intros <-.
-        eapply Genv.find_funct_ptr_match_conv in match_W1_W3 as [? [f' [? [match_fd ?]]]]; eauto.
-        congruence.
-      - exploit delta_zero; eauto; intros ->.
-        rewrite Ptrofs.add_zero.
-        destruct Ptrofs.eq_dec; auto. }
-    { destruct Ptrofs.eq_dec; auto.
-      exploit delta_zero; eauto; intros ->.
-      rewrite Ptrofs.add_zero in *; congruence. }
-  Qed.
-*)
-  Admitted.
-
-(*
-  Lemma find_comp_ignore_offset_preserved:
-    forall j rs rs' r
-      (funct_preserved1: forall (b : block) (fd : fundef), Genv.find_funct_ptr ge1 b = Some fd -> j b = Some (b, 0))
-      (funct_preserved2: forall (b1 b2 : block) (fd : fundef), Genv.find_funct_ptr ge3 b2 = Some fd -> j b1 = Some (b2, 0) -> b1 = b2)
-      (delta_zero: Mem.delta_zero j),
-      rs r <> Vundef ->
-      regset_rel j rs rs' ->
-      Genv.find_comp_ignore_offset ge1 (rs r) =
-        Genv.find_comp_ignore_offset ge3 (rs' r).
-  Proof.
-    intros j rs rs' r funct_preserved1 funct_preserved2 delta_zero nundef H.
-    specialize (H r).
-    inv H; simpl; auto; try congruence.
-    destruct Ptrofs.eq_dec; auto.
-    destruct (Genv.find_funct_ptr ge1 b1) eqn:find_funct;
-      destruct (Genv.find_funct_ptr ge3 b2) eqn:find_funct';
-      auto.
-    - exploit funct_preserved1; eauto; intros.
-      assert (b1 = b2) by congruence; assert (delta = 0) by congruence; subst b2 delta.
-      eapply Genv.find_funct_ptr_match in match_W1_W3 as [? [f' [? [match_fd ?]]]]; eauto.
-      assert (f0 = f') by congruence; subst f0.
-      now inv match_fd.
-    - exploit funct_preserved1; eauto; intros.
-      assert (b1 = b2) by congruence; assert (delta = 0) by congruence; subst b2 delta.
-      eapply Genv.find_funct_ptr_match in match_W1_W3 as [? [f' [? [match_fd ?]]]]; eauto.
-      congruence.
-    - exploit delta_zero; eauto; intros ->.
-      exploit funct_preserved2; eauto; intros <-.
-      eapply Genv.find_funct_ptr_match_conv in match_W1_W3 as [? [f' [? [match_fd ?]]]]; eauto.
-      congruence.
-  Qed.
-*)
-
+  (* Calls *)
   Lemma allowed_call_preserved:
-    forall j cp v v'
-      (funct_preserved1: forall (b : block) (fd : fundef), Genv.find_funct_ptr ge1 b = Some fd -> j b = Some (b, 0))
-      (funct_preserved2: forall (b1 b2 : block) (fd : fundef), Genv.find_funct_ptr ge3 b2 = Some fd -> j b1 = Some (b2, 0) -> b1 = b2)
-      (delta_zero: Mem.delta_zero j),
+    forall j__δ cp v v'
+      (inj_pres: meminj_preserves_globals s δ W1 W3 j__δ)
+      (delta_zero: mem_delta_zero j__δ),
       v <> Vundef ->
-      Val.inject j v v' ->
+      Val.inject j__δ v v' ->
       Genv.allowed_call ge1 cp v ->
       Genv.allowed_call ge3 cp v'.
   Proof.
-    intros * funct_preserved1 funct_preserved2 delta_zero nundef H allowed.
-    inv H; auto; try congruence.
-    (* unfold Genv.allowed_call, Genv.find_comp in allowed. *)
-    destruct (Genv.find_funct ge1 (Vptr b1 ofs1)) eqn:find_v.
-    - simpl in find_v; destruct Ptrofs.eq_dec; try congruence; subst.
-      (* exploit delta_zero; eauto; intros ?; subst delta0. *)
-      exploit funct_preserved1; eauto. intros ?.
-      assert (b1 = b2) by congruence. assert (delta = 0) by congruence. subst b2 delta.
-      rewrite Ptrofs.add_zero.
-      eapply Genv.match_genvs_allowed_calls in match_W1_W3; eauto using has_comp_match_fundef.
-    - destruct (Genv.find_funct ge3 (Vptr b2 (Ptrofs.add ofs1 (Ptrofs.repr delta)))) eqn:find_v'.
-      + exploit delta_zero; eauto. intros ->. rewrite Ptrofs.add_zero in *.
-        simpl in find_v'. destruct Ptrofs.eq_dec; try congruence; subst.
-        exploit funct_preserved2; eauto. intros <-.
-        eapply Genv.find_funct_match_conv with (v := Vptr b1 Ptrofs.zero) in match_W1_W3; eauto.
-        destruct match_W1_W3 as [? [? [? [? ?]]]]; congruence.
-      + destruct allowed.
-(*
-        * left; subst; auto. simpl in *; now rewrite find_v, find_v'.
-        * right. simpl in *. rewrite find_v, find_v' in *.
-          admit.
-*)
-  Admitted.
-
-  Lemma update_stack_call_preserved_left:
-    forall j__left j__right rs1 rs3 st1 st1' st2 st3 cp sig
-      (funct_preserved1: forall (b : block) (fd : fundef), Genv.find_funct_ptr ge1 b = Some fd -> j__left b = Some (b, 0))
-      (funct_preserved2: forall (b1 b2 : block) (fd : fundef), Genv.find_funct_ptr ge3 b2 = Some fd -> j__left b1 = Some (b2, 0) -> b1 = b2)
-      (delta_zero: Mem.delta_zero j__left)
-      (left_side: (s, ge3) |= rs3 ∈ Left),
-      (rs1 PC <> Vundef) ->
-      regset_rel j__left rs1 rs3 ->
-      stack_rel s j__left j__right st1 st2 st3 ->
-      update_stack_call ge1 st1 sig cp rs1 = Some st1' ->
-      exists st3',
-        update_stack_call ge3 st3 sig cp rs3 = Some st3' /\
-          stack_rel s j__left j__right st1' st2 st3'.
-  Proof.
-    intros * funct_preserved1 funct_preserved2 delta_zero left_side nundef rs1_rs3 st_rel.
-    unfold update_stack_call.
-(*
-    erewrite find_comp_ignore_offset_preserved; eauto.
-    destruct ((cp =? Genv.find_comp_ignore_offset ge3 (rs3 PC))%positive); auto.
-    - intros R; inv R.
-      eexists; split; auto.
-    - pose proof (rs1_rs3 X1) as I.
-      inv I; try congruence.
-      intros R; inv R.
-      eexists; split; auto.
-      + eapply stack_rel_cons_left with (st2' := nil); simpl; eauto.
-        constructor; auto. econstructor; eauto.
+    intros * inj_pres delta_zero nundef H allowed.
+    exploit find_comp_preserved; eauto.
+    intros same_comp.
+    destruct allowed as [eq_comp | cross_call].
+    - left; congruence.
+    - right.
+      inv H; auto; try congruence.
+      exploit delta_zero; eauto; intros ->; rewrite Ptrofs.add_zero in *.
+      clear nundef.
+      destruct cross_call as [id [cp' [inv_symb ?]]].
+      exists id, cp'. split.
+      + apply Genv.invert_find_symbol in inv_symb.
+        apply Genv.find_invert_symbol.
+        exploit symbols_inject1; eauto; intros []; auto.
+      + replace (Genv.genv_policy ge3) with (prog_pol W3) by (symmetry; apply Genv.genv_pol_add_globals).
+        replace (Genv.genv_policy ge1) with (prog_pol W1) in * by (symmetry; apply Genv.genv_pol_add_globals).
+        rewrite (match_prog_pol _ _ _ _ match_W1_W3), <- same_comp.
+        destruct H as [? ?]. split; auto.
   Qed.
-*)
-  Admitted.
+  (*       unfold Genv.find_funct, Genv.find_funct_ptr in *. *)
+  (*       intros fd; specialize (H fd). *)
+  (*       destruct (Ptrofs.eq_dec ofs1 Ptrofs.zero); try congruence. *)
+  (*       destruct (Genv.find_def ge3 b2) as [[] |] eqn:?; try congruence. *)
+  (*       exploit defs_rev_inject; eauto. *)
+  (*       intros [? [? [? ?]]]. *)
+  (*       rewrite H2 in H. inv H4. simpl. intros G. inv G. *)
+  (*       inv H7; auto. specialize (H eq_refl). auto. *)
+  (* Qed. *)
+
+  Lemma update_stack_call_preserved_internal:
+    forall j__δ sg rs1 rs3 st1 st1' st3 cp
+      (delta_zero: mem_delta_zero j__δ),
+      agrees_with j__δ (init_meminj W1 W3) ->
+      (rs1 PC <> Vundef) ->
+      Genv.find_comp ge1 (rs1 PC) = Some cp ->
+      regset_rel j__δ rs1 rs3 ->
+      update_stack_call ge1 st1 sg cp rs1 = Some st1' ->
+      st1' = st1 /\
+        update_stack_call ge3 st3 sg cp rs3 = Some st3.
+  Proof.
+    intros * delta_zero agr nundef samecomp rs1_rs3.
+    unfold update_stack_call.
+    rewrite samecomp, Pos.eqb_refl.
+    intros R; inv R.
+    split; eauto.
+    exploit (agrees_with_init_meminj_find_comp_preserved s W1 W3); eauto.
+    intros ->. rewrite Pos.eqb_refl; eauto.
+  Qed.
 
   Lemma call_arguments_preserved:
-    forall j δ m1 m3 rs1 rs3,
-      mem_rel s ge1 ge3 j δ m1 m3 ->
-      regset_rel j rs1 rs3 ->
+    forall j__δ m1 m3 rs1 rs3,
+      mem_rel s ge1 ge3 j__δ δ m1 m3 ->
+      regset_rel j__δ rs1 rs3 ->
       forall sig args, call_arguments rs1 m1 sig args ->
-                  exists args', Val.inject_list j args args'
+                  exists args', Val.inject_list j__δ args args'
                            /\ call_arguments rs3 m3 sig args'.
   Proof.
     intros * m1_m3 rs1_rs3 sig args H.
@@ -1512,7 +1680,7 @@ Section Simulation.
     unfold call_arguments.
     induction H.
     - exists nil. split; auto. constructor.
-    - assert (exists b1', Val.inject j b1 b1' /\ call_arg_pair rs3 m3 a1 b1').
+    - assert (exists b1', Val.inject j__δ b1 b1' /\ call_arg_pair rs3 m3 a1 b1').
       { inv H.
         - inv H1.
           + specialize (rs1_rs3 (preg_of r)).
@@ -1553,209 +1721,353 @@ Section Simulation.
       + constructor; eauto.
   Qed.
 
-  Notation comp_of1 := (@comp_of _ (has_comp_state W1)).
-  Notation comp_of2 := (@comp_of _ (has_comp_state W2)).
-  Notation comp_of3 := (@comp_of _ (has_comp_state W3)).
-
-  Definition stack_of_state (s: state) :=
-    match s with
-    | State st _ _ | ReturnState st _ _ _ => st
-    end.
-
-  Lemma step_E0_strong_Left: forall (s1 s1': state),
-      Step (semantics W1) s1 E0 s1' ->
-      (s (comp_of1 s1) = s (comp_of1 s1')) ->
-      forall (s2 s3: state) j__left j__right,
-        stack_rel s j__left j__right (stack_of_state s1) (stack_of_state s2) (stack_of_state s3) ->
-        strong_equivalence s ge1 ge3 j__left Left s1 s3 ->
-        weak_equivalence s ge2 ge3 j__right Right s2 s3 ->
-        exists (s3': state) j__left' j__right',
-          Plus (semantics W3) s3 E0 s3' /\
-            stack_rel s j__left' j__right' (stack_of_state s1') (stack_of_state s2) (stack_of_state s3') /\
-            strong_equivalence s ge1 ge3 j__left' Left s1' s3' /\
-            weak_equivalence s ge2 ge3 j__right' Right s2 s3'.
+  Lemma call_trace_preserved:
+    forall j__δ cp cp' v v' args args' sig t
+      (agr: agrees_with j__δ (init_meminj W1 W3))
+      (delta_zero: mem_delta_zero j__δ),
+      Val.inject j__δ v v' ->
+      Val.inject_list j__δ args args' ->
+      (Genv.type_of_call cp cp' = Genv.CrossCompartmentCall -> Forall not_ptr args) ->
+      call_trace ge1 cp cp' v args (sig_args sig) t ->
+      call_trace ge3 cp cp' v' args' (sig_args sig) t.
   Proof.
-    simpl.
-    intros s1 s1' H same_side s2 s3 j__left j__right st_rel strong_s1_s3 weak_s2_s3; inv H.
-    - exploit strong_equiv_state_inv_left; eauto.
-      intros (st3 & rs3 & m3 & ? & eq_pc' & find_funct & m1_m3 & rs1_rs3 & side_f); subst.
-      inv weak_s2_s3.
-      exploit exec_instr_preserved_left; simpl; eauto.
-      intros (j__left' & rs3' & m3' & exec_instr' & m1_m3' & m2_m3' & rs1_rs3' & st_rel').
-(*
-      assert (pc_comp: Genv.find_comp_ignore_offset ge1 (rs' PC) = Genv.find_comp_ignore_offset ge3 (rs3' PC)).
-      { pose proof (rs1_rs3' PC) as inj_pc; rewrite NEXTPC in *; inv inj_pc.
-        assert (delta = 0) by now eapply delta_zero with (j := j__left'); eauto. subst delta.
-        rewrite Ptrofs.add_zero.
-        simpl. destruct Ptrofs.eq_dec; try congruence.
-        destruct (Genv.find_funct_ptr ge1 b') eqn:A.
-        - exploit (Genv.find_funct_ptr_match match_W1_W3); eauto.
-          intros [[] [f' [find_f' [match_f_f' _]]]].
-          exploit (funct_preserved1 s ge1 ge3); eauto. intros.
-          assert (b2 = b') by congruence; subst. rewrite find_f'.
-          now inv match_f_f'.
-        - destruct (Genv.find_funct_ptr ge3 b2) eqn:B; [| reflexivity].
-          exploit (funct_preserved2 s ge1 ge3); eauto. intros; subst.
-          (* Find a contradiction *)
-          apply Genv.find_funct_ptr_iff in B.
-          apply Genv.find_def_match_2 with (b := b2) in match_W1_W3.
-          inv match_W1_W3; try congruence.
-          inv H11; try congruence.
-          symmetry in H. apply <- Genv.find_funct_ptr_iff in H. congruence.
-      }
-      exists (State st3 rs3' m3'), j__left', j__right; split; [| split; [| split]].
-      + econstructor; [| now eapply star_refl | now traceEq].
-        (* unfold ge3 in exec_instr'. *)
-        pose proof (rs1_rs3' PC) as inj_pc; rewrite NEXTPC in *; inv inj_pc. rewrite <- H7 in *.
-        econstructor; eauto.
-        * rewrite <- ALLOWED; eauto.
-      + eauto.
-      + econstructor; eauto.
-        * simpl; rewrite NEXTPC; simpl in *; rewrite <- ALLOWED. auto.
-        (* * simpl. rewrite <- pc_comp. rewrite NEXTPC; simpl in *; rewrite <- ALLOWED. auto. *)
-      + econstructor; eauto.
+    intros j__δ cp cp' v v' args args' sig t agr delta_zero inj_v inj_args NPTR EV.
+    inv EV.
+    - constructor; auto.
+    - specialize (NPTR H).
+      inv inj_v; eauto.
+      econstructor; eauto. apply Genv.find_invert_symbol.
+      apply Genv.invert_find_symbol in H1.
+      eapply (symbols_inject2 _ _ W1 W3 (init_meminj W1 W3)) in H1;
+        eauto using init_meminj_preserves_globals.
+      destruct H1 as [? [? ?]]; eauto.
+      exploit agr; eauto. intros []; subst; eauto.
+      (* eapply Genv.invert_find_symbol; eauto. *)
+      remember (sig_args sig) as tys.
+      clear -inj_args NPTR H2.
+      revert args args' tys vl inj_args NPTR H2.
+      induction args;intros args' tys vl inj_args NPTR Hmatch.
+      + inv inj_args; inv Hmatch; constructor.
+      + inv inj_args; inv Hmatch; inv NPTR.
+        constructor; eauto.
+        inv H1; inv H5; try contradiction; econstructor; eauto.
+  Qed.
 
-    - exploit strong_equiv_state_inv_left; eauto.
-      intros (st3 & rs3 & m3 & ? & eq_pc' & find_funct & m1_m3 & rs1_rs3 & side_f); subst.
-      simpl in H3. destruct Ptrofs.eq_dec; try congruence. simpl in H1; rewrite H1 in H3.
-      inv weak_s2_s3.
-      exploit exec_instr_preserved_left; simpl; eauto.
-      intros (j__left' & rs3' & m3' & exec_instr' & m1_m3' & m2_m3' & rs1_rs3' & st_rel').
-      assert (pc_comp: Genv.find_comp_ignore_offset ge1 (rs' PC) = Genv.find_comp_ignore_offset ge3 (rs3' PC)).
-      { pose proof (rs1_rs3' PC) as inj_pc; rewrite NEXTPC in *; inv inj_pc.
-        assert (delta = 0) by now eapply (delta_zero s ge1 ge3); eauto. subst delta.
-        rewrite Ptrofs.add_zero.
-        simpl. destruct Ptrofs.eq_dec; try congruence.
-        destruct (Genv.find_funct_ptr ge1 b') eqn:A.
-        - exploit (Genv.find_funct_ptr_match match_W1_W3); eauto.
-          intros [[] [f' [find_f' [match_f_f' _]]]].
-          exploit (funct_preserved1 s ge1 ge3); eauto. intros.
-          assert (b2 = b') by congruence; subst. rewrite find_f'.
-          now inv match_f_f'.
-        - destruct (Genv.find_funct_ptr (Genv.globalenv W3) b2) eqn:B; [| reflexivity].
-          exploit (funct_preserved2 s ge1 ge3); eauto. intros; subst.
-          (* Find a contradiction *)
-          apply Genv.find_funct_ptr_iff in B.
-          apply Genv.find_def_match_2 with (b := b2) in match_W1_W3.
-          inv match_W1_W3; try congruence. inv H10; try congruence.
-          symmetry in H. apply <- Genv.find_funct_ptr_iff in H. congruence.
-      }
-
-      assert (is_left: s (Genv.find_comp_ignore_offset ge3 (rs3' PC)) = Left).
-      { simpl in same_side. rewrite <- pc_comp, <- same_side, H0.
-        simpl. rewrite H1. auto. }
-      exploit update_stack_call_preserved_left; [| | | exact is_left | | | | |];
-        eauto using funct_preserved1, funct_preserved2, delta_zero;
-        [congruence |].
-      intros [st3' [STUPD' st_rel'']].
-      exploit call_arguments_preserved; eauto.
-      intros [args' [inj_args call_args]].
-
-      exists (State st3' rs3' m3'), j__left', j__right; split; [| split; [| split]].
-      + econstructor; [| now eapply star_refl | now traceEq].
-        pose proof (rs1_rs3' PC) as inj_pc; rewrite NEXTPC in *; inv inj_pc. rewrite <- H6 in *.
-        (* clear dependent j0. *)
-        exploit (delta_zero s ge1 ge3); eauto. intros ->.
-        eapply exec_step_internal_call; eauto.
-        * eapply allowed_call_preserved with (v := Vptr b' Ptrofs.zero);
-            eauto using funct_preserved1, funct_preserved2, delta_zero.
-          congruence.
-        * simpl; now rewrite find_funct.
-        * simpl in STUPD'; now rewrite H1 in STUPD'.
-        * intros is_cross. unfold Genv.find_comp_ignore_offset in pc_comp.
-          rewrite <- pc_comp in is_cross.
-          specialize (NO_CROSS_PTR is_cross).
-          now eapply Val.inject_list_not_ptr; eauto.
-        * inv EV. constructor. unfold Genv.find_comp_ignore_offset in pc_comp.
-          now rewrite <- pc_comp.
-      + eauto.
-      + simpl in same_side.
-        econstructor; eauto.
-        simpl. rewrite <- same_side. rewrite H0. simpl. now rewrite H1.
-      + simpl in same_side.
-        econstructor; eauto.
-
-    (** [State] to [ReturnState] *)
-    - exploit strong_equiv_state_inv_left; eauto.
-      intros (st3 & rs3 & m3 & ? & eq_pc' & find_funct & m1_m3 & rs1_rs3 & side_f); subst.
-      rewrite H0 in H3. simpl in H3. destruct Ptrofs.eq_dec; try congruence. simpl in H1; rewrite H1 in H3.
-      inv weak_s2_s3.
-      exploit exec_instr_preserved_left; simpl; eauto.
-      intros (j__left' & rs3' & m3' & exec_instr' & m1_m3' & m2_m3' & rs1_rs3' & st_rel').
-      (* assert (pc_comp: Genv.find_comp_ignore_offset ge1 (rs' PC) = Genv.find_comp_ignore_offset ge3 (rs3' PC)). *)
-      (* { pose proof (rs1_rs3' PC) as inj_pc; inv inj_pc; auto. admit. *)
-      (*   assert (delta = 0) by now eapply delta_zero; eauto. subst delta. *)
-      (*   rewrite Ptrofs.add_zero. *)
-      (*   simpl. destruct Ptrofs.eq_dec; try congruence. *)
-      (*   destruct (Genv.find_funct_ptr ge1 b') eqn:A. *)
-      (*   - exploit (Genv.find_funct_ptr_match match_W1_W3); eauto. *)
-      (*     intros [[] [f' [find_f' [match_f_f' _]]]]. *)
-      (*     exploit funct_preserved1; eauto. intros. *)
-      (*     assert (b2 = b') by congruence; subst. rewrite find_f'. *)
-      (*     now inv match_f_f'. *)
-      (*   - destruct (Genv.find_funct_ptr (Genv.globalenv W3) b2) eqn:B; [| reflexivity]. *)
-      (*     exploit funct_preserved2; eauto. intros; subst. *)
-      (*     (* Find a contradiction *) *)
-      (*     apply Genv.find_funct_ptr_iff in B. *)
-      (*     apply Genv.find_def_match_2 with (b := b2) in match_W1_W3. *)
-      (*     inv match_W1_W3; try congruence. inv H8; try congruence. *)
-      (*     symmetry in H. apply <- Genv.find_funct_ptr_iff in H. congruence. *)
-      (* } *)
-
-      (* assert (is_left: s (Genv.find_comp_ignore_offset ge3 (rs3' PC)) = Left). *)
-      (* { simpl in same_side. rewrite <- pc_comp, <- same_side, H0. *)
-      (*   simpl. rewrite H1. auto. } *)
-      (* exploit update_stack_call_preserved; [| | | exact is_left | | | | | | ]; *)
-      (*   eauto using funct_preserved1, funct_preserved2, delta_zero; *)
-      (*   [congruence |]. *)
-      (* intros [st3' [STUPD' [st'_st3' st2_st3']]]. *)
-      (* exploit call_arguments_preserved; eauto. *)
-      (* intros [args' [inj_args call_args]]. *)
-
-      exists (ReturnState st3 rs3' m3'), j__left', j__right; split; [| split; [| split]].
-      + econstructor; [| now eapply star_refl | now traceEq].
-        (* pose proof (rs1_rs3' PC) as inj_pc; rewrite NEXTPC in *; inv inj_pc. rewrite <- H6 in *. *)
-        (* clear dependent j0. *)
-        eapply exec_step_internal_return; eauto.
-        * rewrite eq_pc'. simpl. destruct Ptrofs.eq_dec; try congruence; now rewrite find_funct.
-        * rewrite eq_pc'. simpl. destruct Ptrofs.eq_dec; try congruence; rewrite find_funct.
-          rewrite H0 in REC_CURCOMP; simpl in REC_CURCOMP. destruct Ptrofs.eq_dec; try congruence; rewrite H1 in REC_CURCOMP.
-          rewrite REC_CURCOMP.
-          (* Q: am I missing something?? *)
-          admit.
-      + eauto.
-      + simpl in same_side.
-        econstructor; eauto.
-        simpl. rewrite <- same_side. rewrite H0. simpl. now rewrite H1.
-      + (* Am missing the weak relation between state and returnstate *)
-        admit.
-
-    (** [ReturnState] to [State] *)
-    - admit.
-
-    (** Builtin *)
-    - admit.
-
-    (** External call *)
-    - admit.
-*)
-  Admitted.
-
-  Lemma simulation:
-    @threeway_simulation (semantics W1) (semantics W2) (semantics W3) single_L1 single_L2 single_L3.
+  (* Returns *)
+  Lemma update_stack_return_preserved_internal:
+    forall j__δ rs1 rs3 st1 st1' st3 cp
+      (agr: agrees_with j__δ (init_meminj W1 W3))
+      (delta_zero: mem_delta_zero j__δ),
+      (rs1 PC <> Vundef) ->
+      Genv.find_comp ge1 (rs1 PC) = Some cp ->
+      regset_rel j__δ rs1 rs3 ->
+      update_stack_return ge1 st1 cp rs1 = Some st1' ->
+      st1' = st1 /\
+        update_stack_return ge3 st3 cp rs3 = Some st3.
   Proof.
-    (* apply threeway_simulation_diagram with (strong_equivalence1 := strong_equivalence s ge1 ge3 Left) *)
-    (*                                        (strong_equivalence2 := strong_equivalence s ge2 ge3 Right) *)
-    (*                                        (weak_equivalence1   := weak_equivalence   s ge1 ge3 Left) *)
-    (*                                        (weak_equivalence2   := weak_equivalence   s ge1 ge3 Right) *)
-    (*                                        (order := fun _ _ => True). *)
-    (* - apply public_symbol_eq21. *)
-    (* - apply public_symbol_eq32. *)
-    (* - admit. *)
-    (* - admit. *)
-    (* - admit. *)
-    (* - *)
-  Admitted.
+    intros * agr delta_zero nundef samecomp rs1_rs3 (* st_rel *).
+    unfold update_stack_return.
+    rewrite samecomp, Pos.eqb_refl.
+    intros R; inv R.
+    split; eauto.
+    exploit (agrees_with_init_meminj_find_comp_preserved s W1 W3); eauto.
+    intros ->. rewrite Pos.eqb_refl. reflexivity.
+  Qed.
 
-End Simulation.
+  (* Builtins and external calls arguments *)
+  Lemma eval_builtin_arg_inject:
+    forall (rs: regset) m j__δ rs' m' a v
+      (eval: eval_builtin_arg ge1 rs (rs X2) m a v)
+      (* (agr: agrees_with j__δ (init_meminj W1 W3)) *)
+      (inj_pres: meminj_preserves_globals s δ W1 W3 j__δ)
+      (m_m': mem_rel s ge1 ge3 j__δ δ m m')
+      (delta_zero: mem_delta_zero j__δ),
+      regset_rel j__δ rs rs' ->
+      Mem.inject j__δ m m' ->
+      exists v',
+        eval_builtin_arg ge3 rs' (rs' X2) m' a v'
+        /\ Val.inject j__δ v v'.
+  Proof.
+    induction 1; intros AGR MREL DZ RS MI.
+    - exists rs'#x; split; auto. constructor.
+    - econstructor; eauto with barg.
+    - econstructor; eauto with barg.
+    - econstructor; eauto with barg.
+    - econstructor; eauto with barg.
+    - specialize (RS X2); destruct (rs X2); inv RS; simpl in H; try congruence.
+      exploit DZ; eauto; intros ->.
+      rewrite Ptrofs.add_zero in *.
+      exploit Mem.load_inject; eauto.
+      intros (v' & A & B). exists v'; split; auto with barg.
+      rewrite Z.add_0_r in A.
+      econstructor. simpl; eauto.
+    - econstructor; split; eauto with barg.
+      eapply Val.offset_ptr_inject. now apply RS.
+    - assert (Val.inject j__δ (Senv.symbol_address ge1 id ofs) (Senv.symbol_address ge3 id ofs)).
+      { unfold Senv.symbol_address in *; simpl; unfold Genv.symbol_address in *.
+        destruct (Genv.find_symbol ge1 id) as [b|] eqn:FS; auto.
+        unfold Senv.find_symbol in H.
+        simpl in H. rewrite FS in H.
+        simpl in H.
+        Local Transparent Mem.load.
+        unfold Mem.load in H. Local Opaque Mem.load.
+        destruct (Mem.valid_access_dec) as [e | n]; try congruence.
+        unfold Mem.valid_access in e.
+        destruct e as [_ [e ?]]. simpl in e.
+        exploit symbols_inject2; eauto. intros (b' & A & B). rewrite A.
+        econstructor; eauto. rewrite Ptrofs.add_zero; auto. }
+      exploit Mem.loadv_inject; eauto. intros (v' & A & B).
+      exists v'; split; auto with barg.
+      econstructor. simpl; eauto.
+    - econstructor; split; eauto with barg.
+      unfold Senv.symbol_address; simpl.
+    (* - econstructor; split; eauto with barg. *)
+    (*   subst res. *)
+    (*   unfold Genv.symbol_address; simpl; unfold Genv.symbol_address. *)
+      destruct (Genv.find_symbol ge1 id) as [b|] eqn:FS; auto.
+      exploit symbols_inject2; eauto. intros (b' & A & B). rewrite A.
+      econstructor; eauto. now rewrite Ptrofs.add_zero.
+      (* destruct (Genv.find_comp_of_block ge1 b) eqn:FB; auto. *)
+      (* erewrite <- (find_comp_of_block_preserved s W1 W3); eauto. rewrite FB. *)
+      (* destruct (cp =? c)%positive; auto. *)
+      (* econstructor; eauto. now rewrite Ptrofs.add_zero. *)
+      (* destruct (Genv.find_def ge1 b) as [[] |] eqn:?; auto. *)
+      (* exploit defs_inject; eauto. *)
+      (* intros ([] & ? & _ & ? & ?). rewrite H. *)
+      (* econstructor; eauto. now rewrite Ptrofs.add_zero. *)
+      (* inv H0. *)
+    - destruct IHeval1 as (v1' & A1 & B1); eauto using in_or_app.
+      destruct IHeval2 as (v2' & A2 & B2); eauto using in_or_app.
+      exists (Val.longofwords v1' v2'); split; auto with barg.
+      apply Val.longofwords_inject; auto.
+    - destruct IHeval1 as (v1' & A1 & B1); eauto using in_or_app.
+      destruct IHeval2 as (v2' & A2 & B2); eauto using in_or_app.
+      econstructor; split; eauto with barg.
+      destruct Archi.ptr64; auto using Val.add_inject, Val.addl_inject.
+  Qed.
 
+  Lemma eval_builtin_args_inject:
+    forall (rs: regset) m j__δ rs' m' al vl
+      (eval: eval_builtin_args ge1 rs (rs X2) m al vl)
+      (inj_pres: meminj_preserves_globals s δ W1 W3 j__δ)
+      (* (agr: agrees_with j__δ (init_meminj W1 W3)) *)
+      (m_m': mem_rel s ge1 ge3 j__δ δ m m')
+      (delta_zero: mem_delta_zero j__δ),
+      regset_rel j__δ rs rs' ->
+      Mem.inject j__δ m m' ->
+      (* (forall id, In id (globals_of_builtin_args al) -> kept id) -> *)
+      exists vl',
+        eval_builtin_args ge3 rs' (rs' X2) m' al vl'
+        /\ Val.inject_list j__δ vl vl'.
+  Proof.
+    induction 1; intros.
+    - exists (@nil val); split; constructor.
+    - exploit eval_builtin_arg_inject; eauto using in_or_app. intros (v1' & A & B).
+      destruct IHeval as (vl' & C & D); eauto using in_or_app.
+      exists (v1' :: vl'); split; constructor; auto.
+  Qed.
+
+  Lemma extcall_arguments_preserved:
+    forall j__δ δ m1 m3 rs1 rs3,
+      mem_rel s ge1 ge3 j__δ δ m1 m3 ->
+      regset_rel j__δ rs1 rs3 ->
+      forall sig args, extcall_arguments rs1 m1 sig args ->
+                  exists args', Val.inject_list j__δ args args'
+                           /\ extcall_arguments rs3 m3 sig args'.
+  Proof.
+    intros * m1_m3 rs1_rs3 sig args H.
+    unfold extcall_arguments in H.
+    unfold extcall_arguments.
+    induction H.
+    - exists nil. split; auto. constructor.
+    - assert (exists b1', Val.inject j__δ b1 b1' /\ extcall_arg_pair rs3 m3 a1 b1').
+      { inv H.
+        - inv H1.
+          + specialize (rs1_rs3 (preg_of r)).
+            exists (rs3 (preg_of r)). split; eauto. constructor; constructor.
+          + exploit Mem.loadv_inject; eauto using partial_mem_inject.
+            eapply Val.offset_ptr_inject. eapply rs1_rs3.
+            intros [b1' [? ?]].
+            exists b1'; split. eauto. constructor. econstructor; eauto.
+        - inv H1; inv H2.
+          + pose proof (rs1_rs3 (preg_of r)).
+            pose proof (rs1_rs3 (preg_of r0)).
+            eexists; split; [eapply Val.longofwords_inject; eauto |].
+            constructor; constructor; eauto.
+          + pose proof (rs1_rs3 (preg_of r)).
+            exploit Mem.loadv_inject; eauto using partial_mem_inject.
+            eapply Val.offset_ptr_inject. eapply rs1_rs3.
+            intros [b1' [? ?]].
+            eexists; split; [eapply Val.longofwords_inject; eauto |].
+            constructor; econstructor; eauto.
+          + pose proof (rs1_rs3 (preg_of r)).
+            exploit Mem.loadv_inject; eauto using partial_mem_inject.
+            eapply Val.offset_ptr_inject. eapply rs1_rs3.
+            intros [b1' [? ?]].
+            eexists; split; [eapply Val.longofwords_inject; eauto |].
+            constructor; econstructor; eauto.
+          + exploit Mem.loadv_inject; eauto using partial_mem_inject.
+            eapply Val.offset_ptr_inject. eapply rs1_rs3. clear H1.
+            exploit Mem.loadv_inject; eauto using partial_mem_inject.
+            eapply Val.offset_ptr_inject. eapply rs1_rs3.
+            intros [b1' [? ?]].
+            intros [b0' [? ?]].
+            eexists; split; [eapply Val.longofwords_inject; eauto |].
+            constructor; econstructor; eauto. }
+      destruct IHlist_forall2 as [? [? ?]].
+      destruct H1 as [? [? ?]].
+      eexists (cons _ _); split.
+      + constructor; eassumption.
+      + constructor; eauto.
+  Qed.
+
+
+  (* External calls preserved *)
+  Lemma external_call_inject_left:
+    forall ef vargs m1 t vres m2 j__δ j__oppδ m1' vargs' m3 rs1 rs3 st1 st2 st3,
+      s (comp_of ef) = δ ->
+      meminj_preserves_globals s δ W1 W3 j__δ ->
+      (* agrees_with j__δ (init_meminj W1 W3) -> *)
+      external_call ef ge1 vargs m1 t vres m1' ->
+      Val.inject_list j__δ vargs vargs' ->
+
+      mem_rel s ge1 ge3 j__δ δ m1 m3 ->
+      mem_rel s ge2 ge3 j__oppδ (opposite δ) m2 m3 ->
+      regset_rel j__δ rs1 rs3 ->
+      stack_rel s ge3 δ j__δ j__oppδ st1 st2 st3 ->
+
+      exists j__δ', exists vres', exists m3',
+        external_call ef ge3 vargs' m3 t vres' m3'
+        /\ Val.inject j__δ' vres vres'
+        /\ Mem.unchanged_on (loc_unmapped j__δ) m1 m1'
+        /\ Mem.unchanged_on (loc_out_of_reach j__δ m1) m3 m3'
+        /\ inject_incr j__δ j__δ'
+        /\ inject_separated j__δ j__δ' m1 m3 /\
+      (* agrees_with j__δ' (init_meminj W1 W3) /\ *)
+          meminj_preserves_globals s δ W1 W3 j__δ' /\
+          mem_rel s ge1 ge3 j__δ' δ m1' m3' /\
+          mem_rel s ge2 ge3 j__oppδ (opposite δ) m2 m3' /\
+          regset_rel j__δ' rs1 rs3 /\
+          stack_rel s ge3 δ j__δ' j__oppδ st1 st2 st3.
+  Proof.
+    intros * s_ef inj_pres extcall1 inj_args m1_m3 m2_m3 rs1_rs3 st_rel.
+    exploit external_call_mem_inject_gen;
+      eauto using globals_symbols_inject, partial_mem_inject.
+    intros
+      (j__δ' & vres' & m3' & extcall3 & inj_res & inj_mem & unchanged1 & unchanged2 & incr & inj_sep & comp_new).
+
+    eexists; eexists; eexists; intuition eauto.
+    - assert (meminj_preserves_globals s δ W1 W3 j__δ ->
+              mem_rel s ge1 ge3 j__δ δ m1 m3 ->
+              inject_incr j__δ j__δ' ->
+              inject_separated j__δ j__δ' m1 m3 ->
+              meminj_preserves_globals s δ W1 W3 j__δ').
+      { clear. intros m1_m3 inj_pres incr inj_sep.
+        constructor.
+        - (* symbols_inject1 *)
+          intros.
+          exploit symbols_inject2; eauto.
+          intros [? [? ?]]. eapply symbols_inject1; eauto.
+          erewrite (incr b) in *; eauto. congruence.
+        - (* symbols_inject2 *)
+          intros.
+          exploit symbols_inject2; eauto.
+          intros [? [? ?]].
+          now erewrite (incr b) in *; eauto.
+        - (* symbols_inject3 *)
+          intros.
+          exploit symbols_inject3; eauto.
+          intros [? [? ?]]. eexists.
+          erewrite (incr x) in *; eauto.
+        - (* defs_inject *)
+          intros. exploit defs_inject; eauto.
+          destruct (j__δ b) as [[] |] eqn:j_b; [erewrite (incr b) in *; eauto |].
+          exfalso.
+          exploit inj_sep; eauto. exploit find_def_valid1; eauto. intros ? [? ?]; congruence.
+        - (* defs_rev_inject *)
+          intros. exploit defs_rev_inject; eauto.
+          destruct (j__δ b) as [[] |] eqn:j_b; [erewrite (incr b) in *; eauto |].
+          exfalso.
+          exploit inj_sep; eauto. exploit find_def_valid2; eauto. intros ? [? ?]; congruence. }
+      eauto.
+    - exploit extcall_preserves_mem_rel_same_side; eauto.
+    - exploit extcall_preserves_mem_rel_opp_side2; eauto.
+      now destruct δ.
+    - intros x. exploit val_inject_incr; eauto.
+    - exploit inject_incr_stack_rel1; eauto.
+      Admitted.
+  (* Qed. *)
+
+  (* Lemmas about correct register invalidation *)
+  Lemma regset_rel_return_from_builtin:
+    forall j rs1 rs2 vres vres' ef res
+      (RES_NOT_PC : exists reg : builtin_res mreg, res = map_builtin_res preg_of reg),
+      regset_rel j rs1 rs2 ->
+      Val.inject j vres vres' ->
+      regset_rel j
+        (nextinstr (set_res res vres (undef_regs (map preg_of (destroyed_by_builtin ef)) (rs1 # X1 <- Vundef) # X31 <- Vundef)))
+        (nextinstr (set_res res vres' (undef_regs (map preg_of (destroyed_by_builtin ef)) (rs2 # X1 <- Vundef) # X31 <- Vundef))).
+  Proof.
+    intros j rs1 rs2 vres vres' ef res RES_NOT_PC H res_inj.
+    apply regset_rel_inject; auto.
+    - assert (H': regset_rel j
+                    (undef_regs (map preg_of (destroyed_by_builtin ef)) (rs1 # X1 <- Vundef) # X31 <- Vundef)
+                    (undef_regs (map preg_of (destroyed_by_builtin ef)) (rs2 # X1 <- Vundef) # X31 <- Vundef)).
+      { remember (map preg_of (destroyed_by_builtin ef)) as pregs eqn:X. clear X.
+        assert (rel: regset_rel j ((rs1 # X1 <- Vundef) # X31 <- Vundef) ((rs2 # X1 <- Vundef) # X31 <- Vundef)).
+        { do 2 (apply regset_rel_inject; auto). }
+        remember ((rs2 # X1 <- Vundef) # X31 <- Vundef) as regs'.
+        remember ((rs1 # X1 <- Vundef) # X31 <- Vundef) as regs.
+        clear -rel.
+        revert regs regs' rel.
+        induction pregs.
+        - now auto.
+        - intros. simpl. apply IHpregs. apply regset_rel_inject; auto. }
+      remember (undef_regs (map preg_of (destroyed_by_builtin ef)) (rs1 # X1 <- Vundef) # X31 <- Vundef)
+        as regs1 eqn:X; clear X.
+      remember (undef_regs (map preg_of (destroyed_by_builtin ef)) (rs2 # X1 <- Vundef) # X31 <- Vundef)
+        as regs2 eqn:X; clear X.
+      clear -res_inj H'.
+      revert regs1 regs2 vres vres' res_inj H'.
+      induction res; intros.
+      + simpl; apply regset_rel_inject; auto.
+      + simpl; auto.
+      + simpl; auto. apply IHres2; auto using Val.loword_inject.
+        eapply IHres1; auto using Val.hiword_inject.
+    - destruct RES_NOT_PC as [reg ?]; subst res.
+      assert (H': Asmgenproof0.preg_notin PC (destroyed_by_builtin ef)).
+      { Local Transparent destroyed_by_builtin.
+        unfold destroyed_by_builtin.
+        destruct ef; simpl; auto.
+        - destruct orb; simpl; intuition.
+          destruct orb; simpl; intuition.
+        - intuition.
+        - induction clobbers.
+          + simpl; auto.
+          + simpl. destruct register_by_name; auto.
+            simpl; intuition.
+            destruct (destroyed_by_clobber clobbers); [| split]; now destruct m.
+            Local Opaque destroyed_by_builtin. }
+      rewrite 2!Asmgenproof0.set_res_other; auto.
+      rewrite 2!Asmgenproof0.undef_regs_other_2; auto.
+      Simpl. apply Val.offset_ptr_inject. now apply H.
+  Qed.
+
+  Lemma regset_rel_return_from_external:
+    forall j rs1 rs2 ef res1 res2,
+      regset_rel j rs1 rs2 ->
+      Val.inject j res1 res2 ->
+      regset_rel j ((set_pair (loc_external_result (ef_sig ef)) res1 (undef_caller_save_regs rs1)) # PC <- (rs1 X1))
+        ((set_pair (loc_external_result (ef_sig ef)) res2 (undef_caller_save_regs rs2)) # PC <- (rs2 X1)).
+  Proof.
+    intros j rs1 rs2 ef res1 res2 H H0.
+    eapply regset_rel_inject; eauto.
+    destruct (loc_external_result (ef_sig ef)).
+    - eapply regset_rel_inject; eauto.
+      { unfold undef_caller_save_regs.
+        intros x. destruct orb; auto. }
+    - eapply regset_rel_inject; eauto using Val.loword_inject.
+      eapply regset_rel_inject; eauto using Val.hiword_inject.
+      { unfold undef_caller_save_regs.
+        intros x. destruct orb; auto. }
+  Qed.
